<?xml version="1.0"?>
<rdf:RDF xmlns="http://hit2gap.eu/h2g/h2gBI#"
     xml:base="http://hit2gap.eu/h2g/h2gBI"
     xmlns:rdf="http://www.w3.org/1999/02/22-rdf-syntax-ns#"
     xmlns:terms="http://purl.org/dc/terms/"
     xmlns:owl="http://www.w3.org/2002/07/owl#"
     xmlns:xml="http://www.w3.org/XML/1998/namespace"
     xmlns:xsd="http://www.w3.org/2001/XMLSchema#"
     xmlns:skos="http://www.w3.org/2004/02/skos/core#"
     xmlns:rdfs="http://www.w3.org/2000/01/rdf-schema#"
     xmlns:dc="http://purl.org/dc/elements/1.1/">
    <owl:Ontology rdf:about="http://hit2gap.eu/h2g/h2gBI#">
        <owl:imports rdf:resource="http://hit2gap.eu/h2g/h2gProperty#"/>
        <owl:versionInfo xml:lang="en">This current version includes the initial version of the semantic model based on the diagrams generated.</owl:versionInfo>
        <dc:creator xml:lang="en">Aitor Corchero (aitor.corchero@eurecat.org)</dc:creator>
        <dc:creator xml:lang="en">Pierre Bourreau (pbourreau@nobatek.com)</dc:creator>
        <dc:title xml:lang="en">Hit2Gap Ontology-Building Infrastructure</dc:title>
        <terms:license xml:lang="en">https://opensource.org/licenses/MIT</terms:license>
        <dc:creator xml:lang="en">Yudith Cardinale (ycardinale@usb.ve)</dc:creator>
        <dc:creator xml:lang="en">Richard Chbeir (richard.chbeir@univ-pau.fr)</dc:creator>
        <dc:description xml:lang="en">Features of interest are real world representations of the building. They comprise building infrastructure and the corresponding building elements (mechanical and electrical elements, furniture, etc.).

To adapt the SSN ontology to the building domain, the ifcOwl which is the web semantic ontology for the Industry Foundation Class (IFC), has been incorporated. This semantic model permits to link the proposed ontology with the BIM notation.

To do so, the feature of interest class of SSN has been linked (hierarchically) with the concepts Ifc:Building, Ifc:BuildingElement, and Ifc:BuildingAppliance. Each building pertains to a specific type (through the &quot;hasType&quot; semantic relation). Considering their infrastructure, each building contains several real work zones (Ifc:Zone). These zones can be rooms, floors, desk, etc. Moreover, different views of a building can be used: infrastructure to represent the floors, rooms...; but also an electric view (to represent the electric appliances inside the building), fluid view (to represent the possible flow of water/gas inside the building), etc. 
Over these abstracted views, the different building elements are represented: building systems (&quot;Flow Instruments&quot;, &quot;Protective Devices&quot;, “Unitary Control Elements&quot;), sensors and building appliance for monitoring and controlling the building, occupants’ devices, etc. 
The features of interest representation of the building are performed using standard building modelling (IFC and BIM). Moreover, this semantic model ensures the information compatibility and sharing with these models. A part of this, the building infrastructure and their corresponding zones and devices are modelled and linked with their corresponding information, aspect that facilitates data querying based on the corresponding feature of interests.</dc:description>
    </owl:Ontology>
    


    <!-- 
    ///////////////////////////////////////////////////////////////////////////////////////
    //
    // Annotation properties
    //
    ///////////////////////////////////////////////////////////////////////////////////////
     -->

    


    <!-- http://purl.org/dc/elements/1.1/creator -->

    <owl:AnnotationProperty rdf:about="http://purl.org/dc/elements/1.1/creator"/>
    


    <!-- http://purl.org/dc/elements/1.1/description -->

    <owl:AnnotationProperty rdf:about="http://purl.org/dc/elements/1.1/description"/>
    


    <!-- http://purl.org/dc/elements/1.1/title -->

    <owl:AnnotationProperty rdf:about="http://purl.org/dc/elements/1.1/title"/>
    


    <!-- http://purl.org/dc/terms/license -->

    <owl:AnnotationProperty rdf:about="http://purl.org/dc/terms/license"/>
    


    <!-- 
    ///////////////////////////////////////////////////////////////////////////////////////
    //
    // Datatypes
    //
    ///////////////////////////////////////////////////////////////////////////////////////
     -->

    


    <!-- http://www.buildingsmart-tech.org/ifcOWL/IFC2X3_Final#IfcWindowTypeEnum -->

    <rdfs:Datatype rdf:about="http://www.buildingsmart-tech.org/ifcOWL/IFC2X3_Final#IfcWindowTypeEnum">
        <rdfs:isDefinedBy rdf:resource="http://www.buildingsmart-tech.org/ifcOWL/IFC2X3_Final#IfcWindowTypeEnum"/>
        <rdfs:label xml:lang="en">IfcWindowTypeEnum</rdfs:label>
        <owl:equivalentClass>
            <rdfs:Datatype>
                <owl:oneOf>
                    <rdf:Description>
                        <rdf:type rdf:resource="http://www.w3.org/1999/02/22-rdf-syntax-ns#List"/>
                        <rdf:first>LIGHTDOME</rdf:first>
                        <rdf:rest>
                            <rdf:Description>
                                <rdf:type rdf:resource="http://www.w3.org/1999/02/22-rdf-syntax-ns#List"/>
                                <rdf:first>NOTDEFINED</rdf:first>
                                <rdf:rest>
                                    <rdf:Description>
                                        <rdf:type rdf:resource="http://www.w3.org/1999/02/22-rdf-syntax-ns#List"/>
                                        <rdf:first>SKYLIGHT</rdf:first>
                                        <rdf:rest>
                                            <rdf:Description>
                                                <rdf:type rdf:resource="http://www.w3.org/1999/02/22-rdf-syntax-ns#List"/>
                                                <rdf:first>USERDEFINED</rdf:first>
                                                <rdf:rest>
                                                    <rdf:Description>
                                                        <rdf:type rdf:resource="http://www.w3.org/1999/02/22-rdf-syntax-ns#List"/>
                                                        <rdf:first>WINDOW</rdf:first>
                                                        <rdf:rest rdf:resource="http://www.w3.org/1999/02/22-rdf-syntax-ns#nil"/>
                                                    </rdf:Description>
                                                </rdf:rest>
                                            </rdf:Description>
                                        </rdf:rest>
                                    </rdf:Description>
                                </rdf:rest>
                            </rdf:Description>
                        </rdf:rest>
                    </rdf:Description>
                </owl:oneOf>
            </rdfs:Datatype>
        </owl:equivalentClass>
    </rdfs:Datatype>
    


    <!-- http://www.buildingsmart-tech.org/ifcOWL/IFC2X3_Final#IfcWindowTypePartitioningEnum -->

    <rdfs:Datatype rdf:about="http://www.buildingsmart-tech.org/ifcOWL/IFC2X3_Final#IfcWindowTypePartitioningEnum">
        <rdfs:label rdf:resource="http://www.buildingsmart-tech.org/ifcOWL/IFC2X3_Final#IfcWindowTypePartitioningEnum"/>
        <rdfs:label xml:lang="en">IfcWindowTypePartitioningEnum</rdfs:label>
        <owl:equivalentClass>
            <rdfs:Datatype>
                <owl:oneOf>
                    <rdf:Description>
                        <rdf:type rdf:resource="http://www.w3.org/1999/02/22-rdf-syntax-ns#List"/>
                        <rdf:first>DOUBLE_PANEL_HORIZONTAL</rdf:first>
                        <rdf:rest>
                            <rdf:Description>
                                <rdf:type rdf:resource="http://www.w3.org/1999/02/22-rdf-syntax-ns#List"/>
                                <rdf:first>DOUBLE_PANEL_VERTICAL</rdf:first>
                                <rdf:rest>
                                    <rdf:Description>
                                        <rdf:type rdf:resource="http://www.w3.org/1999/02/22-rdf-syntax-ns#List"/>
                                        <rdf:first>NOTDEFINED</rdf:first>
                                        <rdf:rest>
                                            <rdf:Description>
                                                <rdf:type rdf:resource="http://www.w3.org/1999/02/22-rdf-syntax-ns#List"/>
                                                <rdf:first>SINGLE_PANEL</rdf:first>
                                                <rdf:rest>
                                                    <rdf:Description>
                                                        <rdf:type rdf:resource="http://www.w3.org/1999/02/22-rdf-syntax-ns#List"/>
                                                        <rdf:first>TRIPLE_PANEL_BOTTOM</rdf:first>
                                                        <rdf:rest>
                                                            <rdf:Description>
                                                                <rdf:type rdf:resource="http://www.w3.org/1999/02/22-rdf-syntax-ns#List"/>
                                                                <rdf:first>TRIPLE_PANEL_HORIZONTAL</rdf:first>
                                                                <rdf:rest>
                                                                    <rdf:Description>
                                                                        <rdf:type rdf:resource="http://www.w3.org/1999/02/22-rdf-syntax-ns#List"/>
                                                                        <rdf:first>TRIPLE_PANEL_LEFT</rdf:first>
                                                                        <rdf:rest>
                                                                            <rdf:Description>
                                                                                <rdf:type rdf:resource="http://www.w3.org/1999/02/22-rdf-syntax-ns#List"/>
                                                                                <rdf:first>TRIPLE_PANEL_RIGHT</rdf:first>
                                                                                <rdf:rest>
                                                                                    <rdf:Description>
                                                                                        <rdf:type rdf:resource="http://www.w3.org/1999/02/22-rdf-syntax-ns#List"/>
                                                                                        <rdf:first>TRIPLE_PANEL_TOP</rdf:first>
                                                                                        <rdf:rest>
                                                                                            <rdf:Description>
                                                                                                <rdf:type rdf:resource="http://www.w3.org/1999/02/22-rdf-syntax-ns#List"/>
                                                                                                <rdf:first>TRIPLE_PANEL_VERTICAL</rdf:first>
                                                                                                <rdf:rest>
                                                                                                    <rdf:Description>
                                                                                                        <rdf:type rdf:resource="http://www.w3.org/1999/02/22-rdf-syntax-ns#List"/>
                                                                                                        <rdf:first>USERDEFINED</rdf:first>
                                                                                                        <rdf:rest rdf:resource="http://www.w3.org/1999/02/22-rdf-syntax-ns#nil"/>
                                                                                                    </rdf:Description>
                                                                                                </rdf:rest>
                                                                                            </rdf:Description>
                                                                                        </rdf:rest>
                                                                                    </rdf:Description>
                                                                                </rdf:rest>
                                                                            </rdf:Description>
                                                                        </rdf:rest>
                                                                    </rdf:Description>
                                                                </rdf:rest>
                                                            </rdf:Description>
                                                        </rdf:rest>
                                                    </rdf:Description>
                                                </rdf:rest>
                                            </rdf:Description>
                                        </rdf:rest>
                                    </rdf:Description>
                                </rdf:rest>
                            </rdf:Description>
                        </rdf:rest>
                    </rdf:Description>
                </owl:oneOf>
            </rdfs:Datatype>
        </owl:equivalentClass>
    </rdfs:Datatype>
    


    <!-- 
    ///////////////////////////////////////////////////////////////////////////////////////
    //
    // Object Properties
    //
    ///////////////////////////////////////////////////////////////////////////////////////
     -->

    


    <!-- http://data.qudt.org/qudt/owl/1.0.0/qudt.owl#hasUnit -->

    <owl:ObjectProperty rdf:about="http://data.qudt.org/qudt/owl/1.0.0/qudt.owl#hasUnit">
        <rdfs:isDefinedBy xml:lang="en">http://data.qudt.org/qudt/owl/1.0.0/qudt.owl#hasUnit</rdfs:isDefinedBy>
    </owl:ObjectProperty>
    


    <!-- http://hit2gap.eu/h2g/h2gBI#InputOutput -->

    <owl:ObjectProperty rdf:about="http://hit2gap.eu/h2g/h2gBI#InputOutput"/>
    


    <!-- http://hit2gap.eu/h2g/h2gBI#MeasureInputOutput -->

    <owl:ObjectProperty rdf:about="http://hit2gap.eu/h2g/h2gBI#MeasureInputOutput"/>
    


    <!-- http://hit2gap.eu/h2g/h2gBI#OpenClose -->

    <owl:ObjectProperty rdf:about="http://hit2gap.eu/h2g/h2gBI#OpenClose"/>
    


    <!-- http://hit2gap.eu/h2g/h2gBI#consumes -->

    <owl:ObjectProperty rdf:about="http://hit2gap.eu/h2g/h2gBI#consumes"/>
    


    <!-- http://hit2gap.eu/h2g/h2gBI#contains -->

    <owl:ObjectProperty rdf:about="http://hit2gap.eu/h2g/h2gBI#contains">
        <owl:inverseOf rdf:resource="http://hit2gap.eu/h2g/h2gBI#isContainedIn"/>
    </owl:ObjectProperty>
    


    <!-- http://hit2gap.eu/h2g/h2gBI#controls -->

    <owl:ObjectProperty rdf:about="http://hit2gap.eu/h2g/h2gBI#controls"/>
    


    <!-- http://hit2gap.eu/h2g/h2gBI#hasH2GProperty -->

    <owl:ObjectProperty rdf:about="http://hit2gap.eu/h2g/h2gBI#hasH2GProperty"/>
    


    <!-- http://hit2gap.eu/h2g/h2gBI#hasLampType -->

    <owl:ObjectProperty rdf:about="http://hit2gap.eu/h2g/h2gBI#hasLampType"/>
    


    <!-- http://hit2gap.eu/h2g/h2gBI#hasOrientation -->

    <owl:ObjectProperty rdf:about="http://hit2gap.eu/h2g/h2gBI#hasOrientation"/>
    


    <!-- http://hit2gap.eu/h2g/h2gBI#hasSpaceCapacity -->

    <owl:ObjectProperty rdf:about="http://hit2gap.eu/h2g/h2gBI#hasSpaceCapacity"/>
    


    <!-- http://hit2gap.eu/h2g/h2gBI#hasState -->

    <owl:ObjectProperty rdf:about="http://hit2gap.eu/h2g/h2gBI#hasState"/>
    


    <!-- http://hit2gap.eu/h2g/h2gBI#hasType -->

    <owl:ObjectProperty rdf:about="http://hit2gap.eu/h2g/h2gBI#hasType"/>
    


    <!-- http://hit2gap.eu/h2g/h2gBI#hasWindowCovering -->

    <owl:ObjectProperty rdf:about="http://hit2gap.eu/h2g/h2gBI#hasWindowCovering">
        <rdfs:subPropertyOf rdf:resource="http://www.w3.org/2002/07/owl#topObjectProperty"/>
        <rdf:type rdf:resource="http://www.w3.org/2002/07/owl#FunctionalProperty"/>
    </owl:ObjectProperty>
    


    <!-- http://hit2gap.eu/h2g/h2gBI#hasWindowGlazing -->

    <owl:ObjectProperty rdf:about="http://hit2gap.eu/h2g/h2gBI#hasWindowGlazing">
        <rdf:type rdf:resource="http://www.w3.org/2002/07/owl#FunctionalProperty"/>
    </owl:ObjectProperty>
    


    <!-- http://hit2gap.eu/h2g/h2gBI#inContactWith -->

    <owl:ObjectProperty rdf:about="http://hit2gap.eu/h2g/h2gBI#inContactWith"/>
    


    <!-- http://hit2gap.eu/h2g/h2gBI#isContainedIn -->

    <owl:ObjectProperty rdf:about="http://hit2gap.eu/h2g/h2gBI#isContainedIn">
        <rdfs:label rdf:datatype="http://www.w3.org/2001/XMLSchema#string">isContainedIn</rdfs:label>
    </owl:ObjectProperty>
    


    <!-- http://hit2gap.eu/h2g/h2gBI#isLocatedIn -->

    <owl:ObjectProperty rdf:about="http://hit2gap.eu/h2g/h2gBI#isLocatedIn"/>
    


    <!-- http://hit2gap.eu/h2g/h2gBI#locatedInClimate -->

    <owl:ObjectProperty rdf:about="http://hit2gap.eu/h2g/h2gBI#locatedInClimate"/>
    


    <!-- http://hit2gap.eu/h2g/h2gBI#produces -->

    <owl:ObjectProperty rdf:about="http://hit2gap.eu/h2g/h2gBI#produces"/>
    


    <!-- http://hit2gap.eu/h2g/h2gBI#stores -->

    <owl:ObjectProperty rdf:about="http://hit2gap.eu/h2g/h2gBI#stores"/>
    


    <!-- http://hit2gap.eu/h2g/h2gBI#transports -->

    <owl:ObjectProperty rdf:about="http://hit2gap.eu/h2g/h2gBI#transports"/>
    


    <!-- http://hit2gap.eu/h2g/h2gBI#wasLocated -->

    <owl:ObjectProperty rdf:about="http://hit2gap.eu/h2g/h2gBI#wasLocated"/>
    


    <!-- http://hit2gap.eu/h2g/h2gSensor#hasObservationResultTime -->

    <owl:ObjectProperty rdf:about="http://hit2gap.eu/h2g/h2gSensor#hasObservationResultTime">
        <rdfs:isDefinedBy xml:lang="en">http://hit2gap.eu/h2g/h2gSensor#hasObservationResultTime</rdfs:isDefinedBy>
    </owl:ObjectProperty>
    


    <!-- http://hit2gap.eu/h2g/h2gSensor#locatedInHemisphere -->

    <owl:ObjectProperty rdf:about="http://hit2gap.eu/h2g/h2gSensor#locatedInHemisphere">
        <rdfs:isDefinedBy xml:lang="en">http://hit2gap.eu/h2g/h2gSensor#locatedInHemisphere</rdfs:isDefinedBy>
    </owl:ObjectProperty>
    


    <!-- http://hit2gap.eu/ontomg#hasA -->

    <owl:ObjectProperty rdf:about="http://hit2gap.eu/ontomg#hasA">
        <rdfs:isDefinedBy xml:lang="en">http://hit2gap.eu/ontomg#hasA</rdfs:isDefinedBy>
    </owl:ObjectProperty>
    


    <!-- http://hit2gap.eu/ontomg#hasBranch -->

    <owl:ObjectProperty rdf:about="http://hit2gap.eu/ontomg#hasBranch">
        <rdfs:isDefinedBy xml:lang="en">http://hit2gap.eu/ontomg#hasBranch</rdfs:isDefinedBy>
    </owl:ObjectProperty>
    


    <!-- http://hit2gap.eu/ontomg#isComposedOf -->

    <owl:ObjectProperty rdf:about="http://hit2gap.eu/ontomg#isComposedOf">
        <rdfs:isDefinedBy xml:lang="en">http://hit2gap.eu/ontomg#isComposedOf</rdfs:isDefinedBy>
    </owl:ObjectProperty>
    


    <!-- http://www.buildingsmart-tech.org/ifcOWL/IFC2X3_TC1#description_IfcRoot -->

    <owl:ObjectProperty rdf:about="http://www.buildingsmart-tech.org/ifcOWL/IFC2X3_TC1#description_IfcRoot">
        <rdfs:comment xml:lang="en">Optional description, provided for exchanging informative comments.</rdfs:comment>
        <rdfs:isDefinedBy rdf:resource="http://www.buildingsmart-tech.org/ifcOWL/IFC2X3_TC1#description_IfcRoot"/>
        <rdfs:label xml:lang="en">description_IfcRoot</rdfs:label>
    </owl:ObjectProperty>
    


    <!-- http://www.buildingsmart-tech.org/ifcOWL/IFC2X3_TC1#elevation_IfcBuildingStorey -->

    <owl:ObjectProperty rdf:about="http://www.buildingsmart-tech.org/ifcOWL/IFC2X3_TC1#elevation_IfcBuildingStorey"/>
    


    <!-- http://www.buildingsmart-tech.org/ifcOWL/IFC2X3_TC1#globalId_IfcRoot -->

    <owl:ObjectProperty rdf:about="http://www.buildingsmart-tech.org/ifcOWL/IFC2X3_TC1#globalId_IfcRoot">
        <rdfs:comment xml:lang="en">Assignment of a globally unique identifier within the entire software world.</rdfs:comment>
        <rdfs:isDefinedBy rdf:resource="http://www.buildingsmart-tech.org/ifcOWL/IFC2X3_TC1#globalId_IfcRoot"/>
        <rdfs:label xml:lang="en">globalId_IfcRoot</rdfs:label>
    </owl:ObjectProperty>
    


    <!-- http://www.buildingsmart-tech.org/ifcOWL/IFC2X3_TC1#name_IfcRoot -->

    <owl:ObjectProperty rdf:about="http://www.buildingsmart-tech.org/ifcOWL/IFC2X3_TC1#name_IfcRoot">
        <rdfs:comment xml:lang="en">Optional name for use by the participating software systems or users. For some subtypes of IfcRoot the insertion of the Name attribute may be required. This would be enforced by a where rule.</rdfs:comment>
        <rdfs:isDefinedBy rdf:resource="http://www.buildingsmart-tech.org/ifcOWL/IFC2X3_TC1#name_IfcRoot"/>
        <rdfs:label xml:lang="en">name_IfcRoot</rdfs:label>
    </owl:ObjectProperty>
    


    <!-- http://www.buildingsmart-tech.org/ifcOWL/IFC2X3_TC1#refElevation_IfcSite -->

    <owl:ObjectProperty rdf:about="http://www.buildingsmart-tech.org/ifcOWL/IFC2X3_TC1#refElevation_IfcSite">
        <rdfs:comment xml:lang="en">Datum elevation relative to sea level.</rdfs:comment>
        <rdfs:isDefinedBy rdf:resource="http://www.buildingsmart-tech.org/ifcOWL/IFC2X3_TC1#refElevation_IfcSite"/>
        <rdfs:label xml:lang="en">refElevation_IfcSite</rdfs:label>
    </owl:ObjectProperty>
    


    <!-- http://www.buildingsmart-tech.org/ifcOWL/IFC2X3_TC1#refLatitude_IfcSite -->

    <owl:ObjectProperty rdf:about="http://www.buildingsmart-tech.org/ifcOWL/IFC2X3_TC1#refLatitude_IfcSite">
        <rdfs:comment xml:lang="en">World Latitude at reference point (most likely defined in legal description). Defined as integer values for degrees, minutes, seconds, and, optionally, millionths of seconds with respect to the world geodetic system WGS84.
Latitudes are measured relative to the geodetic equator, north of the equator by positive values - from 0 till +90, south of the equator by negative values - from 0 till -90.</rdfs:comment>
        <rdfs:isDefinedBy rdf:resource="http://www.buildingsmart-tech.org/ifcOWL/IFC2X3_TC1#refLatitude_IfcSite"/>
        <rdfs:label xml:lang="en">refLatitude_IfcSite</rdfs:label>
    </owl:ObjectProperty>
    


    <!-- http://www.buildingsmart-tech.org/ifcOWL/IFC2X3_TC1#refLongitude_IfcSite -->

    <owl:ObjectProperty rdf:about="http://www.buildingsmart-tech.org/ifcOWL/IFC2X3_TC1#refLongitude_IfcSite">
        <rdfs:comment xml:lang="en">World Longitude at reference point (most likely defined in legal description). Defined as integer values for degrees, minutes, seconds, and, optionally, millionths of seconds with respect to the world geodetic system WGS84.

Longitudes are measured relative to the geodetic zero meridian, nominally the same as the Greenwich prime meridian: longitudes west of the zero meridian have positive values - from 0 till +180, longitudes east of the zero meridian have negative values - from 0 till -180.</rdfs:comment>
        <rdfs:isDefinedBy rdf:resource="http://www.buildingsmart-tech.org/ifcOWL/IFC2X3_TC1#refLongitude_IfcSite"/>
        <rdfs:label xml:lang="en">refLongitude_IfcSite</rdfs:label>
    </owl:ObjectProperty>
    


    <!-- http://www.georss.org/georss/where -->

    <owl:ObjectProperty rdf:about="http://www.georss.org/georss/where">
        <rdfs:comment rdf:resource="http://www.georss.org/georss/where"/>
    </owl:ObjectProperty>
    


    <!-- http://www.w3.org/ns/sosa/hasFeatureOfInterest -->

    <owl:ObjectProperty rdf:about="http://www.w3.org/ns/sosa/hasFeatureOfInterest">
        <rdfs:isDefinedBy xml:lang="en">http://www.w3.org/ns/sosa/hasFeatureOfInterest</rdfs:isDefinedBy>
    </owl:ObjectProperty>
    


    <!-- http://www.w3.org/ns/sosa/hasResult -->

    <owl:ObjectProperty rdf:about="http://www.w3.org/ns/sosa/hasResult">
        <rdfs:isDefinedBy xml:lang="en">http://www.w3.org/ns/sosa/</rdfs:isDefinedBy>
    </owl:ObjectProperty>
    


    <!-- http://www.w3.org/ns/sosa/madeObservation -->

    <owl:ObjectProperty rdf:about="http://www.w3.org/ns/sosa/madeObservation">
        <rdfs:isDefinedBy xml:lang="en">http://www.w3.org/ns/sosa/madeObservation</rdfs:isDefinedBy>
    </owl:ObjectProperty>
    


    <!-- http://www.w3.org/ns/sosa/observedProperty -->

    <owl:ObjectProperty rdf:about="http://www.w3.org/ns/sosa/observedProperty">
        <rdfs:isDefinedBy xml:lang="en">http://www.w3.org/ns/sosa/observedProperty</rdfs:isDefinedBy>
    </owl:ObjectProperty>
    


    <!-- http://www.w3.org/ns/sosa/observes -->

    <owl:ObjectProperty rdf:about="http://www.w3.org/ns/sosa/observes">
        <rdfs:subPropertyOf rdf:resource="http://www.w3.org/ns/ssn/forProperty"/>
        <rdfs:isDefinedBy xml:lang="en">http://www.w3.org/ns/sosa/observes</rdfs:isDefinedBy>
    </owl:ObjectProperty>
    


    <!-- http://www.w3.org/ns/ssn/forProperty -->

    <owl:ObjectProperty rdf:about="http://www.w3.org/ns/ssn/forProperty">
        <rdfs:isDefinedBy xml:lang="en">http://www.w3.org/ns/ssn/forProperty</rdfs:isDefinedBy>
    </owl:ObjectProperty>
    


    <!-- http://www.w3.org/ns/ssn/hasProperty -->

    <owl:ObjectProperty rdf:about="http://www.w3.org/ns/ssn/hasProperty">
        <rdfs:isDefinedBy xml:lang="en">http://www.w3.org/ns/ssn/hasProperty</rdfs:isDefinedBy>
    </owl:ObjectProperty>
    


    <!-- http://www.w3.org/ns/ssn/hasSubSystem -->

    <owl:ObjectProperty rdf:about="http://www.w3.org/ns/ssn/hasSubSystem">
        <rdfs:isDefinedBy xml:lang="en">http://www.w3.org/ns/ssn/hasSubSystem</rdfs:isDefinedBy>
    </owl:ObjectProperty>
    


    <!-- 
    ///////////////////////////////////////////////////////////////////////////////////////
    //
    // Data properties
    //
    ///////////////////////////////////////////////////////////////////////////////////////
     -->

    


    <!-- http://hit2gap.eu/h2g/h2gBI#floorLevel -->

    <owl:DatatypeProperty rdf:about="http://hit2gap.eu/h2g/h2gBI#floorLevel">
        <rdfs:range rdf:resource="http://www.w3.org/2001/XMLSchema#integer"/>
        <rdfs:label xml:lang="en">floorLevel</rdfs:label>
    </owl:DatatypeProperty>
    


    <!-- http://hit2gap.eu/h2g/h2gBI#hasPartitioningType -->

    <owl:DatatypeProperty rdf:about="http://hit2gap.eu/h2g/h2gBI#hasPartitioningType"/>
    


    <!-- http://hit2gap.eu/h2g/h2gBI#hasWindowType -->

    <owl:DatatypeProperty rdf:about="http://hit2gap.eu/h2g/h2gBI#hasWindowType">
        <rdfs:range rdf:resource="http://www.buildingsmart-tech.org/ifcOWL/IFC2X3_Final#IfcWindowTypeEnum"/>
    </owl:DatatypeProperty>
    


    <!-- http://hit2gap.eu/h2g/h2gBI#isInside -->

    <owl:DatatypeProperty rdf:about="http://hit2gap.eu/h2g/h2gBI#isInside">
        <rdfs:range rdf:resource="http://www.w3.org/2001/XMLSchema#boolean"/>
    </owl:DatatypeProperty>
    


    <!-- http://hit2gap.eu/h2g/h2gBI#propertyValue -->

    <owl:DatatypeProperty rdf:about="http://hit2gap.eu/h2g/h2gBI#propertyValue">
        <rdfs:range rdf:resource="http://www.w3.org/2001/XMLSchema#double"/>
        <rdfs:label xml:lang="en">Property Value</rdfs:label>
    </owl:DatatypeProperty>
    


    <!-- http://hit2gap.eu/h2g/h2gBI#windowWallRatio -->

    <owl:DatatypeProperty rdf:about="http://hit2gap.eu/h2g/h2gBI#windowWallRatio">
        <rdfs:range rdf:resource="http://www.w3.org/2001/XMLSchema#float"/>
        <rdfs:label rdf:datatype="http://www.w3.org/2001/XMLSchema#string">Window Wall Ratio</rdfs:label>
    </owl:DatatypeProperty>
    


    <!-- http://hit2gap.eu/h2g/h2gSensor#externalID -->

    <owl:DatatypeProperty rdf:about="http://hit2gap.eu/h2g/h2gSensor#externalID">
        <rdfs:range rdf:resource="http://www.w3.org/2001/XMLSchema#anyURI"/>
        <rdfs:comment xml:lang="en">Data proeprty to define the external ID regaring the time series stored in Mondas.</rdfs:comment>
        <rdfs:isDefinedBy xml:lang="en">http://hit2gap.eu/h2g/h2gSensor#externalID</rdfs:isDefinedBy>
        <rdfs:label xml:lang="en">externalID</rdfs:label>
    </owl:DatatypeProperty>
    


    <!-- http://webprotege.stanford.edu/RbUxaH9qGAEuKzaa2RttSc -->

    <owl:DatatypeProperty rdf:about="http://webprotege.stanford.edu/RbUxaH9qGAEuKzaa2RttSc">
        <rdfs:label>associatedQuantity</rdfs:label>
    </owl:DatatypeProperty>
    


    <!-- http://www.w3.org/2006/time#inXSDDateTime -->

    <owl:DatatypeProperty rdf:about="http://www.w3.org/2006/time#inXSDDateTime">
        <rdfs:isDefinedBy xml:lang="en">http://www.w3.org/2006/time#inXSDDateTime</rdfs:isDefinedBy>
    </owl:DatatypeProperty>
    


    <!-- 
    ///////////////////////////////////////////////////////////////////////////////////////
    //
    // Classes
    //
    ///////////////////////////////////////////////////////////////////////////////////////
     -->

    


    <!-- http://hit2gap.eu/h2g/h2gBA#BuildingAppliance -->

    <owl:Class rdf:about="http://hit2gap.eu/h2g/h2gBA#BuildingAppliance">
        <rdfs:subClassOf rdf:resource="http://hit2gap.eu/h2g/h2gSensor#FeatureOfInterest"/>
        <rdfs:subClassOf>
            <owl:Restriction>
                <owl:onProperty rdf:resource="http://hit2gap.eu/h2g/h2gBI#contains"/>
                <owl:someValuesFrom rdf:resource="http://hit2gap.eu/h2g/h2gBA#BuildingAppliance"/>
            </owl:Restriction>
        </rdfs:subClassOf>
        <rdfs:comment xml:lang="en">Building Appliances represent the static and mobile appliances inside the building. Several devices and IFC specific devices has been categorised and included.</rdfs:comment>
        <rdfs:isDefinedBy xml:lang="en">http://hit2gap.eu/h2g/h2gBA#BuildingAppliance</rdfs:isDefinedBy>
        <rdfs:label xml:lang="en">BuildingAppliance</rdfs:label>
    </owl:Class>
    


    <!-- http://hit2gap.eu/h2g/h2gBA#Meter -->

    <owl:Class rdf:about="http://hit2gap.eu/h2g/h2gBA#Meter">
        <rdfs:subClassOf rdf:resource="http://hit2gap.eu/h2g/h2gBA#Monitoring"/>
        <rdfs:comment xml:lang="en">A Meter is a device which measures the integral, with respect to time, of the power in an electric circuit.</rdfs:comment>
        <rdfs:isDefinedBy xml:lang="en">http://hit2gap.eu/h2g/h2gBA#Meter</rdfs:isDefinedBy>
        <rdfs:label xml:lang="en">Meter</rdfs:label>
    </owl:Class>
    


    <!-- http://hit2gap.eu/h2g/h2gBA#MobileBuildingAppliance -->

    <owl:Class rdf:about="http://hit2gap.eu/h2g/h2gBA#MobileBuildingAppliance">
        <rdfs:subClassOf rdf:resource="http://hit2gap.eu/h2g/h2gBA#BuildingAppliance"/>
        <rdfs:subClassOf>
            <owl:Restriction>
                <owl:onProperty rdf:resource="http://hit2gap.eu/h2g/h2gBI#wasLocated"/>
                <owl:allValuesFrom rdf:resource="http://hit2gap.eu/h2g/h2gSensor#MobileBuildingApplianceLocationObservation"/>
            </owl:Restriction>
        </rdfs:subClassOf>
        <rdfs:comment xml:lang="en">Mobile Building Appliances represent  mobile appliances inside the building.</rdfs:comment>
        <rdfs:isDefinedBy xml:lang="en">http://hit2gap.eu/h2g/h2gBA#MobileBuildingAppliance</rdfs:isDefinedBy>
        <rdfs:label xml:lang="en">MobileBuildingAppliance</rdfs:label>
    </owl:Class>
    


    <!-- http://hit2gap.eu/h2g/h2gBA#Monitoring -->

    <owl:Class rdf:about="http://hit2gap.eu/h2g/h2gBA#Monitoring">
        <rdfs:subClassOf rdf:resource="http://hit2gap.eu/h2g/h2gBA#StaticBuildingAppliance"/>
        <rdfs:subClassOf>
            <owl:Restriction>
                <owl:onProperty rdf:resource="http://hit2gap.eu/h2g/h2gBI#MeasureInputOutput"/>
                <owl:someValuesFrom rdf:resource="http://hit2gap.eu/h2g/h2gBA#BuildingAppliance"/>
            </owl:Restriction>
        </rdfs:subClassOf>
        <rdfs:comment xml:lang="en">Monitoring is a static building appliance for monitoring and controlling the building, occupants’ devices, etc.</rdfs:comment>
        <rdfs:isDefinedBy xml:lang="en">http://hit2gap.eu/h2g/h2gBA#Monitoring</rdfs:isDefinedBy>
        <rdfs:label xml:lang="en">Monitoring</rdfs:label>
    </owl:Class>
    


    <!-- http://hit2gap.eu/h2g/h2gBA#StaticBuildingAppliance -->

    <owl:Class rdf:about="http://hit2gap.eu/h2g/h2gBA#StaticBuildingAppliance">
        <rdfs:subClassOf rdf:resource="http://hit2gap.eu/h2g/h2gBA#BuildingAppliance"/>
        <rdfs:subClassOf>
            <owl:Restriction>
                <owl:onProperty rdf:resource="http://hit2gap.eu/h2g/h2gBI#isLocatedIn"/>
                <owl:allValuesFrom rdf:resource="http://www.buildingsmart-tech.org/ifcOWL/IFC2X3_Final#IfcZone"/>
            </owl:Restriction>
        </rdfs:subClassOf>
        <rdfs:comment xml:lang="en">Static Building Appliances represent static appliances inside the building. Several devices and IFC specific devices has been categorised and included.</rdfs:comment>
        <rdfs:isDefinedBy xml:lang="en">http://hit2gap.eu/h2g/h2gBA#StaticBuildingAppliance</rdfs:isDefinedBy>
        <rdfs:label xml:lang="en">StaticBuildingAppliance</rdfs:label>
    </owl:Class>
    


    <!-- http://hit2gap.eu/h2g/h2gBA#Wearable -->

    <owl:Class rdf:about="http://hit2gap.eu/h2g/h2gBA#Wearable">
        <rdfs:subClassOf rdf:resource="http://hit2gap.eu/h2g/h2gBA#MobileBuildingAppliance"/>
        <rdfs:comment xml:lang="en">Wearable is a building appliance representing a wereable device such as smartwatches and smartphones.</rdfs:comment>
        <rdfs:isDefinedBy xml:lang="en">http://hit2gap.eu/h2g/h2gBA#Wearable</rdfs:isDefinedBy>
        <rdfs:label xml:lang="en">Wearable</rdfs:label>
    </owl:Class>
    


    <!-- http://hit2gap.eu/h2g/h2gBI#Administration -->

    <owl:Class rdf:about="http://hit2gap.eu/h2g/h2gBI#Administration">
        <rdfs:subClassOf rdf:resource="http://hit2gap.eu/h2g/h2gBI#PublicBuilding"/>
        <rdfs:label>Administration</rdfs:label>
    </owl:Class>
    


    <!-- http://hit2gap.eu/h2g/h2gBI#AgriculturalBuilding -->

    <owl:Class rdf:about="http://hit2gap.eu/h2g/h2gBI#AgriculturalBuilding">
        <rdfs:subClassOf rdf:resource="http://www.buildingsmart-tech.org/ifcOWL/IFC2X3_Final#IfcBuilding"/>
        <rdfs:label>AgriculturalBuilding</rdfs:label>
    </owl:Class>
    


    <!-- http://hit2gap.eu/h2g/h2gBI#Air -->

    <owl:Class rdf:about="http://hit2gap.eu/h2g/h2gBI#Air">
        <rdfs:subClassOf rdf:resource="http://hit2gap.eu/h2g/h2gBI#PhysicalMedium"/>
        <rdfs:comment xml:lang="en">Air represents air as a physical medium to produce energy.</rdfs:comment>
        <rdfs:label xml:lang="en">Air</rdfs:label>
    </owl:Class>
    


    <!-- http://hit2gap.eu/h2g/h2gBI#AirHandlingUnit -->

    <owl:Class rdf:about="http://hit2gap.eu/h2g/h2gBI#AirHandlingUnit">
        <rdfs:subClassOf rdf:resource="http://www.buildingsmart-tech.org/ifcOWL/IFC2X3_Final#IfcEnergyConversionDevice"/>
        <rdfs:comment xml:lang="en">An AirHandlingUnit is a device used to regulate and circulate air as part of a heating, ventilating, and air-conditioning (HVAC) system.</rdfs:comment>
        <rdfs:label xml:lang="en">AirHandlingUnit</rdfs:label>
    </owl:Class>
    


    <!-- http://hit2gap.eu/h2g/h2gBI#Airport -->

    <owl:Class rdf:about="http://hit2gap.eu/h2g/h2gBI#Airport">
        <rdfs:subClassOf rdf:resource="http://hit2gap.eu/h2g/h2gBI#TransportBuilding"/>
        <rdfs:label>Airport</rdfs:label>
    </owl:Class>
    


    <!-- http://hit2gap.eu/h2g/h2gBI#Amplifier -->

    <owl:Class rdf:about="http://hit2gap.eu/h2g/h2gBI#Amplifier">
        <rdfs:subClassOf rdf:resource="http://ifcowl.openbimstandards.org/IFC4_ADD2/index.html#IfcAudioVisualAppliance"/>
    </owl:Class>
    


    <!-- http://hit2gap.eu/h2g/h2gBI#Antenna -->

    <owl:Class rdf:about="http://hit2gap.eu/h2g/h2gBI#Antenna">
        <rdfs:subClassOf rdf:resource="http://ifcowl.openbimstandards.org/IFC4_ADD2/index.html#IfcCommunicationAppliance"/>
    </owl:Class>
    


    <!-- http://hit2gap.eu/h2g/h2gBI#Apartment -->

    <owl:Class rdf:about="http://hit2gap.eu/h2g/h2gBI#Apartment">
        <rdfs:subClassOf rdf:resource="http://hit2gap.eu/h2g/h2gBI#ResidentialBuilding"/>
        <rdfs:label rdf:datatype="http://www.w3.org/2001/XMLSchema#string">Apartment</rdfs:label>
    </owl:Class>
    


    <!-- http://hit2gap.eu/h2g/h2gBI#Arid -->

    <owl:Class rdf:about="http://hit2gap.eu/h2g/h2gBI#Arid">
        <rdfs:subClassOf rdf:resource="http://hit2gap.eu/h2g/h2gBI#Climate"/>
        <rdfs:comment xml:lang="en">Arid represents an observation of the arid climate in a specific time.</rdfs:comment>
        <rdfs:label xml:lang="en">Arid</rdfs:label>
    </owl:Class>
    


    <!-- http://hit2gap.eu/h2g/h2gBI#AutomobileRepair -->

    <owl:Class rdf:about="http://hit2gap.eu/h2g/h2gBI#AutomobileRepair">
        <rdfs:subClassOf rdf:resource="http://hit2gap.eu/h2g/h2gBI#CommercialBuilding"/>
        <rdfs:label>AutomobileRepair</rdfs:label>
    </owl:Class>
    


    <!-- http://hit2gap.eu/h2g/h2gBI#Balcony -->

    <owl:Class rdf:about="http://hit2gap.eu/h2g/h2gBI#Balcony">
        <rdfs:subClassOf rdf:resource="http://www.buildingsmart-tech.org/ifcOWL/IFC2X3_Final#IfcSpace"/>
        <rdfs:comment xml:lang="en">Balcony is an instance of IfcSpace in the building representing a balcony.</rdfs:comment>
        <rdfs:label xml:lang="en">Balcony</rdfs:label>
    </owl:Class>
    


    <!-- http://hit2gap.eu/h2g/h2gBI#BarRestaurant -->

    <owl:Class rdf:about="http://hit2gap.eu/h2g/h2gBI#BarRestaurant">
        <rdfs:subClassOf rdf:resource="http://hit2gap.eu/h2g/h2gBI#CommercialBuilding"/>
        <rdfs:label>BarRestaurant</rdfs:label>
    </owl:Class>
    


    <!-- http://hit2gap.eu/h2g/h2gBI#Barn -->

    <owl:Class rdf:about="http://hit2gap.eu/h2g/h2gBI#Barn">
        <rdfs:subClassOf rdf:resource="http://hit2gap.eu/h2g/h2gBI#AgriculturalBuilding"/>
        <rdfs:label>Barn</rdfs:label>
    </owl:Class>
    


    <!-- http://hit2gap.eu/h2g/h2gBI#Bathroom -->

    <owl:Class rdf:about="http://hit2gap.eu/h2g/h2gBI#Bathroom">
        <rdfs:subClassOf rdf:resource="http://www.buildingsmart-tech.org/ifcOWL/IFC2X3_Final#IfcSpace"/>
        <rdfs:comment xml:lang="en">Bathroom is an instance of IfcSpace in the building representing a bathroom.</rdfs:comment>
        <rdfs:label xml:lang="en">Bathroom</rdfs:label>
    </owl:Class>
    


    <!-- http://hit2gap.eu/h2g/h2gBI#Blind -->

    <owl:Class rdf:about="http://hit2gap.eu/h2g/h2gBI#Blind">
        <rdfs:subClassOf rdf:resource="http://hit2gap.eu/h2g/h2gBI#WindowCovering"/>
        <rdfs:comment xml:lang="en">A Blind is a type of a WindowCovering representing a window blind.</rdfs:comment>
        <rdfs:label xml:lang="en">Blind</rdfs:label>
    </owl:Class>
    


    <!-- http://hit2gap.eu/h2g/h2gBI#Boiler -->

    <owl:Class rdf:about="http://hit2gap.eu/h2g/h2gBI#Boiler">
        <rdfs:subClassOf rdf:resource="http://ifcowl.openbimstandards.org/IFC4_ADD2/index.html#IfcElectricAppliance"/>
    </owl:Class>
    


    <!-- http://hit2gap.eu/h2g/h2gBI#Bridge -->

    <owl:Class rdf:about="http://hit2gap.eu/h2g/h2gBI#Bridge">
        <rdfs:subClassOf rdf:resource="http://hit2gap.eu/h2g/h2gBI#NetworkAppliance"/>
    </owl:Class>
    


    <!-- http://hit2gap.eu/h2g/h2gBI#Bungalow -->

    <owl:Class rdf:about="http://hit2gap.eu/h2g/h2gBI#Bungalow">
        <rdfs:subClassOf rdf:resource="http://hit2gap.eu/h2g/h2gBI#ResidentialBuilding"/>
        <rdfs:label rdf:datatype="http://www.w3.org/2001/XMLSchema#string">Bungalow</rdfs:label>
    </owl:Class>
    


    <!-- http://hit2gap.eu/h2g/h2gBI#BusStation -->

    <owl:Class rdf:about="http://hit2gap.eu/h2g/h2gBI#BusStation">
        <rdfs:subClassOf rdf:resource="http://hit2gap.eu/h2g/h2gBI#TransportBuilding"/>
        <rdfs:label>BusStation</rdfs:label>
    </owl:Class>
    


    <!-- http://hit2gap.eu/h2g/h2gBI#Cafeteria -->

    <owl:Class rdf:about="http://hit2gap.eu/h2g/h2gBI#Cafeteria">
        <rdfs:subClassOf rdf:resource="http://www.buildingsmart-tech.org/ifcOWL/IFC2X3_Final#IfcSpace"/>
        <rdfs:comment xml:lang="en">Cafeteria is an instance of IfcSpace in the building representing a cafeteria.</rdfs:comment>
        <rdfs:label xml:lang="en">Cafeteria</rdfs:label>
    </owl:Class>
    


    <!-- http://hit2gap.eu/h2g/h2gBI#Camera -->

    <owl:Class rdf:about="http://hit2gap.eu/h2g/h2gBI#Camera">
        <rdfs:subClassOf rdf:resource="http://ifcowl.openbimstandards.org/IFC4_ADD2/index.html#IfcAudioVisualAppliance"/>
    </owl:Class>
    


    <!-- http://hit2gap.eu/h2g/h2gBI#Canteen -->

    <owl:Class rdf:about="http://hit2gap.eu/h2g/h2gBI#Canteen">
        <rdfs:subClassOf rdf:resource="http://www.buildingsmart-tech.org/ifcOWL/IFC2X3_Final#IfcSpace"/>
        <rdfs:comment xml:lang="en">Canteen is an instance of IfcSpace in the building representing a canteen.</rdfs:comment>
        <rdfs:label xml:lang="en">Canteen</rdfs:label>
    </owl:Class>
    


    <!-- http://hit2gap.eu/h2g/h2gBI#Cellar -->

    <owl:Class rdf:about="http://hit2gap.eu/h2g/h2gBI#Cellar">
        <rdfs:subClassOf rdf:resource="http://hit2gap.eu/h2g/h2gBI#AgriculturalBuilding"/>
        <rdfs:label>Cellar</rdfs:label>
    </owl:Class>
    


    <!-- http://hit2gap.eu/h2g/h2gBI#ChilledBeams -->

    <owl:Class rdf:about="http://hit2gap.eu/h2g/h2gBI#ChilledBeams">
        <rdfs:subClassOf rdf:resource="http://www.buildingsmart-tech.org/ifcOWL/IFC2X3_Final#IfcEnergyConversionDevice"/>
        <rdfs:comment xml:lang="en">A ChilledBeam is a type of convection HVAC system designed to heat or cool large buildings. Pipes of water are passed through a &quot;beam&quot; (a heat exchanger) either integrated into standard suspended ceiling systems or suspended a short distance from the ceiling of a room.</rdfs:comment>
        <rdfs:label xml:lang="en">ChilledBeams</rdfs:label>
    </owl:Class>
    


    <!-- http://hit2gap.eu/h2g/h2gBI#Cinema -->

    <owl:Class rdf:about="http://hit2gap.eu/h2g/h2gBI#Cinema">
        <rdfs:subClassOf rdf:resource="http://hit2gap.eu/h2g/h2gBI#PublicBuilding"/>
        <rdfs:label>Cinema</rdfs:label>
    </owl:Class>
    


    <!-- http://hit2gap.eu/h2g/h2gBI#CirculationArea -->

    <owl:Class rdf:about="http://hit2gap.eu/h2g/h2gBI#CirculationArea">
        <rdfs:subClassOf rdf:resource="http://www.buildingsmart-tech.org/ifcOWL/IFC2X3_Final#IfcSpace"/>
        <rdfs:comment xml:lang="en">CirculationArea is an instance of IfcSpace in the building representing a circulation area.</rdfs:comment>
        <rdfs:label xml:lang="en">CirculationArea</rdfs:label>
    </owl:Class>
    


    <!-- http://hit2gap.eu/h2g/h2gBI#Climate -->

    <owl:Class rdf:about="http://hit2gap.eu/h2g/h2gBI#Climate">
        <rdfs:comment xml:lang="en">Climate represents an observation of the climate  in a specific time.</rdfs:comment>
        <rdfs:label xml:lang="en">Climate</rdfs:label>
    </owl:Class>
    


    <!-- http://hit2gap.eu/h2g/h2gBI#CoffeeMachine -->

    <owl:Class rdf:about="http://hit2gap.eu/h2g/h2gBI#CoffeeMachine">
        <rdfs:subClassOf rdf:resource="http://ifcowl.openbimstandards.org/IFC4_ADD2/index.html#IfcElectricAppliance"/>
    </owl:Class>
    


    <!-- http://hit2gap.eu/h2g/h2gBI#CommercialBuilding -->

    <owl:Class rdf:about="http://hit2gap.eu/h2g/h2gBI#CommercialBuilding">
        <rdfs:subClassOf rdf:resource="http://www.buildingsmart-tech.org/ifcOWL/IFC2X3_Final#IfcBuilding"/>
        <rdfs:label>CommercialBuilding</rdfs:label>
    </owl:Class>
    


    <!-- http://hit2gap.eu/h2g/h2gBI#Computer -->

    <owl:Class rdf:about="http://hit2gap.eu/h2g/h2gBI#Computer">
        <rdfs:subClassOf rdf:resource="http://ifcowl.openbimstandards.org/IFC4_ADD2/index.html#IfcCommunicationAppliance"/>
    </owl:Class>
    


    <!-- http://hit2gap.eu/h2g/h2gBI#ConferenceRoom -->

    <owl:Class rdf:about="http://hit2gap.eu/h2g/h2gBI#ConferenceRoom">
        <rdfs:subClassOf rdf:resource="http://www.buildingsmart-tech.org/ifcOWL/IFC2X3_Final#IfcSpace"/>
        <rdfs:comment xml:lang="en">ConferenceRoom is an instance of IfcSpace in the building representing a conference room.</rdfs:comment>
        <rdfs:label xml:lang="en">ConferenceRoom</rdfs:label>
    </owl:Class>
    


    <!-- http://hit2gap.eu/h2g/h2gBI#Continental -->

    <owl:Class rdf:about="http://hit2gap.eu/h2g/h2gBI#Continental">
        <rdfs:subClassOf rdf:resource="http://hit2gap.eu/h2g/h2gBI#Climate"/>
        <rdfs:comment xml:lang="en">Continental represents an observation of the continental climate in a specific time.</rdfs:comment>
        <rdfs:label xml:lang="en">Continental</rdfs:label>
    </owl:Class>
    


    <!-- http://hit2gap.eu/h2g/h2gBI#ConventionCenter -->

    <owl:Class rdf:about="http://hit2gap.eu/h2g/h2gBI#ConventionCenter">
        <rdfs:subClassOf rdf:resource="http://hit2gap.eu/h2g/h2gBI#CommercialBuilding"/>
        <rdfs:label>ConventionCenter</rdfs:label>
    </owl:Class>
    


    <!-- http://hit2gap.eu/h2g/h2gBI#Cooker -->

    <owl:Class rdf:about="http://hit2gap.eu/h2g/h2gBI#Cooker">
        <rdfs:subClassOf rdf:resource="http://ifcowl.openbimstandards.org/IFC4_ADD2/index.html#IfcElectricAppliance"/>
    </owl:Class>
    


    <!-- http://hit2gap.eu/h2g/h2gBI#Curtain -->

    <owl:Class rdf:about="http://hit2gap.eu/h2g/h2gBI#Curtain">
        <rdfs:subClassOf rdf:resource="http://hit2gap.eu/h2g/h2gBI#WindowCovering"/>
        <rdfs:comment xml:lang="en">A Curtain is a type of a WindowCovering representing a window curtain.</rdfs:comment>
        <rdfs:label xml:lang="en">Curtain</rdfs:label>
    </owl:Class>
    


    <!-- http://hit2gap.eu/h2g/h2gBI#DataCenter -->

    <owl:Class rdf:about="http://hit2gap.eu/h2g/h2gBI#DataCenter">
        <rdfs:subClassOf rdf:resource="http://hit2gap.eu/h2g/h2gBI#IndustrialBuilding"/>
        <rdfs:label>DataCenter</rdfs:label>
    </owl:Class>
    


    <!-- http://hit2gap.eu/h2g/h2gBI#Desk -->

    <owl:Class rdf:about="http://hit2gap.eu/h2g/h2gBI#Desk">
        <rdfs:subClassOf rdf:resource="http://www.buildingsmart-tech.org/ifcOWL/IFC2X3_Final#IfcSpace"/>
        <rdfs:comment xml:lang="en">Desk is an instance of IfcSpace in the building representing a desk.</rdfs:comment>
        <rdfs:label xml:lang="en">Desk</rdfs:label>
    </owl:Class>
    


    <!-- http://hit2gap.eu/h2g/h2gBI#Dishwasher -->

    <owl:Class rdf:about="http://hit2gap.eu/h2g/h2gBI#Dishwasher">
        <rdfs:subClassOf rdf:resource="http://ifcowl.openbimstandards.org/IFC4_ADD2/index.html#IfcElectricAppliance"/>
    </owl:Class>
    


    <!-- http://hit2gap.eu/h2g/h2gBI#DoubleGlazing -->

    <owl:Class rdf:about="http://hit2gap.eu/h2g/h2gBI#DoubleGlazing">
        <rdfs:subClassOf rdf:resource="http://hit2gap.eu/h2g/h2gBI#WindowGlazing"/>
        <rdfs:comment xml:lang="en">It represents that glasses of the window are double</rdfs:comment>
        <rdfs:label xml:lang="en">Double Glazing</rdfs:label>
    </owl:Class>
    


    <!-- http://hit2gap.eu/h2g/h2gBI#DrugStore -->

    <owl:Class rdf:about="http://hit2gap.eu/h2g/h2gBI#DrugStore">
        <rdfs:subClassOf rdf:resource="http://hit2gap.eu/h2g/h2gBI#CommercialBuilding"/>
        <rdfs:label>DrugStore</rdfs:label>
    </owl:Class>
    


    <!-- http://hit2gap.eu/h2g/h2gBI#EducationalBuilding -->

    <owl:Class rdf:about="http://hit2gap.eu/h2g/h2gBI#EducationalBuilding">
        <rdfs:subClassOf rdf:resource="http://www.buildingsmart-tech.org/ifcOWL/IFC2X3_Final#IfcBuilding"/>
        <rdfs:label rdf:datatype="http://www.w3.org/2001/XMLSchema#string">Educational Building</rdfs:label>
    </owl:Class>
    


    <!-- http://hit2gap.eu/h2g/h2gBI#ElectricHeater -->

    <owl:Class rdf:about="http://hit2gap.eu/h2g/h2gBI#ElectricHeater">
        <rdfs:subClassOf rdf:resource="http://www.buildingsmart-tech.org/ifcOWL/IFC2X3_Final#IfcFlowTerminal"/>
        <rdfs:comment xml:lang="en">An ElectricHeater represents an electrical device that converts electric current to heat.</rdfs:comment>
        <rdfs:label xml:lang="en">ElectricHeater</rdfs:label>
    </owl:Class>
    


    <!-- http://hit2gap.eu/h2g/h2gBI#FS_Electric_Heater -->

    <owl:Class rdf:about="http://hit2gap.eu/h2g/h2gBI#FS_Electric_Heater">
        <rdfs:subClassOf rdf:resource="http://ifcowl.openbimstandards.org/IFC4_ADD2/index.html#IfcElectricAppliance"/>
    </owl:Class>
    


    <!-- http://hit2gap.eu/h2g/h2gBI#FS_Fan -->

    <owl:Class rdf:about="http://hit2gap.eu/h2g/h2gBI#FS_Fan">
        <rdfs:subClassOf rdf:resource="http://ifcowl.openbimstandards.org/IFC4_ADD2/index.html#IfcElectricAppliance"/>
    </owl:Class>
    


    <!-- http://hit2gap.eu/h2g/h2gBI#FS_Water_Cooler -->

    <owl:Class rdf:about="http://hit2gap.eu/h2g/h2gBI#FS_Water_Cooler">
        <rdfs:subClassOf rdf:resource="http://ifcowl.openbimstandards.org/IFC4_ADD2/index.html#IfcElectricAppliance"/>
    </owl:Class>
    


    <!-- http://hit2gap.eu/h2g/h2gBI#FS_Water_Heater -->

    <owl:Class rdf:about="http://hit2gap.eu/h2g/h2gBI#FS_Water_Heater">
        <rdfs:subClassOf rdf:resource="http://ifcowl.openbimstandards.org/IFC4_ADD2/index.html#IfcElectricAppliance"/>
    </owl:Class>
    


    <!-- http://hit2gap.eu/h2g/h2gBI#Factory -->

    <owl:Class rdf:about="http://hit2gap.eu/h2g/h2gBI#Factory">
        <rdfs:subClassOf rdf:resource="http://hit2gap.eu/h2g/h2gBI#IndustrialBuilding"/>
        <rdfs:label>Factory</rdfs:label>
    </owl:Class>
    


    <!-- http://hit2gap.eu/h2g/h2gBI#FanCoilUnit -->

    <owl:Class rdf:about="http://hit2gap.eu/h2g/h2gBI#FanCoilUnit">
        <rdfs:subClassOf rdf:resource="http://ifcowl.openbimstandards.org/IFC4_ADD2/index.html#IfcFan"/>
        <rdfs:subClassOf rdf:resource="http://www.buildingsmart-tech.org/ifcOWL/IFC2X3_Final#IfcFanType"/>
        <rdfs:comment xml:lang="en">A FanCoilUnit is a simple device consisting of a heating or cooling heat exchanger or &apos;coil&apos; and fan. It is part of an HVAC system found in residential, commercial, and industrial buildings. A fan coil unit is a diverse device sometimes using ductwork, and is used to control the temperature in the space where it is installed, or serve multiple spaces. It is controlled either by a manual on/off switch or by a thermostat, which controls the throughput of water to the heat exchanger using a control valve and/or the fan speed.</rdfs:comment>
        <rdfs:label xml:lang="en">FanCoilUnit</rdfs:label>
    </owl:Class>
    


    <!-- http://hit2gap.eu/h2g/h2gBI#Farmhouse -->

    <owl:Class rdf:about="http://hit2gap.eu/h2g/h2gBI#Farmhouse">
        <rdfs:subClassOf rdf:resource="http://hit2gap.eu/h2g/h2gBI#AgriculturalBuilding"/>
        <rdfs:label>Farmhouse</rdfs:label>
    </owl:Class>
    


    <!-- http://hit2gap.eu/h2g/h2gBI#Fax -->

    <owl:Class rdf:about="http://hit2gap.eu/h2g/h2gBI#Fax">
        <rdfs:subClassOf rdf:resource="http://ifcowl.openbimstandards.org/IFC4_ADD2/index.html#IfcCommunicationAppliance"/>
    </owl:Class>
    


    <!-- http://hit2gap.eu/h2g/h2gBI#Floor -->

    <owl:Class rdf:about="http://hit2gap.eu/h2g/h2gBI#Floor">
        <rdfs:subClassOf rdf:resource="http://www.buildingsmart-tech.org/ifcOWL/IFC2X3_Final#IfcBuildingStorey"/>
        <rdfs:subClassOf>
            <owl:Restriction>
                <owl:onProperty rdf:resource="http://www.w3.org/ns/ssn/hasProperty"/>
                <owl:someValuesFrom rdf:resource="http://hit2gap.eu/h2g/h2gProperty#PhenomenonProperty"/>
            </owl:Restriction>
        </rdfs:subClassOf>
        <rdfs:subClassOf>
            <owl:Restriction>
                <owl:onProperty rdf:resource="http://hit2gap.eu/h2g/h2gBI#floorLevel"/>
                <owl:allValuesFrom rdf:resource="http://www.w3.org/2001/XMLSchema#integer"/>
            </owl:Restriction>
        </rdfs:subClassOf>
        <rdfs:comment xml:lang="en">A Floor is an instance of a story in the building.</rdfs:comment>
        <rdfs:label xml:lang="en">Floor</rdfs:label>
    </owl:Class>
    


    <!-- http://hit2gap.eu/h2g/h2gBI#Freezer -->

    <owl:Class rdf:about="http://hit2gap.eu/h2g/h2gBI#Freezer">
        <rdfs:subClassOf rdf:resource="http://ifcowl.openbimstandards.org/IFC4_ADD2/index.html#IfcElectricAppliance"/>
    </owl:Class>
    


    <!-- http://hit2gap.eu/h2g/h2gBI#Fridge -->

    <owl:Class rdf:about="http://hit2gap.eu/h2g/h2gBI#Fridge">
        <rdfs:subClassOf rdf:resource="http://ifcowl.openbimstandards.org/IFC4_ADD2/index.html#IfcElectricAppliance"/>
    </owl:Class>
    


    <!-- http://hit2gap.eu/h2g/h2gBI#Gas -->

    <owl:Class rdf:about="http://hit2gap.eu/h2g/h2gBI#Gas">
        <rdfs:subClassOf rdf:resource="http://hit2gap.eu/h2g/h2gBI#PhysicalMedium"/>
        <rdfs:comment xml:lang="en">Gas represents gas as a physical medium to produce energy.</rdfs:comment>
        <rdfs:label xml:lang="en">Gas</rdfs:label>
    </owl:Class>
    


    <!-- http://hit2gap.eu/h2g/h2gBI#Gateway -->

    <owl:Class rdf:about="http://hit2gap.eu/h2g/h2gBI#Gateway">
        <rdfs:subClassOf rdf:resource="http://ifcowl.openbimstandards.org/IFC4_ADD2/index.html#IfcCommunicationAppliance"/>
    </owl:Class>
    


    <!-- http://hit2gap.eu/h2g/h2gBI#Greenhouse -->

    <owl:Class rdf:about="http://hit2gap.eu/h2g/h2gBI#Greenhouse">
        <rdfs:subClassOf rdf:resource="http://hit2gap.eu/h2g/h2gBI#AgriculturalBuilding"/>
        <rdfs:label>Greenhouse</rdfs:label>
    </owl:Class>
    


    <!-- http://hit2gap.eu/h2g/h2gBI#Ground -->

    <owl:Class rdf:about="http://hit2gap.eu/h2g/h2gBI#Ground">
        <rdfs:subClassOf rdf:resource="http://hit2gap.eu/h2g/h2gBI#Floor"/>
        <rdfs:comment xml:lang="en">A Ground represents a ground floor.</rdfs:comment>
        <rdfs:label xml:lang="en">Ground</rdfs:label>
    </owl:Class>
    


    <!-- http://hit2gap.eu/h2g/h2gBI#Gym -->

    <owl:Class rdf:about="http://hit2gap.eu/h2g/h2gBI#Gym">
        <rdfs:subClassOf rdf:resource="http://hit2gap.eu/h2g/h2gBI#PublicBuilding"/>
        <rdfs:label>Gym</rdfs:label>
    </owl:Class>
    


    <!-- http://hit2gap.eu/h2g/h2gBI#Hand_Dryer -->

    <owl:Class rdf:about="http://hit2gap.eu/h2g/h2gBI#Hand_Dryer">
        <rdfs:subClassOf rdf:resource="http://ifcowl.openbimstandards.org/IFC4_ADD2/index.html#IfcElectricAppliance"/>
    </owl:Class>
    


    <!-- http://hit2gap.eu/h2g/h2gBI#HeatPump -->

    <owl:Class rdf:about="http://hit2gap.eu/h2g/h2gBI#HeatPump">
        <rdfs:subClassOf rdf:resource="http://ifcowl.openbimstandards.org/IFC4_ADD2/index.html#IfcPump"/>
        <rdfs:subClassOf rdf:resource="http://www.buildingsmart-tech.org/ifcOWL/IFC2X3_Final#IfcPumpType"/>
        <rdfs:comment xml:lang="en">A HeatPump is a device that transfers heat energy from a source of heat to a destination called a &quot;heat sink&quot;. Heat pumps are designed to move thermal energy in the opposite direction of spontaneous heat transfer by absorbing heat from a cold space and releasing it to a warmer one. A heat pump uses a small amount of external power to accomplish the work of transferring energy from the heat source to the heat sink.</rdfs:comment>
        <rdfs:label xml:lang="en">HeatPump</rdfs:label>
    </owl:Class>
    


    <!-- http://hit2gap.eu/h2g/h2gBI#Hospital -->

    <owl:Class rdf:about="http://hit2gap.eu/h2g/h2gBI#Hospital">
        <rdfs:subClassOf rdf:resource="http://hit2gap.eu/h2g/h2gBI#PublicBuilding"/>
        <rdfs:label>Hospital</rdfs:label>
    </owl:Class>
    


    <!-- http://hit2gap.eu/h2g/h2gBI#Hotel -->

    <owl:Class rdf:about="http://hit2gap.eu/h2g/h2gBI#Hotel">
        <rdfs:subClassOf rdf:resource="http://hit2gap.eu/h2g/h2gBI#CommercialBuilding"/>
        <rdfs:label>Hotel</rdfs:label>
    </owl:Class>
    


    <!-- http://hit2gap.eu/h2g/h2gBI#House -->

    <owl:Class rdf:about="http://hit2gap.eu/h2g/h2gBI#House">
        <rdfs:subClassOf rdf:resource="http://hit2gap.eu/h2g/h2gBI#ResidentialBuilding"/>
        <rdfs:label rdf:datatype="http://www.w3.org/2001/XMLSchema#string">House</rdfs:label>
    </owl:Class>
    


    <!-- http://hit2gap.eu/h2g/h2gBI#Hub -->

    <owl:Class rdf:about="http://hit2gap.eu/h2g/h2gBI#Hub">
        <rdfs:subClassOf rdf:resource="http://hit2gap.eu/h2g/h2gBI#NetworkAppliance"/>
    </owl:Class>
    


    <!-- http://hit2gap.eu/h2g/h2gBI#IndustrialBuilding -->

    <owl:Class rdf:about="http://hit2gap.eu/h2g/h2gBI#IndustrialBuilding">
        <rdfs:subClassOf rdf:resource="http://www.buildingsmart-tech.org/ifcOWL/IFC2X3_Final#IfcBuilding"/>
        <rdfs:label>IndustrialBuilding</rdfs:label>
    </owl:Class>
    


    <!-- http://hit2gap.eu/h2g/h2gBI#Kitchen -->

    <owl:Class rdf:about="http://hit2gap.eu/h2g/h2gBI#Kitchen">
        <rdfs:subClassOf rdf:resource="http://www.buildingsmart-tech.org/ifcOWL/IFC2X3_Final#IfcSpace"/>
        <rdfs:comment xml:lang="en">Kitchen is an instance of IfcSpace in the building representing a kitchen.</rdfs:comment>
        <rdfs:label xml:lang="en">Kitchen</rdfs:label>
    </owl:Class>
    


    <!-- http://hit2gap.eu/h2g/h2gBI#Kitchen_Device -->

    <owl:Class rdf:about="http://hit2gap.eu/h2g/h2gBI#Kitchen_Device">
        <rdfs:subClassOf rdf:resource="http://ifcowl.openbimstandards.org/IFC4_ADD2/index.html#IfcElectricAppliance"/>
    </owl:Class>
    


    <!-- http://hit2gap.eu/h2g/h2gBI#LampType -->

    <owl:Class rdf:about="http://hit2gap.eu/h2g/h2gBI#LampType">
        <rdfs:comment xml:lang="en">LampType determines the type of the lamp.</rdfs:comment>
        <rdfs:label xml:lang="en">LampType</rdfs:label>
    </owl:Class>
    


    <!-- http://hit2gap.eu/h2g/h2gBI#Library -->

    <owl:Class rdf:about="http://hit2gap.eu/h2g/h2gBI#Library">
        <rdfs:subClassOf rdf:resource="http://hit2gap.eu/h2g/h2gBI#PublicBuilding"/>
        <rdfs:label>Library</rdfs:label>
    </owl:Class>
    


    <!-- http://hit2gap.eu/h2g/h2gBI#LogisticPlatform -->

    <owl:Class rdf:about="http://hit2gap.eu/h2g/h2gBI#LogisticPlatform">
        <rdfs:subClassOf rdf:resource="http://hit2gap.eu/h2g/h2gBI#IndustrialBuilding"/>
        <rdfs:label>LogisticPlatform</rdfs:label>
    </owl:Class>
    


    <!-- http://hit2gap.eu/h2g/h2gBI#MallSupermarket -->

    <owl:Class rdf:about="http://hit2gap.eu/h2g/h2gBI#MallSupermarket">
        <rdfs:subClassOf rdf:resource="http://hit2gap.eu/h2g/h2gBI#CommercialBuilding"/>
        <rdfs:label>MallSupermarket</rdfs:label>
    </owl:Class>
    


    <!-- http://hit2gap.eu/h2g/h2gBI#MetroStation -->

    <owl:Class rdf:about="http://hit2gap.eu/h2g/h2gBI#MetroStation">
        <rdfs:subClassOf rdf:resource="http://hit2gap.eu/h2g/h2gBI#TransportBuilding"/>
        <rdfs:label>MetroStation</rdfs:label>
    </owl:Class>
    


    <!-- http://hit2gap.eu/h2g/h2gBI#Microphone -->

    <owl:Class rdf:about="http://hit2gap.eu/h2g/h2gBI#Microphone">
        <rdfs:subClassOf rdf:resource="http://ifcowl.openbimstandards.org/IFC4_ADD2/index.html#IfcAudioVisualAppliance"/>
    </owl:Class>
    


    <!-- http://hit2gap.eu/h2g/h2gBI#Microwave -->

    <owl:Class rdf:about="http://hit2gap.eu/h2g/h2gBI#Microwave">
        <rdfs:subClassOf rdf:resource="http://ifcowl.openbimstandards.org/IFC4_ADD2/index.html#IfcElectricAppliance"/>
    </owl:Class>
    


    <!-- http://hit2gap.eu/h2g/h2gBI#Modem -->

    <owl:Class rdf:about="http://hit2gap.eu/h2g/h2gBI#Modem">
        <rdfs:subClassOf rdf:resource="http://ifcowl.openbimstandards.org/IFC4_ADD2/index.html#IfcCommunicationAppliance"/>
    </owl:Class>
    


    <!-- http://hit2gap.eu/h2g/h2gBI#MuseumGallery -->

    <owl:Class rdf:about="http://hit2gap.eu/h2g/h2gBI#MuseumGallery">
        <rdfs:subClassOf rdf:resource="http://hit2gap.eu/h2g/h2gBI#PublicBuilding"/>
        <rdfs:label>MuseumGallery</rdfs:label>
    </owl:Class>
    


    <!-- http://hit2gap.eu/h2g/h2gBI#NetworkAppliance -->

    <owl:Class rdf:about="http://hit2gap.eu/h2g/h2gBI#NetworkAppliance">
        <rdfs:subClassOf rdf:resource="http://ifcowl.openbimstandards.org/IFC4_ADD2/index.html#IfcCommunicationAppliance"/>
    </owl:Class>
    


    <!-- http://hit2gap.eu/h2g/h2gBI#NightClubConcertHall -->

    <owl:Class rdf:about="http://hit2gap.eu/h2g/h2gBI#NightClubConcertHall">
        <rdfs:subClassOf rdf:resource="http://hit2gap.eu/h2g/h2gBI#PublicBuilding"/>
        <rdfs:label>NighClubConcertHall</rdfs:label>
    </owl:Class>
    


    <!-- http://hit2gap.eu/h2g/h2gBI#Nursery -->

    <owl:Class rdf:about="http://hit2gap.eu/h2g/h2gBI#Nursery">
        <rdfs:subClassOf rdf:resource="http://hit2gap.eu/h2g/h2gBI#PublicBuilding"/>
        <rdfs:label>Nursery</rdfs:label>
    </owl:Class>
    


    <!-- http://hit2gap.eu/h2g/h2gBI#Office -->

    <owl:Class rdf:about="http://hit2gap.eu/h2g/h2gBI#Office">
        <rdfs:subClassOf rdf:resource="http://www.buildingsmart-tech.org/ifcOWL/IFC2X3_Final#IfcSpace"/>
        <rdfs:comment xml:lang="en">Office is an instance of IfcSpace in the building representing an office.</rdfs:comment>
        <rdfs:label xml:lang="en">Office</rdfs:label>
    </owl:Class>
    


    <!-- http://hit2gap.eu/h2g/h2gBI#Oil -->

    <owl:Class rdf:about="http://hit2gap.eu/h2g/h2gBI#Oil">
        <rdfs:subClassOf rdf:resource="http://hit2gap.eu/h2g/h2gBI#PhysicalMedium"/>
        <rdfs:comment xml:lang="en">Oil represents oil as a physical medium to produce energy.</rdfs:comment>
        <rdfs:label xml:lang="en">Oil</rdfs:label>
    </owl:Class>
    


    <!-- http://hit2gap.eu/h2g/h2gBI#OpenSpace -->

    <owl:Class rdf:about="http://hit2gap.eu/h2g/h2gBI#OpenSpace">
        <rdfs:subClassOf rdf:resource="http://www.buildingsmart-tech.org/ifcOWL/IFC2X3_Final#IfcSpace"/>
        <rdfs:comment xml:lang="en">OpenSpace is an instance of IfcSpace in the building representing an open space.</rdfs:comment>
        <rdfs:label xml:lang="en">OpenSpace</rdfs:label>
    </owl:Class>
    


    <!-- http://hit2gap.eu/h2g/h2gBI#Orientation -->

    <owl:Class rdf:about="http://hit2gap.eu/h2g/h2gBI#Orientation">
        <rdfs:comment xml:lang="en">Orientation determines the orientation of the building.</rdfs:comment>
        <rdfs:label xml:lang="en">Orientation</rdfs:label>
    </owl:Class>
    


    <!-- http://hit2gap.eu/h2g/h2gBI#Pharmacy -->

    <owl:Class rdf:about="http://hit2gap.eu/h2g/h2gBI#Pharmacy">
        <rdfs:subClassOf rdf:resource="http://hit2gap.eu/h2g/h2gBI#CommercialBuilding"/>
        <rdfs:label>Pharmacy</rdfs:label>
    </owl:Class>
    


    <!-- http://hit2gap.eu/h2g/h2gBI#Photocopier -->

    <owl:Class rdf:about="http://hit2gap.eu/h2g/h2gBI#Photocopier">
        <rdfs:subClassOf rdf:resource="http://ifcowl.openbimstandards.org/IFC4_ADD2/index.html#IfcElectricAppliance"/>
    </owl:Class>
    


    <!-- http://hit2gap.eu/h2g/h2gBI#PhysicalMedium -->

    <owl:Class rdf:about="http://hit2gap.eu/h2g/h2gBI#PhysicalMedium">
        <rdfs:subClassOf>
            <owl:Restriction>
                <owl:onProperty rdf:resource="http://www.w3.org/ns/ssn/hasProperty"/>
                <owl:someValuesFrom rdf:resource="http://hit2gap.eu/h2g/h2gProperty#PhenomenonProperty"/>
            </owl:Restriction>
        </rdfs:subClassOf>
        <rdfs:comment xml:lang="en">PhysicalMedium represents the physical element that is used to produce energy.</rdfs:comment>
        <rdfs:label xml:lang="en">PhysicalMedium</rdfs:label>
    </owl:Class>
    


    <!-- http://hit2gap.eu/h2g/h2gBI#Player -->

    <owl:Class rdf:about="http://hit2gap.eu/h2g/h2gBI#Player">
        <rdfs:subClassOf rdf:resource="http://ifcowl.openbimstandards.org/IFC4_ADD2/index.html#IfcAudioVisualAppliance"/>
    </owl:Class>
    


    <!-- http://hit2gap.eu/h2g/h2gBI#Polar -->

    <owl:Class rdf:about="http://hit2gap.eu/h2g/h2gBI#Polar">
        <rdfs:subClassOf rdf:resource="http://hit2gap.eu/h2g/h2gBI#Climate"/>
        <rdfs:comment xml:lang="en">Polar represents an observation of the polar climate in a specific time.</rdfs:comment>
        <rdfs:label xml:lang="en">Polar</rdfs:label>
    </owl:Class>
    


    <!-- http://hit2gap.eu/h2g/h2gBI#PowerPlant -->

    <owl:Class rdf:about="http://hit2gap.eu/h2g/h2gBI#PowerPlant">
        <rdfs:subClassOf rdf:resource="http://hit2gap.eu/h2g/h2gBI#IndustrialBuilding"/>
        <rdfs:label>PowerPlant</rdfs:label>
    </owl:Class>
    


    <!-- http://hit2gap.eu/h2g/h2gBI#PrimarySchool -->

    <owl:Class rdf:about="http://hit2gap.eu/h2g/h2gBI#PrimarySchool">
        <rdfs:subClassOf rdf:resource="http://hit2gap.eu/h2g/h2gBI#EducationalBuilding"/>
        <rdfs:label>PrimarySchool</rdfs:label>
    </owl:Class>
    


    <!-- http://hit2gap.eu/h2g/h2gBI#Printer -->

    <owl:Class rdf:about="http://hit2gap.eu/h2g/h2gBI#Printer">
        <rdfs:subClassOf rdf:resource="http://ifcowl.openbimstandards.org/IFC4_ADD2/index.html#IfcCommunicationAppliance"/>
    </owl:Class>
    


    <!-- http://hit2gap.eu/h2g/h2gBI#Projector -->

    <owl:Class rdf:about="http://hit2gap.eu/h2g/h2gBI#Projector">
        <rdfs:subClassOf rdf:resource="http://ifcowl.openbimstandards.org/IFC4_ADD2/index.html#IfcAudioVisualAppliance"/>
    </owl:Class>
    


    <!-- http://hit2gap.eu/h2g/h2gBI#PublicBuilding -->

    <owl:Class rdf:about="http://hit2gap.eu/h2g/h2gBI#PublicBuilding">
        <rdfs:subClassOf rdf:resource="http://www.buildingsmart-tech.org/ifcOWL/IFC2X3_Final#IfcBuilding"/>
        <rdfs:label rdf:datatype="http://www.w3.org/2001/XMLSchema#string">PublicBuilding</rdfs:label>
    </owl:Class>
    


    <!-- http://hit2gap.eu/h2g/h2gBI#Radiation -->

    <owl:Class rdf:about="http://hit2gap.eu/h2g/h2gBI#Radiation">
        <rdfs:subClassOf rdf:resource="http://hit2gap.eu/h2g/h2gBI#PhysicalMedium"/>
        <rdfs:comment xml:lang="en">Radiation represents radiation as a physical medium to produce energy.</rdfs:comment>
    </owl:Class>
    


    <!-- http://hit2gap.eu/h2g/h2gBI#Receiver -->

    <owl:Class rdf:about="http://hit2gap.eu/h2g/h2gBI#Receiver">
        <rdfs:subClassOf rdf:resource="http://ifcowl.openbimstandards.org/IFC4_ADD2/index.html#IfcAudioVisualAppliance"/>
    </owl:Class>
    


    <!-- http://hit2gap.eu/h2g/h2gBI#Refrigerator -->

    <owl:Class rdf:about="http://hit2gap.eu/h2g/h2gBI#Refrigerator">
        <rdfs:subClassOf rdf:resource="http://ifcowl.openbimstandards.org/IFC4_ADD2/index.html#IfcElectricAppliance"/>
    </owl:Class>
    


    <!-- http://hit2gap.eu/h2g/h2gBI#ReligiousBuilding -->

    <owl:Class rdf:about="http://hit2gap.eu/h2g/h2gBI#ReligiousBuilding">
        <rdfs:subClassOf rdf:resource="http://www.buildingsmart-tech.org/ifcOWL/IFC2X3_Final#IfcBuilding"/>
        <rdfs:label>ReligiousBuilding</rdfs:label>
    </owl:Class>
    


    <!-- http://hit2gap.eu/h2g/h2gBI#Repeater -->

    <owl:Class rdf:about="http://hit2gap.eu/h2g/h2gBI#Repeater">
        <rdfs:subClassOf rdf:resource="http://hit2gap.eu/h2g/h2gBI#NetworkAppliance"/>
    </owl:Class>
    


    <!-- http://hit2gap.eu/h2g/h2gBI#ResidentialBuilding -->

    <owl:Class rdf:about="http://hit2gap.eu/h2g/h2gBI#ResidentialBuilding">
        <rdfs:subClassOf rdf:resource="http://www.buildingsmart-tech.org/ifcOWL/IFC2X3_Final#IfcBuilding"/>
        <rdfs:label>ResidentialBuilding</rdfs:label>
    </owl:Class>
    


    <!-- http://hit2gap.eu/h2g/h2gBI#RestRoom -->

    <owl:Class rdf:about="http://hit2gap.eu/h2g/h2gBI#RestRoom">
        <rdfs:subClassOf rdf:resource="http://www.buildingsmart-tech.org/ifcOWL/IFC2X3_Final#IfcSpace"/>
        <rdfs:comment xml:lang="en">RestRoom is an instance of IfcSpace in the building representing a rest room.</rdfs:comment>
        <rdfs:label xml:lang="en">RestRoom</rdfs:label>
    </owl:Class>
    


    <!-- http://hit2gap.eu/h2g/h2gBI#Room -->

    <owl:Class rdf:about="http://hit2gap.eu/h2g/h2gBI#Room">
        <rdfs:subClassOf rdf:resource="http://www.buildingsmart-tech.org/ifcOWL/IFC2X3_Final#IfcSpace"/>
        <rdfs:comment xml:lang="en">Room is an instance of IfcSpace in the building representing a Room.</rdfs:comment>
        <rdfs:label xml:lang="en">Room</rdfs:label>
    </owl:Class>
    


    <!-- http://hit2gap.eu/h2g/h2gBI#Router -->

    <owl:Class rdf:about="http://hit2gap.eu/h2g/h2gBI#Router">
        <rdfs:subClassOf rdf:resource="http://hit2gap.eu/h2g/h2gBI#NetworkAppliance"/>
    </owl:Class>
    


    <!-- http://hit2gap.eu/h2g/h2gBI#Scanner -->

    <owl:Class rdf:about="http://hit2gap.eu/h2g/h2gBI#Scanner">
        <rdfs:subClassOf rdf:resource="http://ifcowl.openbimstandards.org/IFC4_ADD2/index.html#IfcCommunicationAppliance"/>
    </owl:Class>
    


    <!-- http://hit2gap.eu/h2g/h2gBI#SecondarySchool -->

    <owl:Class rdf:about="http://hit2gap.eu/h2g/h2gBI#SecondarySchool">
        <rdfs:subClassOf rdf:resource="http://hit2gap.eu/h2g/h2gBI#EducationalBuilding"/>
        <rdfs:label>SecondarySchool</rdfs:label>
    </owl:Class>
    


    <!-- http://hit2gap.eu/h2g/h2gBI#Shade -->

    <owl:Class rdf:about="http://hit2gap.eu/h2g/h2gBI#Shade">
        <rdfs:subClassOf rdf:resource="http://hit2gap.eu/h2g/h2gBI#WindowCovering"/>
        <rdfs:comment xml:lang="en">A Shade is a type of a WindowCovering representing a window shade.</rdfs:comment>
        <rdfs:label xml:lang="en">Shade</rdfs:label>
    </owl:Class>
    


    <!-- http://hit2gap.eu/h2g/h2gBI#Shop -->

    <owl:Class rdf:about="http://hit2gap.eu/h2g/h2gBI#Shop">
        <rdfs:subClassOf rdf:resource="http://hit2gap.eu/h2g/h2gBI#CommercialBuilding"/>
        <rdfs:label rdf:datatype="http://www.w3.org/2001/XMLSchema#string">Shop</rdfs:label>
    </owl:Class>
    


    <!-- http://hit2gap.eu/h2g/h2gBI#Shutter -->

    <owl:Class rdf:about="http://hit2gap.eu/h2g/h2gBI#Shutter">
        <rdfs:subClassOf rdf:resource="http://hit2gap.eu/h2g/h2gBI#WindowCovering"/>
        <rdfs:comment xml:lang="en">A Shutter is a type of a WindowCovering representing a window shutter.</rdfs:comment>
        <rdfs:label xml:lang="en">Shutter</rdfs:label>
    </owl:Class>
    


    <!-- http://hit2gap.eu/h2g/h2gBI#Silo -->

    <owl:Class rdf:about="http://hit2gap.eu/h2g/h2gBI#Silo">
        <rdfs:subClassOf rdf:resource="http://hit2gap.eu/h2g/h2gBI#AgriculturalBuilding"/>
        <rdfs:label>Silo</rdfs:label>
    </owl:Class>
    


    <!-- http://hit2gap.eu/h2g/h2gBI#SimpleGlazing -->

    <owl:Class rdf:about="http://hit2gap.eu/h2g/h2gBI#SimpleGlazing">
        <rdfs:subClassOf rdf:resource="http://hit2gap.eu/h2g/h2gBI#WindowGlazing"/>
        <rdfs:comment xml:lang="en">It represents that glasses of the window are simple</rdfs:comment>
        <rdfs:label xml:lang="en">Simple Glazing</rdfs:label>
    </owl:Class>
    


    <!-- http://hit2gap.eu/h2g/h2gBI#Smartphone_Station -->

    <owl:Class rdf:about="http://hit2gap.eu/h2g/h2gBI#Smartphone_Station">
        <rdfs:subClassOf rdf:resource="http://ifcowl.openbimstandards.org/IFC4_ADD2/index.html#IfcAudioVisualAppliance"/>
    </owl:Class>
    


    <!-- http://hit2gap.eu/h2g/h2gBI#Steam -->

    <owl:Class rdf:about="http://hit2gap.eu/h2g/h2gBI#Steam">
        <rdfs:subClassOf rdf:resource="http://hit2gap.eu/h2g/h2gBI#PhysicalMedium"/>
        <rdfs:comment xml:lang="en">Steam represents steam as a physical medium to produce energy.</rdfs:comment>
        <rdfs:label xml:lang="en">Steam</rdfs:label>
    </owl:Class>
    


    <!-- http://hit2gap.eu/h2g/h2gBI#SteamPlant -->

    <owl:Class rdf:about="http://hit2gap.eu/h2g/h2gBI#SteamPlant">
        <rdfs:subClassOf rdf:resource="http://www.buildingsmart-tech.org/ifcOWL/IFC2X3_Final#IfcEnergyConversionDevice"/>
        <rdfs:comment xml:lang="en">A SteamPlant represents a plant using steam prime movers to drive electric generating apparatus.</rdfs:comment>
        <rdfs:label xml:lang="en">SteamPlant</rdfs:label>
    </owl:Class>
    


    <!-- http://hit2gap.eu/h2g/h2gBI#Subterranean -->

    <owl:Class rdf:about="http://hit2gap.eu/h2g/h2gBI#Subterranean">
        <rdfs:subClassOf rdf:resource="http://hit2gap.eu/h2g/h2gBI#Floor"/>
        <rdfs:comment xml:lang="en">A Sunterranean represents a subterranean floor.</rdfs:comment>
        <rdfs:label xml:lang="en">Subterranean</rdfs:label>
    </owl:Class>
    


    <!-- http://hit2gap.eu/h2g/h2gBI#SwimmingCenter -->

    <owl:Class rdf:about="http://hit2gap.eu/h2g/h2gBI#SwimmingCenter">
        <rdfs:subClassOf rdf:resource="http://hit2gap.eu/h2g/h2gBI#PublicBuilding"/>
        <rdfs:label>SwimmingCenter</rdfs:label>
    </owl:Class>
    


    <!-- http://hit2gap.eu/h2g/h2gBI#Switcher -->

    <owl:Class rdf:about="http://hit2gap.eu/h2g/h2gBI#Switcher">
        <rdfs:subClassOf rdf:resource="http://ifcowl.openbimstandards.org/IFC4_ADD2/index.html#IfcAudioVisualAppliance"/>
    </owl:Class>
    


    <!-- http://hit2gap.eu/h2g/h2gBI#Telephone -->

    <owl:Class rdf:about="http://hit2gap.eu/h2g/h2gBI#Telephone">
        <rdfs:subClassOf rdf:resource="http://ifcowl.openbimstandards.org/IFC4_ADD2/index.html#IfcAudioVisualAppliance"/>
    </owl:Class>
    


    <!-- http://hit2gap.eu/h2g/h2gBI#Temperate -->

    <owl:Class rdf:about="http://hit2gap.eu/h2g/h2gBI#Temperate">
        <rdfs:subClassOf rdf:resource="http://hit2gap.eu/h2g/h2gBI#Climate"/>
        <rdfs:comment xml:lang="en">Temperate represents an observation of the temperate climate in a specific time.</rdfs:comment>
        <rdfs:label xml:lang="en">Temperate</rdfs:label>
    </owl:Class>
    


    <!-- http://hit2gap.eu/h2g/h2gBI#Toilets -->

    <owl:Class rdf:about="http://hit2gap.eu/h2g/h2gBI#Toilets">
        <rdfs:subClassOf rdf:resource="http://www.buildingsmart-tech.org/ifcOWL/IFC2X3_Final#IfcSpace"/>
        <rdfs:comment xml:lang="en">Toilets is an instance of IfcSpace in the building representing toilets.</rdfs:comment>
        <rdfs:label xml:lang="en">Toilets</rdfs:label>
    </owl:Class>
    


    <!-- http://hit2gap.eu/h2g/h2gBI#TrainStation -->

    <owl:Class rdf:about="http://hit2gap.eu/h2g/h2gBI#TrainStation">
        <rdfs:subClassOf rdf:resource="http://hit2gap.eu/h2g/h2gBI#TransportBuilding"/>
        <rdfs:label rdf:datatype="http://www.w3.org/2001/XMLSchema#string">TrainStation</rdfs:label>
    </owl:Class>
    


    <!-- http://hit2gap.eu/h2g/h2gBI#TransportBuilding -->

    <owl:Class rdf:about="http://hit2gap.eu/h2g/h2gBI#TransportBuilding">
        <rdfs:subClassOf rdf:resource="http://www.buildingsmart-tech.org/ifcOWL/IFC2X3_Final#IfcBuilding"/>
        <rdfs:label>TransportBuilding</rdfs:label>
    </owl:Class>
    


    <!-- http://hit2gap.eu/h2g/h2gBI#Tropical -->

    <owl:Class rdf:about="http://hit2gap.eu/h2g/h2gBI#Tropical">
        <rdfs:subClassOf rdf:resource="http://hit2gap.eu/h2g/h2gBI#Climate"/>
        <rdfs:comment xml:lang="en">Tropical represents an observation of the tropical climate in a specific time.</rdfs:comment>
        <rdfs:label xml:lang="en">Tropical</rdfs:label>
    </owl:Class>
    


    <!-- http://hit2gap.eu/h2g/h2gBI#Tumble_Dryer -->

    <owl:Class rdf:about="http://hit2gap.eu/h2g/h2gBI#Tumble_Dryer">
        <rdfs:subClassOf rdf:resource="http://ifcowl.openbimstandards.org/IFC4_ADD2/index.html#IfcElectricAppliance"/>
    </owl:Class>
    


    <!-- http://hit2gap.eu/h2g/h2gBI#Tuner -->

    <owl:Class rdf:about="http://hit2gap.eu/h2g/h2gBI#Tuner">
        <rdfs:subClassOf rdf:resource="http://ifcowl.openbimstandards.org/IFC4_ADD2/index.html#IfcAudioVisualAppliance"/>
    </owl:Class>
    


    <!-- http://hit2gap.eu/h2g/h2gBI#University -->

    <owl:Class rdf:about="http://hit2gap.eu/h2g/h2gBI#University">
        <rdfs:subClassOf rdf:resource="http://hit2gap.eu/h2g/h2gBI#EducationalBuilding"/>
        <rdfs:label rdf:datatype="http://www.w3.org/2001/XMLSchema#string">University</rdfs:label>
    </owl:Class>
    


    <!-- http://hit2gap.eu/h2g/h2gBI#Vending_Machine -->

    <owl:Class rdf:about="http://hit2gap.eu/h2g/h2gBI#Vending_Machine">
        <rdfs:subClassOf rdf:resource="http://ifcowl.openbimstandards.org/IFC4_ADD2/index.html#IfcElectricAppliance"/>
    </owl:Class>
    


    <!-- http://hit2gap.eu/h2g/h2gBI#Warehouse -->

    <owl:Class rdf:about="http://hit2gap.eu/h2g/h2gBI#Warehouse">
        <rdfs:subClassOf rdf:resource="http://hit2gap.eu/h2g/h2gBI#IndustrialBuilding"/>
        <rdfs:label rdf:datatype="http://www.w3.org/2001/XMLSchema#string">Warehouse</rdfs:label>
    </owl:Class>
    


    <!-- http://hit2gap.eu/h2g/h2gBI#Washing_Machine -->

    <owl:Class rdf:about="http://hit2gap.eu/h2g/h2gBI#Washing_Machine">
        <rdfs:subClassOf rdf:resource="http://ifcowl.openbimstandards.org/IFC4_ADD2/index.html#IfcElectricAppliance"/>
    </owl:Class>
    


    <!-- http://hit2gap.eu/h2g/h2gBI#Water -->

    <owl:Class rdf:about="http://hit2gap.eu/h2g/h2gBI#Water">
        <rdfs:subClassOf rdf:resource="http://hit2gap.eu/h2g/h2gBI#PhysicalMedium"/>
        <rdfs:comment xml:lang="en">Water represents water as a physical medium to produce energy.</rdfs:comment>
        <rdfs:label xml:lang="en">Water</rdfs:label>
    </owl:Class>
    


    <!-- http://hit2gap.eu/h2g/h2gBI#WaterPlant -->

    <owl:Class rdf:about="http://hit2gap.eu/h2g/h2gBI#WaterPlant">
        <rdfs:subClassOf rdf:resource="http://www.buildingsmart-tech.org/ifcOWL/IFC2X3_Final#IfcEnergyConversionDevice"/>
        <rdfs:comment xml:lang="en">A WaterPlant represents a plant operated by pressure transmitted through a pipe by a liquid, such as water or oil.</rdfs:comment>
        <rdfs:label xml:lang="en">WaterPlant</rdfs:label>
    </owl:Class>
    


    <!-- http://hit2gap.eu/h2g/h2gBI#WetArea -->

    <owl:Class rdf:about="http://hit2gap.eu/h2g/h2gBI#WetArea">
        <rdfs:subClassOf rdf:resource="http://www.buildingsmart-tech.org/ifcOWL/IFC2X3_Final#IfcSpace"/>
        <rdfs:comment xml:lang="en">WetArea is an instance of IfcSpace in the building representing a wet area.</rdfs:comment>
        <rdfs:label xml:lang="en">WetArea</rdfs:label>
    </owl:Class>
    


    <!-- http://hit2gap.eu/h2g/h2gBI#WindowCovering -->

    <owl:Class rdf:about="http://hit2gap.eu/h2g/h2gBI#WindowCovering">
        <rdfs:comment xml:lang="en">A window covering is an element which covers a window in the building and is fully dependent on that window. The WindowCovering defines the occurrence of a covering type.</rdfs:comment>
        <rdfs:label xml:lang="en">Window Covering</rdfs:label>
    </owl:Class>
    


    <!-- http://hit2gap.eu/h2g/h2gBI#WindowGlazing -->

    <owl:Class rdf:about="http://hit2gap.eu/h2g/h2gBI#WindowGlazing">
        <rdfs:comment xml:lang="en">A window glazing describes the type of glass of a window in the building and is fully dependent on that window. The WindowGlazing defines the occurrence of a glass type.</rdfs:comment>
        <rdfs:label xml:lang="en">Window Glazing</rdfs:label>
    </owl:Class>
    


    <!-- http://hit2gap.eu/h2g/h2gBI#Display/screen -->

    <owl:Class rdf:about="http://hit2gap.eu/h2g/h2gBI#Display/screen">
        <rdfs:subClassOf rdf:resource="http://ifcowl.openbimstandards.org/IFC4_ADD2/index.html#IfcAudioVisualAppliance"/>
    </owl:Class>
    


    <!-- http://hit2gap.eu/h2g/h2gSensor#FeatureOfInterest -->

    <owl:Class rdf:about="http://hit2gap.eu/h2g/h2gSensor#FeatureOfInterest">
        <owl:equivalentClass rdf:resource="http://www.w3.org/ns/sosa/FeatureOfInterest"/>
        <rdfs:subClassOf rdf:resource="http://www.opengis/net/gml/_Feature"/>
        <rdfs:comment xml:lang="en">FeatureOfInterest is an extension of ssn#FeatureOfInterest  defined in SSN. We have extended it and made them equivalents.

A feature is an abstraction of real world phenomena (thing, person, event, etc). The thing whose property is being estimated or calculated in the course of an Observation to arrive at a Result or whose property is being manipulated by an Actuator, or which is being sampled or transformed in an act of Sampling.</rdfs:comment>
        <rdfs:isDefinedBy xml:lang="en">http://hit2gap.eu/h2g/h2gSensor#FeatureOfInterest</rdfs:isDefinedBy>
        <rdfs:label xml:lang="en">FeatureOfInterest</rdfs:label>
    </owl:Class>
    


    <!-- http://hit2gap.eu/h2g/h2gSensor#Hemisphere -->

    <owl:Class rdf:about="http://hit2gap.eu/h2g/h2gSensor#Hemisphere">
        <rdfs:comment xml:lang="en">Hemisphere denotes the hemisphere of a feature.</rdfs:comment>
        <rdfs:isDefinedBy>http://hit2gap.eu/h2g/h2gSensor#Hemisphere</rdfs:isDefinedBy>
        <rdfs:label xml:lang="en">Hemisphere</rdfs:label>
    </owl:Class>
    


    <!-- http://hit2gap.eu/h2g/h2gSensor#MobileBuildingApplianceLocationObservation -->

    <owl:Class rdf:about="http://hit2gap.eu/h2g/h2gSensor#MobileBuildingApplianceLocationObservation">
        <rdfs:subClassOf rdf:resource="http://hit2gap.eu/h2g/h2gSensor#Observation"/>
        <rdfs:comment xml:lang="en">This observation specifies a particular location of a mobile building appliance in a specific time.</rdfs:comment>
        <rdfs:isDefinedBy rdf:resource="http://hit2gap.eu/h2g/h2gSensor#MobileBuildingApplianceLocationObservation"/>
        <rdfs:isDefinedBy xml:lang="en">http://hit2gap.eu/h2g/h2gSensor#MobileBuildingApplianceLocationObservation</rdfs:isDefinedBy>
        <rdfs:label xml:lang="en">MobileBuildingApplianceLocationObservation</rdfs:label>
    </owl:Class>
    


    <!-- http://hit2gap.eu/h2g/h2gSensor#Observation -->

    <owl:Class rdf:about="http://hit2gap.eu/h2g/h2gSensor#Observation">
        <rdfs:subClassOf>
            <owl:Restriction>
                <owl:onProperty rdf:resource="http://hit2gap.eu/h2g/h2gSensor#hasObservationResultTime"/>
                <owl:someValuesFrom>
                    <owl:Class>
                        <owl:unionOf rdf:parseType="Collection">
                            <rdf:Description rdf:about="http://www.w3.org/2006/time#DateTimeInterval"/>
                            <rdf:Description rdf:about="http://www.w3.org/2006/time#Instant"/>
                        </owl:unionOf>
                    </owl:Class>
                </owl:someValuesFrom>
            </owl:Restriction>
        </rdfs:subClassOf>
        <rdfs:subClassOf>
            <owl:Restriction>
                <owl:onProperty rdf:resource="http://www.w3.org/ns/sosa/hasFeatureOfInterest"/>
                <owl:someValuesFrom rdf:resource="http://hit2gap.eu/h2g/h2gSensor#FeatureOfInterest"/>
            </owl:Restriction>
        </rdfs:subClassOf>
        <rdfs:subClassOf>
            <owl:Restriction>
                <owl:onProperty rdf:resource="http://hit2gap.eu/h2g/h2gSensor#hasObservationResultTime"/>
                <owl:allValuesFrom rdf:resource="http://www.w3.org/2006/time#DateTimeInterval"/>
            </owl:Restriction>
        </rdfs:subClassOf>
        <rdfs:subClassOf>
            <owl:Restriction>
                <owl:onProperty rdf:resource="http://hit2gap.eu/h2g/h2gSensor#hasObservationResultTime"/>
                <owl:allValuesFrom rdf:resource="http://www.w3.org/2006/time#Instant"/>
            </owl:Restriction>
        </rdfs:subClassOf>
        <rdfs:subClassOf>
            <owl:Restriction>
                <owl:onProperty rdf:resource="http://www.w3.org/ns/sosa/hasResult"/>
                <owl:allValuesFrom rdf:resource="http://www.w3.org/ns/sosa/Result"/>
            </owl:Restriction>
        </rdfs:subClassOf>
        <rdfs:subClassOf>
            <owl:Restriction>
                <owl:onProperty rdf:resource="http://hit2gap.eu/h2g/h2gSensor#externalID"/>
                <owl:allValuesFrom rdf:resource="http://www.w3.org/2001/XMLSchema#anyURI"/>
            </owl:Restriction>
        </rdfs:subClassOf>
        <rdfs:comment xml:lang="en">Observation is an extension of ssn#Observation  defined in SSN. We have extended it and made them equivalents.</rdfs:comment>
        <rdfs:isDefinedBy xml:lang="en">http://hit2gap.eu/h2g/h2gSensor#Observation</rdfs:isDefinedBy>
        <rdfs:label xml:lang="en">Observation</rdfs:label>
    </owl:Class>
    


    <!-- http://hit2gap.eu/ontomg#AcDcConverter -->

    <owl:Class rdf:about="http://hit2gap.eu/ontomg#AcDcConverter">
        <rdfs:subClassOf rdf:resource="http://hit2gap.eu/ontomg#Converter"/>
        <rdfs:comment xml:lang="en">An inverter and a rectifier perform opposite functions in electronic circuits. Both act as electric power converters; a rectifier changes current from alternating current (AC) to direct current (DC), while an inverter converts DC to AC.</rdfs:comment>
        <rdfs:isDefinedBy xml:lang="en">http://hit2gap.eu/ontomg#AcDcConverter</rdfs:isDefinedBy>
        <rdfs:label xml:lang="en">AcDcConverter</rdfs:label>
    </owl:Class>
    


    <!-- http://hit2gap.eu/ontomg#BiomassBranch -->

    <owl:Class rdf:about="http://hit2gap.eu/ontomg#BiomassBranch">
        <rdfs:subClassOf rdf:resource="http://hit2gap.eu/ontomg#RenewableDERBranch"/>
        <rdfs:comment xml:lang="en">BiomassBranch represents a  branch which produces energy by burning wood and other organic matter.</rdfs:comment>
        <rdfs:isDefinedBy xml:lang="en">http://hit2gap.eu/ontomg#BiomassBranch</rdfs:isDefinedBy>
        <rdfs:label xml:lang="en">BiomassBranch</rdfs:label>
    </owl:Class>
    


    <!-- http://hit2gap.eu/ontomg#Branch -->

    <owl:Class rdf:about="http://hit2gap.eu/ontomg#Branch">
        <rdfs:subClassOf>
            <owl:Restriction>
                <owl:onProperty rdf:resource="http://hit2gap.eu/ontomg#hasA"/>
                <owl:someValuesFrom rdf:resource="http://hit2gap.eu/ontomg#BranchController"/>
            </owl:Restriction>
        </rdfs:subClassOf>
        <rdfs:subClassOf>
            <owl:Restriction>
                <owl:onProperty rdf:resource="http://hit2gap.eu/ontomg#isComposedOf"/>
                <owl:someValuesFrom rdf:resource="http://hit2gap.eu/ontomg#Branch"/>
            </owl:Restriction>
        </rdfs:subClassOf>
        <rdfs:comment xml:lang="en">A branch is an energy consumer or producer that has a specific energy load over a certain time span (called energyprofile).</rdfs:comment>
        <rdfs:isDefinedBy xml:lang="en">http://hit2gap.eu/ontomg#Branch</rdfs:isDefinedBy>
        <rdfs:label xml:lang="en">Branch</rdfs:label>
    </owl:Class>
    


    <!-- http://hit2gap.eu/ontomg#BranchController -->

    <owl:Class rdf:about="http://hit2gap.eu/ontomg#BranchController">
        <rdfs:subClassOf rdf:resource="http://hit2gap.eu/ontomg#CIMConductingEquipement"/>
        <rdfs:comment xml:lang="en">A Branch Controller is the manager of  branch operations.</rdfs:comment>
        <rdfs:isDefinedBy xml:lang="en">http://hit2gap.eu/ontomg#BranchController</rdfs:isDefinedBy>
        <rdfs:label xml:lang="en">BranchController</rdfs:label>
    </owl:Class>
    


    <!-- http://hit2gap.eu/ontomg#BranchSwitch -->

    <owl:Class rdf:about="http://hit2gap.eu/ontomg#BranchSwitch">
        <rdfs:comment xml:lang="en">The Branch Switch is responsible of turning on/off a branch.</rdfs:comment>
        <rdfs:isDefinedBy xml:lang="en">http://hit2gap.eu/ontomg#BranchSwitch</rdfs:isDefinedBy>
        <rdfs:label xml:lang="en">BranchSwitch</rdfs:label>
    </owl:Class>
    


    <!-- http://hit2gap.eu/ontomg#CHPBranch -->

    <owl:Class rdf:about="http://hit2gap.eu/ontomg#CHPBranch">
        <rdfs:subClassOf rdf:resource="http://hit2gap.eu/ontomg#NonRenewableDERBranch"/>
        <rdfs:comment xml:lang="en">CHPBranch represents a combined heat and power (CHP) branch, which uses  a heat engine or power station to generate electricity and useful heat at the same time.</rdfs:comment>
        <rdfs:isDefinedBy xml:lang="en">http://hit2gap.eu/ontomg#CHPBranch</rdfs:isDefinedBy>
        <rdfs:label xml:lang="en">CHPBranch</rdfs:label>
    </owl:Class>
    


    <!-- http://hit2gap.eu/ontomg#CIMConductingEquipement -->

    <owl:Class rdf:about="http://hit2gap.eu/ontomg#CIMConductingEquipement">
        <rdfs:comment xml:lang="en">A ConductingEquipment concept, represents the parts of the power system that are designed to carry current. This concepts is from the  Common Information Model (CIM), which is a widely accepted energy information
model being part of the IEC 61970 standards.</rdfs:comment>
        <rdfs:isDefinedBy xml:lang="en">http://hit2gap.eu/ontomg#CIMConductingEquipement</rdfs:isDefinedBy>
        <rdfs:label xml:lang="en">ConductingEquipment</rdfs:label>
    </owl:Class>
    


    <!-- http://hit2gap.eu/ontomg#CIMRectifierInverter -->

    <owl:Class rdf:about="http://hit2gap.eu/ontomg#CIMRectifierInverter">
        <rdfs:comment xml:lang="en">A CIMRectifierInverter concept, represents the parts of the power system that are designed to inverte/rectify current.  
An inverter and a rectifier perform opposite functions in electronic circuits. Both act as electric power converters; a rectifier changes current from alternating current (AC) to direct current (DC), while an inverter converts DC to AC.
This concepts is from the  Common Information Model (CIM), which is a widely accepted energy information model being part of the IEC 61970 standards.</rdfs:comment>
        <rdfs:isDefinedBy xml:lang="en">http://hit2gap.eu/ontomg#CIMRectifierInverter</rdfs:isDefinedBy>
        <rdfs:label xml:lang="en">CIMRectifierInverter</rdfs:label>
    </owl:Class>
    


    <!-- http://hit2gap.eu/ontomg#CoalBranch -->

    <owl:Class rdf:about="http://hit2gap.eu/ontomg#CoalBranch">
        <rdfs:subClassOf rdf:resource="http://hit2gap.eu/ontomg#NonRenewableDERBranch"/>
        <rdfs:comment xml:lang="en">CoalBranch represents a  branch which uses coal  to generate energy.</rdfs:comment>
        <rdfs:isDefinedBy xml:lang="en">http://hit2gap.eu/ontomg#CoalBranch</rdfs:isDefinedBy>
        <rdfs:label xml:lang="en">CoalBranch</rdfs:label>
    </owl:Class>
    


    <!-- http://hit2gap.eu/ontomg#Converter -->

    <owl:Class rdf:about="http://hit2gap.eu/ontomg#Converter">
        <rdfs:subClassOf rdf:resource="http://hit2gap.eu/ontomg#CIMRectifierInverter"/>
        <rdfs:comment xml:lang="en">An inverter and a rectifier perform opposite functions in electronic circuits. Both act as electric power converters; a rectifier changes current from alternating current (AC) to direct current (DC), while an inverter converts DC to AC.</rdfs:comment>
        <rdfs:isDefinedBy xml:lang="en">http://hit2gap.eu/ontomg#Converter</rdfs:isDefinedBy>
        <rdfs:label xml:lang="en">Converter</rdfs:label>
    </owl:Class>
    


    <!-- http://hit2gap.eu/ontomg#DERBranch -->

    <owl:Class rdf:about="http://hit2gap.eu/ontomg#DERBranch">
        <rdfs:subClassOf rdf:resource="http://hit2gap.eu/ontomg#Branch"/>
        <rdfs:subClassOf>
            <owl:Restriction>
                <owl:onProperty rdf:resource="http://hit2gap.eu/ontomg#hasA"/>
                <owl:someValuesFrom rdf:resource="http://hit2gap.eu/ontomg#BranchSwitch"/>
            </owl:Restriction>
        </rdfs:subClassOf>
        <rdfs:comment xml:lang="en">DERBranch represents a distributed energy resource branch, which consists of renewable or nonrenewable energy sources.</rdfs:comment>
        <rdfs:isDefinedBy xml:lang="en">http://hit2gap.eu/ontomg#DERBranch</rdfs:isDefinedBy>
        <rdfs:label xml:lang="en">DERBranch</rdfs:label>
    </owl:Class>
    


    <!-- http://hit2gap.eu/ontomg#DieselGenerator -->

    <owl:Class rdf:about="http://hit2gap.eu/ontomg#DieselGenerator">
        <rdfs:subClassOf rdf:resource="http://hit2gap.eu/ontomg#NonRenewableDERBranch"/>
        <rdfs:comment xml:lang="en">A DieselGenerator is the combination of a diesel engine with an electric generator (often an alternator) to generate electrical energy.</rdfs:comment>
        <rdfs:isDefinedBy xml:lang="en">http://hit2gap.eu/ontomg#DieselGenerator</rdfs:isDefinedBy>
        <rdfs:label xml:lang="en">DieselGenerator</rdfs:label>
    </owl:Class>
    


    <!-- http://hit2gap.eu/ontomg#ELBranch -->

    <owl:Class rdf:about="http://hit2gap.eu/ontomg#ELBranch">
        <rdfs:subClassOf rdf:resource="http://hit2gap.eu/ontomg#Branch"/>
        <rdfs:comment xml:lang="en">An Electrical Load Branch is an electrical component or branch that consumes electric power. It mainly consists of electrical appliance components.</rdfs:comment>
        <rdfs:isDefinedBy xml:lang="en">http://hit2gap.eu/ontomg#ELBranch</rdfs:isDefinedBy>
        <rdfs:label xml:lang="en">ELBranch</rdfs:label>
    </owl:Class>
    


    <!-- http://hit2gap.eu/ontomg#ESBranch -->

    <owl:Class rdf:about="http://hit2gap.eu/ontomg#ESBranch">
        <rdfs:subClassOf rdf:resource="http://hit2gap.eu/ontomg#Branch"/>
        <rdfs:comment xml:lang="en">Energy storage systems play an essential role in stabilizing the power system, improving the quality of power supply, and achieving power peak shaving. The energy storage branch consists mainly of the energy storage device (e.g., flywheel, super-capacitor) and a converter.</rdfs:comment>
        <rdfs:isDefinedBy xml:lang="en">http://hit2gap.eu/ontomg#ESBranch</rdfs:isDefinedBy>
        <rdfs:label xml:lang="en">ESBranch</rdfs:label>
    </owl:Class>
    


    <!-- http://hit2gap.eu/ontomg#FuelCellBranch -->

    <owl:Class rdf:about="http://hit2gap.eu/ontomg#FuelCellBranch">
        <rdfs:subClassOf rdf:resource="http://hit2gap.eu/ontomg#OilBranch"/>
        <rdfs:subClassOf>
            <owl:Restriction>
                <owl:onProperty rdf:resource="http://hit2gap.eu/ontomg#hasA"/>
                <owl:allValuesFrom rdf:resource="http://hit2gap.eu/ontomg#Converter"/>
            </owl:Restriction>
        </rdfs:subClassOf>
        <rdfs:subClassOf>
            <owl:Restriction>
                <owl:onProperty rdf:resource="http://hit2gap.eu/ontomg#hasA"/>
                <owl:allValuesFrom rdf:resource="http://hit2gap.eu/ontomg#DieselGenerator"/>
            </owl:Restriction>
        </rdfs:subClassOf>
        <rdfs:comment xml:lang="en">FuelCellBranch is an electrochemical energy conversion device. It produces electricity from external supplies of fuel (on the anode side) and oxidant (on the cathode side). These reacts in the presence of an electrolyte.</rdfs:comment>
        <rdfs:isDefinedBy xml:lang="en">http://hit2gap.eu/ontomg#FuelCellBranch</rdfs:isDefinedBy>
        <rdfs:label xml:lang="en">FuelCellBranch</rdfs:label>
    </owl:Class>
    


    <!-- http://hit2gap.eu/ontomg#GasBranch -->

    <owl:Class rdf:about="http://hit2gap.eu/ontomg#GasBranch">
        <rdfs:subClassOf rdf:resource="http://hit2gap.eu/ontomg#NonRenewableDERBranch"/>
        <rdfs:comment xml:lang="en">GasBranch represents a  branch which uses gas  to generate energy.</rdfs:comment>
        <rdfs:isDefinedBy xml:lang="en">http://hit2gap.eu/ontomg#GasBranch</rdfs:isDefinedBy>
        <rdfs:label xml:lang="en">GasBranch</rdfs:label>
    </owl:Class>
    


    <!-- http://hit2gap.eu/ontomg#GeoThermalBranch -->

    <owl:Class rdf:about="http://hit2gap.eu/ontomg#GeoThermalBranch">
        <rdfs:subClassOf rdf:resource="http://hit2gap.eu/ontomg#RenewableDERBranch"/>
        <rdfs:comment xml:lang="en">GeoThermalBranch represents a  branch which produces geothermal energy.
Geothermal resources are reservoirs of hot water that exist at varying temperatures and depths below the Earth&apos;s surface.</rdfs:comment>
        <rdfs:isDefinedBy xml:lang="en">http://hit2gap.eu/ontomg#GeoThermalBranch</rdfs:isDefinedBy>
        <rdfs:label xml:lang="en">GeoThermalBranch</rdfs:label>
    </owl:Class>
    


    <!-- http://hit2gap.eu/ontomg#HydroPowerBranch -->

    <owl:Class rdf:about="http://hit2gap.eu/ontomg#HydroPowerBranch">
        <rdfs:subClassOf rdf:resource="http://hit2gap.eu/ontomg#RenewableDERBranch"/>
        <rdfs:comment xml:lang="en">HydroPowerBranch represents a  branch which produces energy derived from the energy of falling water or fast running water.</rdfs:comment>
        <rdfs:isDefinedBy xml:lang="en">http://hit2gap.eu/ontomg#HydroPowerBranch</rdfs:isDefinedBy>
        <rdfs:label xml:lang="en">HydroPowerBranch</rdfs:label>
    </owl:Class>
    


    <!-- http://hit2gap.eu/ontomg#InfraBranch -->

    <owl:Class rdf:about="http://hit2gap.eu/ontomg#InfraBranch">
        <rdfs:subClassOf rdf:resource="http://hit2gap.eu/ontomg#Branch"/>
        <rdfs:comment xml:lang="en">An InfraBranch represents an infrastructure branch, where each has its own Branch Switch and Branch Controller.</rdfs:comment>
        <rdfs:isDefinedBy xml:lang="en">http://hit2gap.eu/ontomg#InfraBranch</rdfs:isDefinedBy>
        <rdfs:label xml:lang="en">InfraBranch</rdfs:label>
    </owl:Class>
    


    <!-- http://hit2gap.eu/ontomg#Inverter -->

    <owl:Class rdf:about="http://hit2gap.eu/ontomg#Inverter">
        <rdfs:subClassOf rdf:resource="http://hit2gap.eu/ontomg#Converter"/>
        <rdfs:comment xml:lang="en">An inverter and a rectifier perform opposite functions in electronic circuits. Both act as electric power converters; a rectifier changes current from alternating current (AC) to direct current (DC), while an inverter converts DC to AC. An inverter can be a Monophasic  or a Triphasic.</rdfs:comment>
        <rdfs:isDefinedBy xml:lang="en">http://hit2gap.eu/ontomg#Inverter</rdfs:isDefinedBy>
        <rdfs:label xml:lang="en">Inverter</rdfs:label>
    </owl:Class>
    


    <!-- http://hit2gap.eu/ontomg#MicroCHPBranch -->

    <owl:Class rdf:about="http://hit2gap.eu/ontomg#MicroCHPBranch">
        <rdfs:subClassOf rdf:resource="http://hit2gap.eu/ontomg#NonRenewableDERBranch"/>
        <rdfs:comment xml:lang="en">MicroCHPBranch represents a micro combined heat and power (CHP) branch, which uses  a heat engine or power station to generate electricity and useful heat at the same time.</rdfs:comment>
        <rdfs:isDefinedBy xml:lang="en">http://hit2gap.eu/ontomg#MicroCHPBranch</rdfs:isDefinedBy>
        <rdfs:label xml:lang="en">MicroCHPBranch</rdfs:label>
    </owl:Class>
    


    <!-- http://hit2gap.eu/ontomg#Microgrid -->

    <owl:Class rdf:about="http://hit2gap.eu/ontomg#Microgrid">
        <rdfs:subClassOf rdf:resource="http://hit2gap.eu/h2g/h2gSensor#FeatureOfInterest"/>
        <rdfs:subClassOf>
            <owl:Restriction>
                <owl:onProperty rdf:resource="http://hit2gap.eu/ontomg#hasBranch"/>
                <owl:someValuesFrom rdf:resource="http://hit2gap.eu/ontomg#Branch"/>
            </owl:Restriction>
        </rdfs:subClassOf>
        <rdfs:comment xml:lang="en">A microgrid is based on several branches that link the building infrastructure with the generated building renewable flows, non-renewable flows and the different building systems linked with that flows.</rdfs:comment>
        <rdfs:isDefinedBy xml:lang="en">http://hit2gap.eu/ontomg#Microgrid</rdfs:isDefinedBy>
        <rdfs:label xml:lang="en">Microgrid</rdfs:label>
    </owl:Class>
    


    <!-- http://hit2gap.eu/ontomg#MicroturbinesBranch -->

    <owl:Class rdf:about="http://hit2gap.eu/ontomg#MicroturbinesBranch">
        <rdfs:subClassOf rdf:resource="http://hit2gap.eu/ontomg#RenewableDERBranch"/>
        <rdfs:comment xml:lang="en">MicroturbinesBranch represents a  branch with a type of combustion turbine that produces both heat and electricity on a relatively small scale.</rdfs:comment>
        <rdfs:isDefinedBy xml:lang="en">http://hit2gap.eu/ontomg#MicroturbinesBranch</rdfs:isDefinedBy>
        <rdfs:label xml:lang="en">MicroturbinesBranch</rdfs:label>
    </owl:Class>
    


    <!-- http://hit2gap.eu/ontomg#MonophasicInverter -->

    <owl:Class rdf:about="http://hit2gap.eu/ontomg#MonophasicInverter">
        <rdfs:subClassOf rdf:resource="http://hit2gap.eu/ontomg#Inverter"/>
        <rdfs:comment xml:lang="en">An Inverter can be a Monophasic  or a Triphasic.</rdfs:comment>
        <rdfs:isDefinedBy xml:lang="en">http://hit2gap.eu/ontomg#MonophasicInverter</rdfs:isDefinedBy>
        <rdfs:label xml:lang="en">MonophasicInverter</rdfs:label>
    </owl:Class>
    


    <!-- http://hit2gap.eu/ontomg#NonRenewableDERBranch -->

    <owl:Class rdf:about="http://hit2gap.eu/ontomg#NonRenewableDERBranch">
        <rdfs:subClassOf rdf:resource="http://hit2gap.eu/ontomg#DERBranch"/>
        <rdfs:comment xml:lang="en">NonRenewableDERBranch represents the non-renewable distributed energy resource branches.</rdfs:comment>
        <rdfs:isDefinedBy xml:lang="en">http://hit2gap.eu/ontomg#NonRenewableDERBranch</rdfs:isDefinedBy>
        <rdfs:label xml:lang="en">NonRenewableDERBranch</rdfs:label>
    </owl:Class>
    


    <!-- http://hit2gap.eu/ontomg#NuclearBranch -->

    <owl:Class rdf:about="http://hit2gap.eu/ontomg#NuclearBranch">
        <rdfs:subClassOf rdf:resource="http://hit2gap.eu/ontomg#NonRenewableDERBranch"/>
        <rdfs:comment xml:lang="en">NuclearBranch represents a  branch, which uses nuclear energy to generate energy.</rdfs:comment>
        <rdfs:isDefinedBy xml:lang="en">http://hit2gap.eu/ontomg#NuclearBranch</rdfs:isDefinedBy>
        <rdfs:label xml:lang="en">NuclearBranch</rdfs:label>
    </owl:Class>
    


    <!-- http://hit2gap.eu/ontomg#OilBranch -->

    <owl:Class rdf:about="http://hit2gap.eu/ontomg#OilBranch">
        <rdfs:subClassOf rdf:resource="http://hit2gap.eu/ontomg#NonRenewableDERBranch"/>
        <rdfs:comment xml:lang="en">OilBranch represents a  branch which uses oil to generate energy.</rdfs:comment>
        <rdfs:isDefinedBy xml:lang="en">http://hit2gap.eu/ontomg#OilBranch</rdfs:isDefinedBy>
        <rdfs:label xml:lang="en">OilBranch</rdfs:label>
    </owl:Class>
    


    <!-- http://hit2gap.eu/ontomg#PhotovoltaicBranch -->

    <owl:Class rdf:about="http://hit2gap.eu/ontomg#PhotovoltaicBranch">
        <rdfs:subClassOf rdf:resource="http://hit2gap.eu/ontomg#RenewableDERBranch"/>
        <rdfs:comment xml:lang="en">A PhotovoltaicBranch represents a photovoltaic power system that directly converts solar energy into electricity.</rdfs:comment>
        <rdfs:isDefinedBy xml:lang="en">http://hit2gap.eu/ontomg#PhotovoltaicBranch</rdfs:isDefinedBy>
        <rdfs:label xml:lang="en">PhotovoltaicBranch</rdfs:label>
    </owl:Class>
    


    <!-- http://hit2gap.eu/ontomg#ReciprocatingBranch -->

    <owl:Class rdf:about="http://hit2gap.eu/ontomg#ReciprocatingBranch">
        <rdfs:subClassOf rdf:resource="http://hit2gap.eu/ontomg#NonRenewableDERBranch"/>
        <rdfs:comment xml:lang="en">ReciprocatingBranch is an engine that utilizes one or more pressure-driven pistons in order to convert back-and-forth motion into a rotating motion. The most common form of reciprocating engine used to generate electricity is the diesel engine, which is used in combination with an electric generator to form a diesel generator.</rdfs:comment>
        <rdfs:isDefinedBy xml:lang="en">http://hit2gap.eu/ontomg#ReciprocatingBranch</rdfs:isDefinedBy>
        <rdfs:label xml:lang="en">ReciprocatingBranch</rdfs:label>
    </owl:Class>
    


    <!-- http://hit2gap.eu/ontomg#RegulatingCondEq -->

    <owl:Class rdf:about="http://hit2gap.eu/ontomg#RegulatingCondEq">
        <rdfs:isDefinedBy xml:lang="en">http://hit2gap.eu/ontomg#RegulatingCondEq</rdfs:isDefinedBy>
        <rdfs:label xml:lang="en">RegulatingCondEq</rdfs:label>
    </owl:Class>
    


    <!-- http://hit2gap.eu/ontomg#RenewableDERBranch -->

    <owl:Class rdf:about="http://hit2gap.eu/ontomg#RenewableDERBranch">
        <rdfs:subClassOf rdf:resource="http://hit2gap.eu/ontomg#DERBranch"/>
        <rdfs:comment xml:lang="en">RenewableDERBranch represents the renewable distributed energy resource branches.</rdfs:comment>
        <rdfs:isDefinedBy xml:lang="en">http://hit2gap.eu/ontomg#RenewableDERBranch</rdfs:isDefinedBy>
        <rdfs:label xml:lang="en">RenewableDERBranch</rdfs:label>
    </owl:Class>
    


    <!-- http://hit2gap.eu/ontomg#SmallWindPowerBranch -->

    <owl:Class rdf:about="http://hit2gap.eu/ontomg#SmallWindPowerBranch">
        <rdfs:subClassOf rdf:resource="http://hit2gap.eu/ontomg#RenewableDERBranch"/>
        <rdfs:subClassOf>
            <owl:Restriction>
                <owl:onProperty rdf:resource="http://hit2gap.eu/ontomg#hasA"/>
                <owl:someValuesFrom rdf:resource="http://hit2gap.eu/ontomg#SmallWindTurbine"/>
            </owl:Restriction>
        </rdfs:subClassOf>
        <rdfs:subClassOf>
            <owl:Restriction>
                <owl:onProperty rdf:resource="http://hit2gap.eu/ontomg#hasA"/>
                <owl:allValuesFrom rdf:resource="http://hit2gap.eu/ontomg#Converter"/>
            </owl:Restriction>
        </rdfs:subClassOf>
        <rdfs:comment xml:lang="en">SmallWindPowerBranch represents a branch that uses air flow through wind turbines to mechanically generate electric power.</rdfs:comment>
        <rdfs:isDefinedBy xml:lang="en">http://hit2gap.eu/ontomg#SmallWindPowerBranch</rdfs:isDefinedBy>
        <rdfs:label xml:lang="en">SmallWindPowerBranch</rdfs:label>
    </owl:Class>
    


    <!-- http://hit2gap.eu/ontomg#SmallWindTurbine -->

    <owl:Class rdf:about="http://hit2gap.eu/ontomg#SmallWindTurbine">
        <rdfs:subClassOf rdf:resource="http://hit2gap.eu/ontomg#RegulatingCondEq"/>
        <rdfs:isDefinedBy xml:lang="en">http://hit2gap.eu/ontomg#SmallWindTurbine</rdfs:isDefinedBy>
        <rdfs:label xml:lang="en">SmallWindTurbine</rdfs:label>
    </owl:Class>
    


    <!-- http://hit2gap.eu/ontomg#SolarCell -->

    <owl:Class rdf:about="http://hit2gap.eu/ontomg#SolarCell">
        <rdfs:subClassOf rdf:resource="http://hit2gap.eu/ontomg#RegulatingCondEq"/>
        <rdfs:isDefinedBy xml:lang="en">http://hit2gap.eu/ontomg#SolarCell</rdfs:isDefinedBy>
        <rdfs:label xml:lang="en">SolarCell</rdfs:label>
    </owl:Class>
    


    <!-- http://hit2gap.eu/ontomg#SolarHybridBranch -->

    <owl:Class rdf:about="http://hit2gap.eu/ontomg#SolarHybridBranch">
        <rdfs:subClassOf rdf:resource="http://hit2gap.eu/ontomg#RenewableDERBranch"/>
        <rdfs:comment xml:lang="en">A SolarHybridBranch represents a power system that the transforms  energy from sunlight into electricity, either directly using photovoltaics (PV), indirectly using concentrated solar power, or a combination.</rdfs:comment>
        <rdfs:isDefinedBy xml:lang="en">http://hit2gap.eu/ontomg#SolarHybridBranch</rdfs:isDefinedBy>
        <rdfs:label xml:lang="en">SolarHybridBranch</rdfs:label>
    </owl:Class>
    


    <!-- http://hit2gap.eu/ontomg#SolarPowerBranch -->

    <owl:Class rdf:about="http://hit2gap.eu/ontomg#SolarPowerBranch">
        <rdfs:subClassOf rdf:resource="http://hit2gap.eu/ontomg#RenewableDERBranch"/>
        <rdfs:subClassOf>
            <owl:Restriction>
                <owl:onProperty rdf:resource="http://hit2gap.eu/ontomg#hasA"/>
                <owl:someValuesFrom rdf:resource="http://hit2gap.eu/ontomg#SolarCell"/>
            </owl:Restriction>
        </rdfs:subClassOf>
        <rdfs:subClassOf>
            <owl:Restriction>
                <owl:onProperty rdf:resource="http://hit2gap.eu/ontomg#hasA"/>
                <owl:allValuesFrom rdf:resource="http://hit2gap.eu/ontomg#Converter"/>
            </owl:Restriction>
        </rdfs:subClassOf>
        <rdfs:comment xml:lang="en">A SolarPowerBranch represents a power system that directly converts solar energy into electricity.</rdfs:comment>
        <rdfs:isDefinedBy xml:lang="en">http://hit2gap.eu/ontomg#SolarPowerBranch</rdfs:isDefinedBy>
        <rdfs:label xml:lang="en">SolarPowerBranch</rdfs:label>
    </owl:Class>
    


    <!-- http://hit2gap.eu/ontomg#StirlingBranch -->

    <owl:Class rdf:about="http://hit2gap.eu/ontomg#StirlingBranch">
        <rdfs:subClassOf rdf:resource="http://hit2gap.eu/ontomg#NonRenewableDERBranch"/>
        <rdfs:comment xml:lang="en">A StirlingBranch represents a heat engine that operates by cyclic compression and expansion of air or other gas (the working fluid) at different temperatures, such that there is a net conversion of heat energy to mechanical work. More specifically, the Stirling engine is a closed-cycle regenerative heat engine with a permanently gaseous working fluid.</rdfs:comment>
        <rdfs:isDefinedBy xml:lang="en">http://hit2gap.eu/ontomg#StirlingBranch</rdfs:isDefinedBy>
        <rdfs:label xml:lang="en">StirlingBranch</rdfs:label>
    </owl:Class>
    


    <!-- http://hit2gap.eu/ontomg#TriphasicInverter -->

    <owl:Class rdf:about="http://hit2gap.eu/ontomg#TriphasicInverter">
        <rdfs:subClassOf rdf:resource="http://hit2gap.eu/ontomg#Inverter"/>
        <rdfs:comment xml:lang="en">An Inverter can be a Monophasic  or a Triphasic.</rdfs:comment>
        <rdfs:isDefinedBy xml:lang="en">http://hit2gap.eu/ontomg#TriphasicInverter</rdfs:isDefinedBy>
        <rdfs:label xml:lang="en">TriphasicInverter</rdfs:label>
    </owl:Class>
    


    <!-- http://hit2gap.eu/ontomg#WindHybridBranch -->

    <owl:Class rdf:about="http://hit2gap.eu/ontomg#WindHybridBranch">
        <rdfs:subClassOf rdf:resource="http://hit2gap.eu/ontomg#RenewableDERBranch"/>
        <rdfs:comment xml:lang="en">WindHybridBranch represents the use of air flow through wind turbines to mechanically power generators for electric power.</rdfs:comment>
        <rdfs:isDefinedBy xml:lang="en">http://hit2gap.eu/ontomg#WindHybridBranch</rdfs:isDefinedBy>
        <rdfs:label xml:lang="en">WindHybridBranch</rdfs:label>
    </owl:Class>
    


    <!-- http://ifcowl.openbimstandards.org/IFC4_ADD2/index.html#IfcActuator -->

    <owl:Class rdf:about="http://ifcowl.openbimstandards.org/IFC4_ADD2/index.html#IfcActuator">
        <owl:equivalentClass rdf:resource="http://www.buildingsmart-tech.org/ifcOWL/IFC2X3_Final#IfcActuatorType"/>
        <rdfs:subClassOf rdf:resource="http://hit2gap.eu/h2g/h2gBA#Monitoring"/>
        <rdfs:subClassOf rdf:resource="http://www.buildingsmart-tech.org/ifcOWL/IFC2X3_Final#IfcDistributionControlElement"/>
        <rdfs:subClassOf>
            <owl:Restriction>
                <owl:onProperty rdf:resource="http://hit2gap.eu/h2g/h2gBI#OpenClose"/>
                <owl:allValuesFrom rdf:resource="http://hit2gap.eu/h2g/h2gBI#WindowCovering"/>
            </owl:Restriction>
        </rdfs:subClassOf>
        <rdfs:subClassOf>
            <owl:Restriction>
                <owl:onProperty rdf:resource="http://hit2gap.eu/h2g/h2gBI#OpenClose"/>
                <owl:allValuesFrom rdf:resource="http://www.buildingsmart-tech.org/ifcOWL/IFC2X3_Final#IfcWindow"/>
            </owl:Restriction>
        </rdfs:subClassOf>
        <rdfs:comment xml:lang="en">An actuator is a mechanical device for moving or controlling a mechanism or system. An actuator takes energy, usually created by air, electricity, or liquid, and converts that into some kind of motion.</rdfs:comment>
        <rdfs:isDefinedBy xml:lang="en">http://ifcowl.openbimstandards.org/IFC4_ADD2/index.html#IfcActuator</rdfs:isDefinedBy>
        <rdfs:label xml:lang="en">IfcActuator</rdfs:label>
    </owl:Class>
    


    <!-- http://ifcowl.openbimstandards.org/IFC4_ADD2/index.html#IfcAirToAirHeatRecover -->

    <owl:Class rdf:about="http://ifcowl.openbimstandards.org/IFC4_ADD2/index.html#IfcAirToAirHeatRecover">
        <owl:equivalentClass rdf:resource="http://www.buildingsmart-tech.org/ifcOWL/IFC2X3_Final#IfcAirToAirHeatRecoveryType"/>
        <rdfs:subClassOf rdf:resource="http://www.buildingsmart-tech.org/ifcOWL/IFC2X3_Final#IfcEnergyConversionDevice"/>
        <rdfs:comment xml:lang="en">IfcAirToAirHeatRecovery defines the occurrence of any air-to-air heat recovery device; common information about air-to-air heat recovery device types is handled by IfcAirToAirHeatRecoveryType. The IfcAirToAirHeatRecoveryType (if present) may establish the common type name, usage (predefined type), properties, materials, ports, composition, assignments, and representations. The IfcAirToAirHeatRecoveryType is attached using the IfcRelDefinesByType objectified relationship and is accessible by the IsTypedBy inverse attribute.</rdfs:comment>
        <rdfs:isDefinedBy xml:lang="en">http://ifcowl.openbimstandards.org/IFC4_ADD2/index.html#IfcAirToAirHeatRecover</rdfs:isDefinedBy>
        <rdfs:label xml:lang="en">IfcAirToAirHeatRecover</rdfs:label>
    </owl:Class>
    


    <!-- http://ifcowl.openbimstandards.org/IFC4_ADD2/index.html#IfcAlarm -->

    <owl:Class rdf:about="http://ifcowl.openbimstandards.org/IFC4_ADD2/index.html#IfcAlarm">
        <owl:equivalentClass rdf:resource="http://www.buildingsmart-tech.org/ifcOWL/IFC2X3_Final#IfcAlarmType"/>
        <rdfs:subClassOf rdf:resource="http://hit2gap.eu/h2g/h2gBA#Monitoring"/>
        <rdfs:subClassOf rdf:resource="http://www.buildingsmart-tech.org/ifcOWL/IFC2X3_Final#IfcDistributionControlElement"/>
        <rdfs:comment xml:lang="en">An alarm is a device that signals the existence of a condition or situation that is outside the boundaries of normal expectation or that activates such a device. Alarms include the provision of break glass buttons and manual pull boxes that are used to activate alarms.</rdfs:comment>
        <rdfs:isDefinedBy xml:lang="en">http://ifcowl.openbimstandards.org/IFC4_ADD2/index.html#IfcAlarm</rdfs:isDefinedBy>
        <rdfs:label xml:lang="en">IfcAlarm</rdfs:label>
    </owl:Class>
    


    <!-- http://ifcowl.openbimstandards.org/IFC4_ADD2/index.html#IfcAudioVisualAppliance -->

    <owl:Class rdf:about="http://ifcowl.openbimstandards.org/IFC4_ADD2/index.html#IfcAudioVisualAppliance">
        <rdfs:subClassOf rdf:resource="http://www.buildingsmart-tech.org/ifcOWL/IFC2X3_Final#IfcFlowTerminal"/>
        <rdfs:comment xml:lang="en">An audio-visual appliance is a device that displays, captures, transmits, or receives audio or video.
Audio-visual appliances may be fixed in place or may be able to be moved from one space to another. They may require an electrical supply that may be supplied either by an electrical circuit or provided from a local battery source. Audio-visual appliances may be connected to data circuits including specialist circuits for audio visual purposes only.</rdfs:comment>
        <rdfs:isDefinedBy xml:lang="en">http://ifcowl.openbimstandards.org/IFC4_ADD2/index.html#IfcAudioVisualAppliance</rdfs:isDefinedBy>
        <rdfs:label xml:lang="en">IfcAudioVisualAppliance</rdfs:label>
    </owl:Class>
    


    <!-- http://ifcowl.openbimstandards.org/IFC4_ADD2/index.html#IfcBoiler -->

    <owl:Class rdf:about="http://ifcowl.openbimstandards.org/IFC4_ADD2/index.html#IfcBoiler">
        <owl:equivalentClass rdf:resource="http://www.buildingsmart-tech.org/ifcOWL/IFC2X3_Final#IfcBoilerType"/>
        <rdfs:subClassOf rdf:resource="http://www.buildingsmart-tech.org/ifcOWL/IFC2X3_Final#IfcEnergyConversionDevice"/>
        <rdfs:comment xml:lang="en">IfcBoiler defines the occurrence of any boiler; common information about boiler types is handled by IfcBoilerType. The IfcBoilerType (if present) may establish the common type name, usage (predefined type), properties, materials, ports, composition, assignments, and representations. The IfcBoilerType is attached using the IfcRelDefinesByType objectified relationship and is accessible by the IsTypedBy inverse attribute.</rdfs:comment>
        <rdfs:isDefinedBy xml:lang="en">http://ifcowl.openbimstandards.org/IFC4_ADD2/index.html#IfcBoiler</rdfs:isDefinedBy>
        <rdfs:label xml:lang="en">IfcBoiler</rdfs:label>
    </owl:Class>
    


    <!-- http://ifcowl.openbimstandards.org/IFC4_ADD2/index.html#IfcBurner -->

    <owl:Class rdf:about="http://ifcowl.openbimstandards.org/IFC4_ADD2/index.html#IfcBurner">
        <rdfs:subClassOf rdf:resource="http://www.buildingsmart-tech.org/ifcOWL/IFC2X3_Final#IfcEnergyConversionDevice"/>
        <rdfs:comment xml:lang="en">A burner is a device that converts fuel into heat through combustion. It includes gas, oil, and wood burners.</rdfs:comment>
        <rdfs:isDefinedBy xml:lang="en">http://ifcowl.openbimstandards.org/IFC4_ADD2/index.html#IfcBurner</rdfs:isDefinedBy>
        <rdfs:label xml:lang="en">IfcBurner</rdfs:label>
    </owl:Class>
    


    <!-- http://ifcowl.openbimstandards.org/IFC4_ADD2/index.html#IfcChiller -->

    <owl:Class rdf:about="http://ifcowl.openbimstandards.org/IFC4_ADD2/index.html#IfcChiller">
        <owl:equivalentClass rdf:resource="http://www.buildingsmart-tech.org/ifcOWL/IFC2X3_Final#IfcChillerType"/>
        <rdfs:subClassOf rdf:resource="http://www.buildingsmart-tech.org/ifcOWL/IFC2X3_Final#IfcEnergyConversionDevice"/>
        <rdfs:comment xml:lang="en">A chiller is a device used to remove heat from a liquid via a vapor-compression or absorption refrigeration cycle to cool a fluid, typically water or a mixture of water and glycol. The chilled fluid is then used to cool and dehumidify air in a building.</rdfs:comment>
        <rdfs:isDefinedBy xml:lang="en">http://ifcowl.openbimstandards.org/IFC4_ADD2/index.html#IfcChiller</rdfs:isDefinedBy>
        <rdfs:label xml:lang="en">IfcChiller</rdfs:label>
    </owl:Class>
    


    <!-- http://ifcowl.openbimstandards.org/IFC4_ADD2/index.html#IfcCoil -->

    <owl:Class rdf:about="http://ifcowl.openbimstandards.org/IFC4_ADD2/index.html#IfcCoil">
        <owl:equivalentClass rdf:resource="http://www.buildingsmart-tech.org/ifcOWL/IFC2X3_Final#IfcCoilType"/>
        <rdfs:subClassOf rdf:resource="http://www.buildingsmart-tech.org/ifcOWL/IFC2X3_Final#IfcEnergyConversionDevice"/>
        <rdfs:comment xml:lang="en">A coil is a device used to provide heat transfer between non-mixing media. A common example is a cooling coil, which utilizes a finned coil in which circulates chilled water, antifreeze, or refrigerant that is used to remove heat from air moving across the surface of the coil. A coil may be used either for heating or cooling purposes by placing a series of tubes (the coil) carrying a heating or cooling fluid into an airstream. The coil may be constructed from tubes bundled in a serpentine form or from finned tubes that give a extended heat transfer surface</rdfs:comment>
        <rdfs:isDefinedBy xml:lang="en">http://ifcowl.openbimstandards.org/IFC4_ADD2/index.html#IfcCoil</rdfs:isDefinedBy>
        <rdfs:label xml:lang="en">IfcCoil</rdfs:label>
    </owl:Class>
    


    <!-- http://ifcowl.openbimstandards.org/IFC4_ADD2/index.html#IfcCommunicationAppliance -->

    <owl:Class rdf:about="http://ifcowl.openbimstandards.org/IFC4_ADD2/index.html#IfcCommunicationAppliance">
        <rdfs:subClassOf rdf:resource="http://www.buildingsmart-tech.org/ifcOWL/IFC2X3_Final#IfcFlowTerminal"/>
        <rdfs:comment xml:lang="en">A communications appliance transmits and receives electronic or digital information as data or sound.
Communication appliances may be fixed in place or may be able to be moved from one space to another. Communication appliances require an electrical supply that may be supplied either by an electrical circuit or provided from a local battery source.</rdfs:comment>
        <rdfs:isDefinedBy xml:lang="en">http://ifcowl.openbimstandards.org/IFC4_ADD2/index.html#IfcCommunicationAppliance</rdfs:isDefinedBy>
        <rdfs:label xml:lang="en">IfcCommunicationAppliance</rdfs:label>
    </owl:Class>
    


    <!-- http://ifcowl.openbimstandards.org/IFC4_ADD2/index.html#IfcCompressor -->

    <owl:Class rdf:about="http://ifcowl.openbimstandards.org/IFC4_ADD2/index.html#IfcCompressor">
        <owl:equivalentClass rdf:resource="http://www.buildingsmart-tech.org/ifcOWL/IFC2X3_Final#IfcCompressorType"/>
        <rdfs:subClassOf rdf:resource="http://www.buildingsmart-tech.org/ifcOWL/IFC2X3_Final#IfcFlowMovingDevice"/>
        <rdfs:comment xml:lang="en">An IfcCompressor is a device that compresses a fluid typically used in a refrigeration circuit.</rdfs:comment>
        <rdfs:isDefinedBy xml:lang="en">http://ifcowl.openbimstandards.org/IFC4_ADD2/index.html#IfcCompressor</rdfs:isDefinedBy>
        <rdfs:label xml:lang="en">IfcCompressor</rdfs:label>
    </owl:Class>
    


    <!-- http://ifcowl.openbimstandards.org/IFC4_ADD2/index.html#IfcCondenser -->

    <owl:Class rdf:about="http://ifcowl.openbimstandards.org/IFC4_ADD2/index.html#IfcCondenser">
        <owl:equivalentClass rdf:resource="http://www.buildingsmart-tech.org/ifcOWL/IFC2X3_Final#IfcCondenserType"/>
        <rdfs:subClassOf rdf:resource="http://www.buildingsmart-tech.org/ifcOWL/IFC2X3_Final#IfcEnergyConversionDevice"/>
        <rdfs:comment xml:lang="en">A condenser is a device that is used to dissipate heat, typically by condensing a substance such as a refrigerant from its gaseous to its liquid state.</rdfs:comment>
        <rdfs:isDefinedBy xml:lang="en">http://ifcowl.openbimstandards.org/IFC4_ADD2/index.html#IfcCondenser</rdfs:isDefinedBy>
        <rdfs:label xml:lang="en">IfcCondenser</rdfs:label>
    </owl:Class>
    


    <!-- http://ifcowl.openbimstandards.org/IFC4_ADD2/index.html#IfcCoolingTower -->

    <owl:Class rdf:about="http://ifcowl.openbimstandards.org/IFC4_ADD2/index.html#IfcCoolingTower">
        <owl:equivalentClass rdf:resource="http://www.buildingsmart-tech.org/ifcOWL/IFC2X3_Final#IfcCoolingTowerType"/>
        <rdfs:subClassOf rdf:resource="http://www.buildingsmart-tech.org/ifcOWL/IFC2X3_Final#IfcEnergyConversionDevice"/>
        <rdfs:comment xml:lang="en">A cooling tower is a device which rejects heat to ambient air by circulating a fluid such as water through it to reduce its temperature by partial evaporation.</rdfs:comment>
        <rdfs:isDefinedBy xml:lang="en">http://ifcowl.openbimstandards.org/IFC4_ADD2/index.html#IfcCoolingTower</rdfs:isDefinedBy>
        <rdfs:label xml:lang="en">IfcCoolingTower</rdfs:label>
    </owl:Class>
    


    <!-- http://ifcowl.openbimstandards.org/IFC4_ADD2/index.html#IfcDamper -->

    <owl:Class rdf:about="http://ifcowl.openbimstandards.org/IFC4_ADD2/index.html#IfcDamper">
        <owl:equivalentClass rdf:resource="http://www.buildingsmart-tech.org/ifcOWL/IFC2X3_Final#IfcDamperType"/>
        <rdfs:subClassOf rdf:resource="http://www.buildingsmart-tech.org/ifcOWL/IFC2X3_Final#IfcFlowController"/>
        <rdfs:comment xml:lang="en">IfcDamper defines the occurrence of any damper; common information about damper types is handled by IfcDamperType. The IfcDamperType (if present) may establish the common type name, usage (predefined type), properties, materials, ports, composition, assignments, and representations. The IfcDamperType is attached using the IfcRelDefinesByType objectified relationship and is accessible by the IsTypedBy inverse attribute.</rdfs:comment>
        <rdfs:isDefinedBy xml:lang="en">http://ifcowl.openbimstandards.org/IFC4_ADD2/index.html#IfcDamper</rdfs:isDefinedBy>
        <rdfs:label xml:lang="en">IfcDamper</rdfs:label>
    </owl:Class>
    


    <!-- http://ifcowl.openbimstandards.org/IFC4_ADD2/index.html#IfcElectricAppliance -->

    <owl:Class rdf:about="http://ifcowl.openbimstandards.org/IFC4_ADD2/index.html#IfcElectricAppliance">
        <owl:equivalentClass rdf:resource="http://www.buildingsmart-tech.org/ifcOWL/IFC2X3_Final#IfcElectricApplianceType"/>
        <rdfs:subClassOf rdf:resource="http://www.buildingsmart-tech.org/ifcOWL/IFC2X3_Final#IfcFlowTerminal"/>
        <rdfs:comment xml:lang="en">IfcElectricAppliance defines the occurrence of any electric appliance; common information about electric appliance types is handled by IfcElectricApplianceType. The IfcElectricApplianceType (if present) may establish the common type name, usage (predefined type), properties, materials, ports, composition, assignments, and representations.</rdfs:comment>
        <rdfs:isDefinedBy xml:lang="en">http://ifcowl.openbimstandards.org/IFC4_ADD2/index.html#IfcElectricAppliance</rdfs:isDefinedBy>
        <rdfs:label xml:lang="en">IfcElectricAppliance</rdfs:label>
    </owl:Class>
    


    <!-- http://ifcowl.openbimstandards.org/IFC4_ADD2/index.html#IfcElectricFlowStorageDevice -->

    <owl:Class rdf:about="http://ifcowl.openbimstandards.org/IFC4_ADD2/index.html#IfcElectricFlowStorageDevice">
        <owl:equivalentClass rdf:resource="http://www.buildingsmart-tech.org/ifcOWL/IFC2X3_Final#IfcElectricFlowStorageDeviceType"/>
        <rdfs:subClassOf rdf:resource="http://www.buildingsmart-tech.org/ifcOWL/IFC2X3_Final#IfcFlowStorageDevice"/>
        <rdfs:comment xml:lang="en">An electric flow storage device is a device in which electrical energy is stored and from which energy may be progressively released.</rdfs:comment>
        <rdfs:isDefinedBy xml:lang="en">http://ifcowl.openbimstandards.org/IFC4_ADD2/index.html#IfcElectricFlowStorageDevice</rdfs:isDefinedBy>
        <rdfs:label xml:lang="en">IfcElectricFlowStorageDevice</rdfs:label>
    </owl:Class>
    


    <!-- http://ifcowl.openbimstandards.org/IFC4_ADD2/index.html#IfcElectricGenerator -->

    <owl:Class rdf:about="http://ifcowl.openbimstandards.org/IFC4_ADD2/index.html#IfcElectricGenerator">
        <owl:equivalentClass rdf:resource="http://www.buildingsmart-tech.org/ifcOWL/IFC2X3_Final#IfcElectricGeneratorType"/>
        <rdfs:subClassOf rdf:resource="http://www.buildingsmart-tech.org/ifcOWL/IFC2X3_Final#IfcEnergyConversionDevice"/>
        <rdfs:comment xml:lang="en">An electric generator is an engine that is a machine for converting mechanical energy into electrical energy.</rdfs:comment>
        <rdfs:isDefinedBy xml:lang="en">http://ifcowl.openbimstandards.org/IFC4_ADD2/index.html#IfcElectricGenerator</rdfs:isDefinedBy>
        <rdfs:label xml:lang="en">IfcElectricGenerator</rdfs:label>
    </owl:Class>
    


    <!-- http://ifcowl.openbimstandards.org/IFC4_ADD2/index.html#IfcElectricMotor -->

    <owl:Class rdf:about="http://ifcowl.openbimstandards.org/IFC4_ADD2/index.html#IfcElectricMotor">
        <owl:equivalentClass rdf:resource="http://www.buildingsmart-tech.org/ifcOWL/IFC2X3_Final#IfcElectricMotorType"/>
        <rdfs:subClassOf rdf:resource="http://www.buildingsmart-tech.org/ifcOWL/IFC2X3_Final#IfcEnergyConversionDevice"/>
        <rdfs:comment xml:lang="en">An electric motor is an engine that is a machine for converting electrical energy into mechanical energy.</rdfs:comment>
        <rdfs:isDefinedBy xml:lang="en">http://ifcowl.openbimstandards.org/IFC4_ADD2/index.html#IfcElectricMotor</rdfs:isDefinedBy>
        <rdfs:label xml:lang="en">IfcElectricMotor</rdfs:label>
    </owl:Class>
    


    <!-- http://ifcowl.openbimstandards.org/IFC4_ADD2/index.html#IfcEngine -->

    <owl:Class rdf:about="http://ifcowl.openbimstandards.org/IFC4_ADD2/index.html#IfcEngine">
        <rdfs:subClassOf rdf:resource="http://www.buildingsmart-tech.org/ifcOWL/IFC2X3_Final#IfcEnergyConversionDevice"/>
        <rdfs:comment xml:lang="en">An engine is a device that converts fuel into mechanical energy through combustion.</rdfs:comment>
        <rdfs:isDefinedBy xml:lang="en">http://ifcowl.openbimstandards.org/IFC4_ADD2/index.html#IfcEngine</rdfs:isDefinedBy>
        <rdfs:label xml:lang="en">IfcEngine</rdfs:label>
    </owl:Class>
    


    <!-- http://ifcowl.openbimstandards.org/IFC4_ADD2/index.html#IfcEvaporativeCooler -->

    <owl:Class rdf:about="http://ifcowl.openbimstandards.org/IFC4_ADD2/index.html#IfcEvaporativeCooler">
        <owl:equivalentClass rdf:resource="http://www.buildingsmart-tech.org/ifcOWL/IFC2X3_Final#IfcEvaporativeCoolerType"/>
        <rdfs:subClassOf rdf:resource="http://www.buildingsmart-tech.org/ifcOWL/IFC2X3_Final#IfcEnergyConversionDevice"/>
        <rdfs:comment xml:lang="en">An evaporative cooler is a device that cools air by saturating it with water vapor.</rdfs:comment>
        <rdfs:isDefinedBy xml:lang="en">http://ifcowl.openbimstandards.org/IFC4_ADD2/index.html#IfcEvaporativeCooler</rdfs:isDefinedBy>
        <rdfs:label xml:lang="en">IfcEvaporativeCooler</rdfs:label>
    </owl:Class>
    


    <!-- http://ifcowl.openbimstandards.org/IFC4_ADD2/index.html#IfcEvaporator -->

    <owl:Class rdf:about="http://ifcowl.openbimstandards.org/IFC4_ADD2/index.html#IfcEvaporator">
        <owl:equivalentClass rdf:resource="http://www.buildingsmart-tech.org/ifcOWL/IFC2X3_Final#IfcEvaporatorType"/>
        <rdfs:subClassOf rdf:resource="http://www.buildingsmart-tech.org/ifcOWL/IFC2X3_Final#IfcEnergyConversionDevice"/>
        <rdfs:comment xml:lang="en">An evaporator is a device in which a liquid refrigerent is vaporized and absorbs heat from the surrounding fluid.</rdfs:comment>
        <rdfs:isDefinedBy xml:lang="en">http://ifcowl.openbimstandards.org/IFC4_ADD2/index.html#IfcEvaporator</rdfs:isDefinedBy>
        <rdfs:label xml:lang="en">IfcEvaporator</rdfs:label>
    </owl:Class>
    


    <!-- http://ifcowl.openbimstandards.org/IFC4_ADD2/index.html#IfcFan -->

    <owl:Class rdf:about="http://ifcowl.openbimstandards.org/IFC4_ADD2/index.html#IfcFan">
        <owl:equivalentClass rdf:resource="http://www.buildingsmart-tech.org/ifcOWL/IFC2X3_Final#IfcFanType"/>
        <rdfs:subClassOf rdf:resource="http://www.buildingsmart-tech.org/ifcOWL/IFC2X3_Final#IfcFlowMovingDevice"/>
        <rdfs:comment xml:lang="en">IfcFan defines the occurrence of any fan; common information about fan types is handled by IfcFanType. The IfcFanType (if present) may establish the common type name, usage (predefined type), properties, materials, ports, composition, assignments, and representations.</rdfs:comment>
        <rdfs:isDefinedBy xml:lang="en">http://ifcowl.openbimstandards.org/IFC4_ADD2/index.html#IfcFan</rdfs:isDefinedBy>
        <rdfs:label xml:lang="en">IfcFan</rdfs:label>
    </owl:Class>
    


    <!-- http://ifcowl.openbimstandards.org/IFC4_ADD2/index.html#IfcFireSuppressionTerminal -->

    <owl:Class rdf:about="http://ifcowl.openbimstandards.org/IFC4_ADD2/index.html#IfcFireSuppressionTerminal">
        <owl:equivalentClass rdf:resource="http://www.buildingsmart-tech.org/ifcOWL/IFC2X3_Final#IfcFireSuppressionTerminalType"/>
        <rdfs:subClassOf rdf:resource="http://www.buildingsmart-tech.org/ifcOWL/IFC2X3_Final#IfcFlowTerminal"/>
        <rdfs:comment xml:lang="en">A fire suppression terminal has the purpose of delivering a fluid (gas or liquid) that will suppress a fire.
A fire suppression terminal provides for all forms of sprinkler, spreader and other form of terminal that is connected to a pipework system and intended to act in the role of suppressing a fire.</rdfs:comment>
        <rdfs:isDefinedBy xml:lang="en">http://ifcowl.openbimstandards.org/IFC4_ADD2/index.html#IfcFireSuppressionTerminal</rdfs:isDefinedBy>
        <rdfs:label xml:lang="en">IfcFireSuppressionTerminal</rdfs:label>
    </owl:Class>
    


    <!-- http://ifcowl.openbimstandards.org/IFC4_ADD2/index.html#IfcHeatExchanger -->

    <owl:Class rdf:about="http://ifcowl.openbimstandards.org/IFC4_ADD2/index.html#IfcHeatExchanger">
        <owl:equivalentClass rdf:resource="http://www.buildingsmart-tech.org/ifcOWL/IFC2X3_Final#IfcHeatExchangerType"/>
        <rdfs:subClassOf rdf:resource="http://www.buildingsmart-tech.org/ifcOWL/IFC2X3_Final#IfcEnergyConversionDevice"/>
        <rdfs:comment xml:lang="en">A heat exchanger is a device used to provide heat transfer between non-mixing media such as plate and shell and tube heat exchangers.
IfcHeatExchanger is commonly used on water-side distribution systems to recover energy from a liquid to another liquid (typically water-based), whereas IfcAirToAirHeatRecovery is commonly used on air-side distribution systems to recover energy from a gas to a gas (usually air).</rdfs:comment>
        <rdfs:isDefinedBy xml:lang="en">http://ifcowl.openbimstandards.org/IFC4_ADD2/index.html#IfcHeatExchanger</rdfs:isDefinedBy>
        <rdfs:label xml:lang="en">IfcHeatExchanger</rdfs:label>
    </owl:Class>
    


    <!-- http://ifcowl.openbimstandards.org/IFC4_ADD2/index.html#IfcHumidifier -->

    <owl:Class rdf:about="http://ifcowl.openbimstandards.org/IFC4_ADD2/index.html#IfcHumidifier">
        <owl:equivalentClass rdf:resource="http://www.buildingsmart-tech.org/ifcOWL/IFC2X3_Final#IfcHumidifierType"/>
        <rdfs:subClassOf rdf:resource="http://www.buildingsmart-tech.org/ifcOWL/IFC2X3_Final#IfcEnergyConversionDevice"/>
        <rdfs:comment xml:lang="en">A humidifier is a device that adds moisture into the air.</rdfs:comment>
        <rdfs:isDefinedBy xml:lang="en">http://ifcowl.openbimstandards.org/IFC4_ADD2/index.html#IfcHumidifier</rdfs:isDefinedBy>
        <rdfs:label xml:lang="en">IfcHumidifier</rdfs:label>
    </owl:Class>
    


    <!-- http://ifcowl.openbimstandards.org/IFC4_ADD2/index.html#IfcInterceptor -->

    <owl:Class rdf:about="http://ifcowl.openbimstandards.org/IFC4_ADD2/index.html#IfcInterceptor">
        <rdfs:subClassOf rdf:resource="http://www.buildingsmart-tech.org/ifcOWL/IFC2X3_Final#IfcFlowTreatmentDevice"/>
        <rdfs:comment xml:lang="en">An interceptor is a device designed and installed in order to separate and retain deleterious, hazardous or undesirable matter while permitting normal sewage or liquids to discharge into a collection system by gravity.</rdfs:comment>
        <rdfs:isDefinedBy xml:lang="en">http://ifcowl.openbimstandards.org/IFC4_ADD2/index.html#IfcInterceptor</rdfs:isDefinedBy>
        <rdfs:label xml:lang="en">IfcInterceptor</rdfs:label>
    </owl:Class>
    


    <!-- http://ifcowl.openbimstandards.org/IFC4_ADD2/index.html#IfcLamp -->

    <owl:Class rdf:about="http://ifcowl.openbimstandards.org/IFC4_ADD2/index.html#IfcLamp">
        <owl:equivalentClass rdf:resource="http://www.buildingsmart-tech.org/ifcOWL/IFC2X3_Final#IfcLampType"/>
        <rdfs:subClassOf rdf:resource="http://www.buildingsmart-tech.org/ifcOWL/IFC2X3_Final#IfcFlowTerminal"/>
        <rdfs:subClassOf>
            <owl:Restriction>
                <owl:onProperty rdf:resource="http://hit2gap.eu/h2g/h2gBI#hasLampType"/>
                <owl:allValuesFrom rdf:resource="http://hit2gap.eu/h2g/h2gBI#LampType"/>
            </owl:Restriction>
        </rdfs:subClassOf>
        <rdfs:comment xml:lang="en">A lamp is an artificial light source such as a light bulb or tube.</rdfs:comment>
        <rdfs:isDefinedBy xml:lang="en">http://ifcowl.openbimstandards.org/IFC4_ADD2/index.html#IfcLamp</rdfs:isDefinedBy>
        <rdfs:label xml:lang="en">IfcLamp</rdfs:label>
    </owl:Class>
    


    <!-- http://ifcowl.openbimstandards.org/IFC4_ADD2/index.html#IfcOutlet -->

    <owl:Class rdf:about="http://ifcowl.openbimstandards.org/IFC4_ADD2/index.html#IfcOutlet">
        <owl:equivalentClass rdf:resource="http://www.buildingsmart-tech.org/ifcOWL/IFC2X3_Final#IfcOutletType"/>
        <rdfs:subClassOf rdf:resource="http://www.buildingsmart-tech.org/ifcOWL/IFC2X3_Final#IfcFlowTerminal"/>
        <rdfs:comment xml:lang="en">IfcOutlet defines the occurrence of any outlet; common information about outlet types is handled by IfcOutletType. The IfcOutletType (if present) may establish the common type name, usage (predefined type), properties, materials, ports, composition, assignments, and representations.</rdfs:comment>
        <rdfs:isDefinedBy xml:lang="en">http://ifcowl.openbimstandards.org/IFC4_ADD2/index.html#IfcOutlet</rdfs:isDefinedBy>
        <rdfs:label xml:lang="en">IfcOutlet</rdfs:label>
    </owl:Class>
    


    <!-- http://ifcowl.openbimstandards.org/IFC4_ADD2/index.html#IfcPump -->

    <owl:Class rdf:about="http://ifcowl.openbimstandards.org/IFC4_ADD2/index.html#IfcPump">
        <owl:equivalentClass rdf:resource="http://www.buildingsmart-tech.org/ifcOWL/IFC2X3_Final#IfcPumpType"/>
        <rdfs:subClassOf rdf:resource="http://www.buildingsmart-tech.org/ifcOWL/IFC2X3_Final#IfcFlowMovingDevice"/>
        <rdfs:comment xml:lang="en">IfcPump defines the occurrence of any pump; common information about pump types is handled by IfcPumpType. The IfcPumpType (if present) may establish the common type name, usage (predefined type), properties, materials, ports, composition, assignments, and representations.</rdfs:comment>
        <rdfs:isDefinedBy xml:lang="en">http://ifcowl.openbimstandards.org/IFC4_ADD2/index.html#IfcPump</rdfs:isDefinedBy>
        <rdfs:label xml:lang="en">IfcPump</rdfs:label>
    </owl:Class>
    


    <!-- http://ifcowl.openbimstandards.org/IFC4_ADD2/index.html#IfcSanitaryTerminal -->

    <owl:Class rdf:about="http://ifcowl.openbimstandards.org/IFC4_ADD2/index.html#IfcSanitaryTerminal">
        <owl:equivalentClass rdf:resource="http://www.buildingsmart-tech.org/ifcOWL/IFC2X3_Final#IfcSanitaryTerminalType"/>
        <rdfs:subClassOf rdf:resource="http://www.buildingsmart-tech.org/ifcOWL/IFC2X3_Final#IfcFlowTerminal"/>
        <rdfs:comment xml:lang="en">IfcSanitaryTerminal defines the occurrence of any sanitary terminal; common information about sanitary terminal types is handled by IfcSanitaryTerminalType. The IfcSanitaryTerminalType (if present) may establish the common type name, usage (predefined type), properties, materials, ports, composition, assignments, and representations.</rdfs:comment>
        <rdfs:isDefinedBy xml:lang="en">http://ifcowl.openbimstandards.org/IFC4_ADD2/index.html#IfcSanitaryTerminal</rdfs:isDefinedBy>
        <rdfs:label xml:lang="en">IfcSanitaryTerminal</rdfs:label>
    </owl:Class>
    


    <!-- http://ifcowl.openbimstandards.org/IFC4_ADD2/index.html#IfcSensor -->

    <owl:Class rdf:about="http://ifcowl.openbimstandards.org/IFC4_ADD2/index.html#IfcSensor">
        <owl:equivalentClass rdf:resource="http://www.buildingsmart-tech.org/ifcOWL/IFC2X3_Final#IfcSensorType"/>
        <owl:equivalentClass rdf:resource="http://www.w3.org/ns/sosa/Sensor"/>
        <rdfs:subClassOf rdf:resource="http://hit2gap.eu/h2g/h2gBA#Monitoring"/>
        <rdfs:subClassOf rdf:resource="http://www.buildingsmart-tech.org/ifcOWL/IFC2X3_Final#IfcDistributionControlElement"/>
        <rdfs:subClassOf rdf:resource="http://www.w3.org/ns/ssn/System"/>
        <rdfs:comment xml:lang="en">A sensor is a device that measures a physical quantity and converts it into a signal which can be read by an observer or by an instrument.</rdfs:comment>
        <rdfs:isDefinedBy xml:lang="en">http://ifcowl.openbimstandards.org/IFC4_ADD2/index.html#IfcSensor</rdfs:isDefinedBy>
        <rdfs:label xml:lang="en">IfcSensor</rdfs:label>
    </owl:Class>
    


    <!-- http://ifcowl.openbimstandards.org/IFC4_ADD2/index.html#IfcSolarDevice -->

    <owl:Class rdf:about="http://ifcowl.openbimstandards.org/IFC4_ADD2/index.html#IfcSolarDevice">
        <rdfs:subClassOf rdf:resource="http://www.buildingsmart-tech.org/ifcOWL/IFC2X3_Final#IfcEnergyConversionDevice"/>
        <rdfs:comment xml:lang="en">A solar device converts solar radiation into other energy such as electric current or thermal energy.</rdfs:comment>
        <rdfs:isDefinedBy xml:lang="en">http://ifcowl.openbimstandards.org/IFC4_ADD2/index.html#IfcSolarDevice</rdfs:isDefinedBy>
        <rdfs:label xml:lang="en">IfcSolarDevice</rdfs:label>
    </owl:Class>
    


    <!-- http://ifcowl.openbimstandards.org/IFC4_ADD2/index.html#IfcSpaceHeater -->

    <owl:Class rdf:about="http://ifcowl.openbimstandards.org/IFC4_ADD2/index.html#IfcSpaceHeater">
        <owl:equivalentClass rdf:resource="http://www.buildingsmart-tech.org/ifcOWL/IFC2X3_Final#IfcSpaceHeaterType"/>
        <rdfs:subClassOf rdf:resource="http://www.buildingsmart-tech.org/ifcOWL/IFC2X3_Final#IfcFlowTerminal"/>
        <rdfs:comment xml:lang="en">Space heaters utilize a combination of radiation and/or natural convection using a heating source such as electricity, steam or hot water to heat a limited space or area. Examples of space heaters include radiators, convectors, baseboard and finned-tube heaters.</rdfs:comment>
        <rdfs:isDefinedBy xml:lang="en">http://ifcowl.openbimstandards.org/IFC4_ADD2/index.html#IfcSpaceHeater</rdfs:isDefinedBy>
        <rdfs:label xml:lang="en">IfcSpaceHeater</rdfs:label>
    </owl:Class>
    


    <!-- http://ifcowl.openbimstandards.org/IFC4_ADD2/index.html#IfcStackTerminal -->

    <owl:Class rdf:about="http://ifcowl.openbimstandards.org/IFC4_ADD2/index.html#IfcStackTerminal">
        <owl:equivalentClass rdf:resource="http://www.buildingsmart-tech.org/ifcOWL/IFC2X3_Final#IfcStackTerminalType"/>
        <rdfs:subClassOf rdf:resource="http://www.buildingsmart-tech.org/ifcOWL/IFC2X3_Final#IfcFlowTerminal"/>
        <rdfs:comment xml:lang="en">A stack terminal is placed at the top of a ventilating stack (such as to prevent ingress by birds or rainwater) or rainwater pipe (to act as a collector or hopper for discharge from guttering).</rdfs:comment>
        <rdfs:isDefinedBy xml:lang="en">http://ifcowl.openbimstandards.org/IFC4_ADD2/index.html#IfcStackTerminal</rdfs:isDefinedBy>
        <rdfs:label xml:lang="en">IfcStackTerminal</rdfs:label>
    </owl:Class>
    


    <!-- http://ifcowl.openbimstandards.org/IFC4_ADD2/index.html#IfcTank -->

    <owl:Class rdf:about="http://ifcowl.openbimstandards.org/IFC4_ADD2/index.html#IfcTank">
        <owl:equivalentClass rdf:resource="http://www.buildingsmart-tech.org/ifcOWL/IFC2X3_Final#IfcTankType"/>
        <rdfs:subClassOf rdf:resource="http://www.buildingsmart-tech.org/ifcOWL/IFC2X3_Final#IfcFlowStorageDevice"/>
        <rdfs:comment xml:lang="en">A tank is a vessel or container in which a fluid or gas is stored for later use.</rdfs:comment>
        <rdfs:isDefinedBy xml:lang="en">http://ifcowl.openbimstandards.org/IFC4_ADD2/index.html#IfcTank</rdfs:isDefinedBy>
        <rdfs:label xml:lang="en">IfcTank</rdfs:label>
    </owl:Class>
    


    <!-- http://ifcowl.openbimstandards.org/IFC4_ADD2/index.html#IfcTransformer -->

    <owl:Class rdf:about="http://ifcowl.openbimstandards.org/IFC4_ADD2/index.html#IfcTransformer">
        <owl:equivalentClass rdf:resource="http://www.buildingsmart-tech.org/ifcOWL/IFC2X3_Final#IfcTransformerType"/>
        <rdfs:subClassOf rdf:resource="http://www.buildingsmart-tech.org/ifcOWL/IFC2X3_Final#IfcEnergyConversionDevice"/>
        <rdfs:comment xml:lang="en">A transformer is an inductive stationary device that transfers electrical energy from one circuit to another.
IfcTransformer is used to transform electric power; conversion of electric signals for other purposes is handled at other entities: IfcController converts arbitrary signals, IfcAudioVisualAppliance converts signals for audio or video streams, and IfcCommunicationsAppliance converts signals for data or other communications usage.</rdfs:comment>
        <rdfs:isDefinedBy xml:lang="en">http://ifcowl.openbimstandards.org/IFC4_ADD2/index.html#IfcTransformer</rdfs:isDefinedBy>
        <rdfs:label xml:lang="en">IfcTransformer</rdfs:label>
    </owl:Class>
    


    <!-- http://ifcowl.openbimstandards.org/IFC4_ADD2/index.html#IfcUnitaryControlElement -->

    <owl:Class rdf:about="http://ifcowl.openbimstandards.org/IFC4_ADD2/index.html#IfcUnitaryControlElement">
        <owl:equivalentClass rdf:resource="http://www.buildingsmart-tech.org/ifcOWL/IFC2X3_Final#IfcUnitaryControlElementType"/>
        <rdfs:subClassOf rdf:resource="http://www.buildingsmart-tech.org/ifcOWL/IFC2X3_Final#IfcDistributionControlElement"/>
        <rdfs:comment xml:lang="en">A unitary control element combines a number of control components into a single product, such as a thermostat or humidistat.
A unitary control element provides a housing for an aggregation of control or electrical distribution elements that, in combination, perform a singular (unitary) purpose. Each item in the aggregation may have its own geometric representation and location.</rdfs:comment>
        <rdfs:isDefinedBy xml:lang="en">http://ifcowl.openbimstandards.org/IFC4_ADD2/index.html#IfcUnitaryControlElement</rdfs:isDefinedBy>
        <rdfs:label xml:lang="en">IfcUnitaryControlElement</rdfs:label>
    </owl:Class>
    


    <!-- http://ifcowl.openbimstandards.org/IFC4_ADD2/index.html#IfcValve -->

    <owl:Class rdf:about="http://ifcowl.openbimstandards.org/IFC4_ADD2/index.html#IfcValve">
        <owl:equivalentClass rdf:resource="http://www.buildingsmart-tech.org/ifcOWL/IFC2X3_Final#IfcValveType"/>
        <rdfs:subClassOf rdf:resource="http://www.buildingsmart-tech.org/ifcOWL/IFC2X3_Final#IfcFlowController"/>
        <rdfs:comment xml:lang="en">IfcValve defines the occurrence of any valve; common information about valve types is handled by IfcValveType. The IfcValveType (if present) may establish the common type name, usage (predefined type), properties, materials, ports, composition, assignments, and representations. The IfcValveType is attached using the IfcRelDefinesByType objectified relationship and is accessible by the IsTypedBy inverse attribute.</rdfs:comment>
        <rdfs:isDefinedBy xml:lang="en">http://ifcowl.openbimstandards.org/IFC4_ADD2/index.html#IfcValve</rdfs:isDefinedBy>
        <rdfs:label xml:lang="en">IfcValve</rdfs:label>
    </owl:Class>
    


    <!-- http://ifcowl.openbimstandards.org/IFC4_ADD2/index.html#IfcVibrationIsolator -->

    <owl:Class rdf:about="http://ifcowl.openbimstandards.org/IFC4_ADD2/index.html#IfcVibrationIsolator">
        <owl:equivalentClass rdf:resource="http://www.buildingsmart-tech.org/ifcOWL/IFC2X3_Final#IfcVibrationIsolatorType"/>
        <rdfs:subClassOf rdf:resource="http://www.buildingsmart-tech.org/ifcOWL/IFC2X3_Final#IfcElementComponent"/>
        <rdfs:comment xml:lang="en">A vibration isolator is a device used to minimize the effects of vibration transmissibility in a building.</rdfs:comment>
        <rdfs:isDefinedBy xml:lang="en">http://ifcowl.openbimstandards.org/IFC4_ADD2/index.html#IfcVibrationIsolator</rdfs:isDefinedBy>
        <rdfs:label xml:lang="en">IfcVibrationIsolator</rdfs:label>
    </owl:Class>
    


    <!-- http://ifcowl.openbimstandards.org/IFC4_ADD2/index.html#IfcWasteTerminal -->

    <owl:Class rdf:about="http://ifcowl.openbimstandards.org/IFC4_ADD2/index.html#IfcWasteTerminal">
        <owl:equivalentClass rdf:resource="http://www.buildingsmart-tech.org/ifcOWL/IFC2X3_Final#IfcWasteTerminalType"/>
        <rdfs:subClassOf rdf:resource="http://www.buildingsmart-tech.org/ifcOWL/IFC2X3_Final#IfcFlowTerminal"/>
        <rdfs:comment xml:lang="en">IfcWasteTerminal defines the occurrence of any waste terminal; common information about waste terminal types is handled by IfcWasteTerminalType. The IfcWasteTerminalType (if present) may establish the common type name, usage (predefined type), properties, materials, ports, composition, assignments, and representations. The IfcWasteTerminalType is attached using the IfcRelDefinesByType objectified relationship and is accessible by the IsTypedBy inverse attribute.</rdfs:comment>
        <rdfs:isDefinedBy xml:lang="en">http://ifcowl.openbimstandards.org/IFC4_ADD2/index.html#IfcWasteTerminal</rdfs:isDefinedBy>
        <rdfs:label xml:lang="en">IfcWasteTerminal</rdfs:label>
    </owl:Class>
    


    <!-- http://www.buildingsmart-tech.org/ifcOWL/IFC2X3_Final#IfcActuatorType -->

    <owl:Class rdf:about="http://www.buildingsmart-tech.org/ifcOWL/IFC2X3_Final#IfcActuatorType">
        <rdfs:subClassOf rdf:resource="http://hit2gap.eu/h2g/h2gBA#Monitoring"/>
        <rdfs:subClassOf rdf:resource="http://www.buildingsmart-tech.org/ifcOWL/IFC2X3_Final#IfcDistributionControlElement"/>
        <rdfs:subClassOf>
            <owl:Restriction>
                <owl:onProperty rdf:resource="http://hit2gap.eu/h2g/h2gBI#OpenClose"/>
                <owl:allValuesFrom rdf:resource="http://hit2gap.eu/h2g/h2gBI#WindowCovering"/>
            </owl:Restriction>
        </rdfs:subClassOf>
        <rdfs:subClassOf>
            <owl:Restriction>
                <owl:onProperty rdf:resource="http://hit2gap.eu/h2g/h2gBI#OpenClose"/>
                <owl:allValuesFrom rdf:resource="http://www.buildingsmart-tech.org/ifcOWL/IFC2X3_Final#IfcWindow"/>
            </owl:Restriction>
        </rdfs:subClassOf>
        <rdfs:comment xml:lang="en">IfcActuatorType is defined in IFC2X3. We made it equivalent to IfcActuator defined in IFC4.</rdfs:comment>
        <rdfs:isDefinedBy xml:lang="en">http://www.buildingsmart-tech.org/ifcOWL/IFC2X3_Final#IfcActuatorType</rdfs:isDefinedBy>
        <rdfs:label xml:lang="en">IfcActuatorType</rdfs:label>
    </owl:Class>
    


    <!-- http://www.buildingsmart-tech.org/ifcOWL/IFC2X3_Final#IfcAirToAirHeatRecoveryType -->

    <owl:Class rdf:about="http://www.buildingsmart-tech.org/ifcOWL/IFC2X3_Final#IfcAirToAirHeatRecoveryType">
        <rdfs:subClassOf rdf:resource="http://www.buildingsmart-tech.org/ifcOWL/IFC2X3_Final#IfcEnergyConversionDevice"/>
        <rdfs:comment xml:lang="en">IfcAirToAirHeatRecoveryType is defined in IFC2X3. We made it equivalent to IfcAirToAirHeatRecovery defined in IFC4.</rdfs:comment>
        <rdfs:isDefinedBy xml:lang="en">http://www.buildingsmart-tech.org/ifcOWL/IFC2X3_Final#IfcAirToAirHeatRecoveryType</rdfs:isDefinedBy>
        <rdfs:label xml:lang="en">IfcAirToAirHeatRecoverType</rdfs:label>
    </owl:Class>
    


    <!-- http://www.buildingsmart-tech.org/ifcOWL/IFC2X3_Final#IfcAlarmType -->

    <owl:Class rdf:about="http://www.buildingsmart-tech.org/ifcOWL/IFC2X3_Final#IfcAlarmType">
        <rdfs:subClassOf rdf:resource="http://hit2gap.eu/h2g/h2gBA#Monitoring"/>
        <rdfs:subClassOf rdf:resource="http://www.buildingsmart-tech.org/ifcOWL/IFC2X3_Final#IfcDistributionControlElement"/>
        <rdfs:comment xml:lang="en">IfcAlarmType is defined in IFC2X3. We made it equivalent to IfcAlarm defined in IFC4.</rdfs:comment>
        <rdfs:isDefinedBy xml:lang="en">http://www.buildingsmart-tech.org/ifcOWL/IFC2X3_Final#IfcAlarmType</rdfs:isDefinedBy>
        <rdfs:label xml:lang="en">IfcAlarmType</rdfs:label>
    </owl:Class>
    


    <!-- http://www.buildingsmart-tech.org/ifcOWL/IFC2X3_Final#IfcBeam -->

    <owl:Class rdf:about="http://www.buildingsmart-tech.org/ifcOWL/IFC2X3_Final#IfcBeam">
        <rdfs:subClassOf rdf:resource="http://www.buildingsmart-tech.org/ifcOWL/IFC2X3_Final#IfcBuildingElement"/>
        <rdfs:comment xml:lang="en">An IfcBeam is a horizontal, or nearly horizontal, structural member. It represents such a member from an architectural point of view. It is not required to be load bearing.</rdfs:comment>
        <rdfs:isDefinedBy rdf:resource="http://www.buildingsmart-tech.org/ifcOWL/IFC2X3_Final#IfcBeam"/>
        <rdfs:label xml:lang="en">IfcBeam</rdfs:label>
    </owl:Class>
    


    <!-- http://www.buildingsmart-tech.org/ifcOWL/IFC2X3_Final#IfcBoilerType -->

    <owl:Class rdf:about="http://www.buildingsmart-tech.org/ifcOWL/IFC2X3_Final#IfcBoilerType">
        <rdfs:subClassOf rdf:resource="http://www.buildingsmart-tech.org/ifcOWL/IFC2X3_Final#IfcEnergyConversionDevice"/>
        <rdfs:comment xml:lang="en">IfcBoilerType is defined in IFC2X3. We made it equivalent to IfcBoiler defined in IFC4.</rdfs:comment>
        <rdfs:isDefinedBy xml:lang="en">http://www.buildingsmart-tech.org/ifcOWL/IFC2X3_Final#IfcBoilerType</rdfs:isDefinedBy>
        <rdfs:label xml:lang="en">IfcBoilerType</rdfs:label>
    </owl:Class>
    


    <!-- http://www.buildingsmart-tech.org/ifcOWL/IFC2X3_Final#IfcBuilding -->

    <owl:Class rdf:about="http://www.buildingsmart-tech.org/ifcOWL/IFC2X3_Final#IfcBuilding">
        <rdfs:subClassOf rdf:resource="http://www.buildingsmart-tech.org/ifcOWL/IFC2X3_Final#IfcSpatialStructureElement"/>
        <rdfs:subClassOf>
            <owl:Restriction>
                <owl:onProperty rdf:resource="http://hit2gap.eu/h2g/h2gBI#contains"/>
                <owl:someValuesFrom rdf:resource="http://www.buildingsmart-tech.org/ifcOWL/IFC2X3_Final#IfcBuilding"/>
            </owl:Restriction>
        </rdfs:subClassOf>
        <rdfs:subClassOf>
            <owl:Restriction>
                <owl:onProperty rdf:resource="http://hit2gap.eu/h2g/h2gBI#contains"/>
                <owl:someValuesFrom rdf:resource="http://www.buildingsmart-tech.org/ifcOWL/IFC2X3_Final#IfcBuildingStorey"/>
            </owl:Restriction>
        </rdfs:subClassOf>
        <rdfs:subClassOf>
            <owl:Restriction>
                <owl:onProperty rdf:resource="http://hit2gap.eu/h2g/h2gBI#contains"/>
                <owl:someValuesFrom rdf:resource="http://www.buildingsmart-tech.org/ifcOWL/IFC2X3_Final#IfcSpace"/>
            </owl:Restriction>
        </rdfs:subClassOf>
        <rdfs:subClassOf>
            <owl:Restriction>
                <owl:onProperty rdf:resource="http://hit2gap.eu/h2g/h2gBI#contains"/>
                <owl:someValuesFrom rdf:resource="http://www.buildingsmart-tech.org/ifcOWL/IFC2X3_Final#IfcSpatialZone"/>
            </owl:Restriction>
        </rdfs:subClassOf>
        <rdfs:subClassOf>
            <owl:Restriction>
                <owl:onProperty rdf:resource="http://hit2gap.eu/h2g/h2gBI#hasOrientation"/>
                <owl:allValuesFrom rdf:resource="http://hit2gap.eu/h2g/h2gBI#Orientation"/>
            </owl:Restriction>
        </rdfs:subClassOf>
        <rdfs:subClassOf>
            <owl:Restriction>
                <owl:onProperty rdf:resource="http://hit2gap.eu/h2g/h2gBI#isContainedIn"/>
                <owl:allValuesFrom rdf:resource="http://www.buildingsmart-tech.org/ifcOWL/IFC2X3_Final#IfcSite"/>
            </owl:Restriction>
        </rdfs:subClassOf>
        <rdfs:subClassOf>
            <owl:Restriction>
                <owl:onProperty rdf:resource="http://webprotege.stanford.edu/RbUxaH9qGAEuKzaa2RttSc"/>
                <owl:hasValue rdf:datatype="http://www.w3.org/2001/XMLSchema#string">qudt:Quantity</owl:hasValue>
            </owl:Restriction>
        </rdfs:subClassOf>
        <rdfs:comment xml:lang="en">A building represents a structure that provides shelter for its occupants or contents and stands in one place. The building is also used to provide a basic element within the spatial structure hierarchy for the components of a building project (together with site, storey, and space).</rdfs:comment>
        <rdfs:isDefinedBy rdf:resource="http://www.buildingsmart-tech.org/ifcOWL/IFC2X3_Final#IfcBuilding"/>
        <rdfs:isDefinedBy xml:lang="en">http://www.buildingsmart-tech.org/ifcOWL/IFC2X3_Final#IfcBuilding</rdfs:isDefinedBy>
        <rdfs:label xml:lang="en">IfcBuilding</rdfs:label>
    </owl:Class>
    


    <!-- http://www.buildingsmart-tech.org/ifcOWL/IFC2X3_Final#IfcBuildingElement -->

    <owl:Class rdf:about="http://www.buildingsmart-tech.org/ifcOWL/IFC2X3_Final#IfcBuildingElement">
        <rdfs:subClassOf rdf:resource="http://www.buildingsmart-tech.org/ifcOWL/IFC2X3_Final#IfcElement"/>
        <rdfs:subClassOf>
            <owl:Restriction>
                <owl:onProperty rdf:resource="http://hit2gap.eu/h2g/h2gBI#contains"/>
                <owl:someValuesFrom rdf:resource="http://www.buildingsmart-tech.org/ifcOWL/IFC2X3_Final#IfcBuildingElement"/>
            </owl:Restriction>
        </rdfs:subClassOf>
        <rdfs:subClassOf>
            <owl:Restriction>
                <owl:onProperty rdf:resource="http://hit2gap.eu/h2g/h2gBI#inContactWith"/>
                <owl:someValuesFrom rdf:resource="http://www.buildingsmart-tech.org/ifcOWL/IFC2X3_Final#IfcSpatialElement"/>
            </owl:Restriction>
        </rdfs:subClassOf>
        <rdfs:subClassOf>
            <owl:Restriction>
                <owl:onProperty rdf:resource="http://hit2gap.eu/h2g/h2gBI#isContainedIn"/>
                <owl:someValuesFrom rdf:resource="http://www.buildingsmart-tech.org/ifcOWL/IFC2X3_Final#IfcSpatialElement"/>
            </owl:Restriction>
        </rdfs:subClassOf>
        <rdfs:comment rdf:resource="http://www.buildingsmart-tech.org/ifcOWL/IFC2X3_Final#IfcBuildingElement"/>
        <rdfs:comment xml:lang="en">The building element comprises all elements that are primarily part of the construction of a building, i.e., its structural and space separating system.

EXAMPLEs of building elements are walls, beams, or doors, they are all physically existent and tangible things</rdfs:comment>
        <rdfs:label xml:lang="en">IfcBuildingElement</rdfs:label>
    </owl:Class>
    


    <!-- http://www.buildingsmart-tech.org/ifcOWL/IFC2X3_Final#IfcBuildingStorey -->

    <owl:Class rdf:about="http://www.buildingsmart-tech.org/ifcOWL/IFC2X3_Final#IfcBuildingStorey">
        <rdfs:subClassOf rdf:resource="http://www.buildingsmart-tech.org/ifcOWL/IFC2X3_Final#IfcSpatialStructureElement"/>
        <rdfs:subClassOf>
            <owl:Restriction>
                <owl:onProperty rdf:resource="http://hit2gap.eu/h2g/h2gBI#contains"/>
                <owl:someValuesFrom rdf:resource="http://www.buildingsmart-tech.org/ifcOWL/IFC2X3_Final#IfcSpace"/>
            </owl:Restriction>
        </rdfs:subClassOf>
        <rdfs:subClassOf>
            <owl:Restriction>
                <owl:onProperty rdf:resource="http://hit2gap.eu/h2g/h2gBI#isContainedIn"/>
                <owl:allValuesFrom rdf:resource="http://www.buildingsmart-tech.org/ifcOWL/IFC2X3_Final#IfcBuilding"/>
            </owl:Restriction>
        </rdfs:subClassOf>
        <rdfs:subClassOf>
            <owl:Restriction>
                <owl:onProperty rdf:resource="http://www.buildingsmart-tech.org/ifcOWL/IFC2X3_TC1#elevation_IfcBuildingStorey"/>
                <owl:allValuesFrom rdf:resource="http://www.buildingsmart-tech.org/ifcOWL/IFC2X3_TC1#IfcLengthMeasure"/>
            </owl:Restriction>
        </rdfs:subClassOf>
        <rdfs:subClassOf>
            <owl:Restriction>
                <owl:onProperty rdf:resource="http://www.buildingsmart-tech.org/ifcOWL/IFC2X3_TC1#elevation_IfcBuildingStorey"/>
                <owl:maxQualifiedCardinality rdf:datatype="http://www.w3.org/2001/XMLSchema#nonNegativeInteger">1</owl:maxQualifiedCardinality>
                <owl:onClass rdf:resource="http://www.buildingsmart-tech.org/ifcOWL/IFC2X3_TC1#IfcLengthMeasure"/>
            </owl:Restriction>
        </rdfs:subClassOf>
        <rdfs:comment xml:lang="en">The building storey has an elevation and typically represents a (nearly) horizontal aggregation of spaces that are vertically bound.

A storey is (if specified) associated to a building. A storey may span over several connected storeys. Therefore storey complex provides for a collection of storeys included in a building. A storey can also be decomposed in (horizontal) parts, where each part defines a partial storey. This is defined by the composition type attribute of the supertype IfcSpatialStructureElements which is interpreted as follow:

COMPLEX = building storey complex
ELEMENT = building storey
PARTIAL = partial building storey

EXAMPLE: In split level houses, a storey is split into two or more partial storeys, each with a different elevation. It can be handled by defining a storey, which includes two or more partial storeys with the individual elevations.</rdfs:comment>
        <rdfs:isDefinedBy rdf:resource="http://www.buildingsmart-tech.org/ifcOWL/IFC2X3_Final#IfcBuildingStorey"/>
        <rdfs:label xml:lang="en">IfcBuildingStorey</rdfs:label>
    </owl:Class>
    


    <!-- http://www.buildingsmart-tech.org/ifcOWL/IFC2X3_Final#IfcChillerType -->

    <owl:Class rdf:about="http://www.buildingsmart-tech.org/ifcOWL/IFC2X3_Final#IfcChillerType">
        <rdfs:subClassOf rdf:resource="http://www.buildingsmart-tech.org/ifcOWL/IFC2X3_Final#IfcEnergyConversionDevice"/>
        <rdfs:comment xml:lang="en">IfcChillerType is defined in IFC2X3. We made it equivalent to IfcChiller defined in IFC4.</rdfs:comment>
        <rdfs:isDefinedBy xml:lang="en">http://www.buildingsmart-tech.org/ifcOWL/IFC2X3_Final#IfcChillerType</rdfs:isDefinedBy>
        <rdfs:label xml:lang="en">IfcChillerType</rdfs:label>
    </owl:Class>
    


    <!-- http://www.buildingsmart-tech.org/ifcOWL/IFC2X3_Final#IfcChimmey -->

    <owl:Class rdf:about="http://www.buildingsmart-tech.org/ifcOWL/IFC2X3_Final#IfcChimmey">
        <rdfs:subClassOf rdf:resource="http://www.buildingsmart-tech.org/ifcOWL/IFC2X3_Final#IfcBuildingElement"/>
        <rdfs:comment xml:lang="en">Chimneys are typically vertical, or as near as vertical, parts of the construction of a building and part of the building fabric. Often constructed by pre-cast or insitu concrete, today seldom by bricks.</rdfs:comment>
        <rdfs:isDefinedBy rdf:resource="http://www.buildingsmart-tech.org/ifcOWL/IFC2X3_Final#IfcChimmey"/>
        <rdfs:label xml:lang="en">IfcChimmey</rdfs:label>
    </owl:Class>
    


    <!-- http://www.buildingsmart-tech.org/ifcOWL/IFC2X3_Final#IfcCoilType -->

    <owl:Class rdf:about="http://www.buildingsmart-tech.org/ifcOWL/IFC2X3_Final#IfcCoilType">
        <rdfs:subClassOf rdf:resource="http://www.buildingsmart-tech.org/ifcOWL/IFC2X3_Final#IfcEnergyConversionDevice"/>
        <rdfs:comment xml:lang="en">IfcCoilType is defined in IFC2X3. We made it equivalent to IfcCoil defined in IFC4.</rdfs:comment>
        <rdfs:isDefinedBy xml:lang="en">http://www.buildingsmart-tech.org/ifcOWL/IFC2X3_Final#IfcCoilType</rdfs:isDefinedBy>
        <rdfs:label xml:lang="en">IfcCoilType</rdfs:label>
    </owl:Class>
    


    <!-- http://www.buildingsmart-tech.org/ifcOWL/IFC2X3_Final#IfcColumn -->

    <owl:Class rdf:about="http://www.buildingsmart-tech.org/ifcOWL/IFC2X3_Final#IfcColumn">
        <rdfs:subClassOf rdf:resource="http://www.buildingsmart-tech.org/ifcOWL/IFC2X3_Final#IfcBuildingElement"/>
        <rdfs:comment xml:lang="en">An IfcColumn is a vertical structural member which often is aligned with a structural grid intersection. It represents a vertical, or nearly vertical, structural member from an architectural point of view. It is not required to be load bearing.</rdfs:comment>
        <rdfs:isDefinedBy rdf:resource="http://www.buildingsmart-tech.org/ifcOWL/IFC2X3_Final#IfcColumn"/>
        <rdfs:label xml:lang="en">IfcColumn</rdfs:label>
    </owl:Class>
    


    <!-- http://www.buildingsmart-tech.org/ifcOWL/IFC2X3_Final#IfcCompressorType -->

    <owl:Class rdf:about="http://www.buildingsmart-tech.org/ifcOWL/IFC2X3_Final#IfcCompressorType">
        <rdfs:subClassOf rdf:resource="http://www.buildingsmart-tech.org/ifcOWL/IFC2X3_Final#IfcFlowMovingDevice"/>
        <rdfs:comment xml:lang="en">IfcCompressorType is defined in IFC2X3. We made it equivalent to IfcCompressor defined in IFC4.</rdfs:comment>
        <rdfs:isDefinedBy xml:lang="en">http://www.buildingsmart-tech.org/ifcOWL/IFC2X3_Final#IfcCompressorType</rdfs:isDefinedBy>
        <rdfs:label xml:lang="en">IfcCompressorType</rdfs:label>
    </owl:Class>
    


    <!-- http://www.buildingsmart-tech.org/ifcOWL/IFC2X3_Final#IfcCondenserType -->

    <owl:Class rdf:about="http://www.buildingsmart-tech.org/ifcOWL/IFC2X3_Final#IfcCondenserType">
        <rdfs:subClassOf rdf:resource="http://www.buildingsmart-tech.org/ifcOWL/IFC2X3_Final#IfcEnergyConversionDevice"/>
        <rdfs:comment xml:lang="en">IfcCondenserType is defined in IFC2X3. We made it equivalent to IfcCondenser defined in IFC4.</rdfs:comment>
        <rdfs:isDefinedBy xml:lang="en">http://www.buildingsmart-tech.org/ifcOWL/IFC2X3_Final#IfcCondenserType</rdfs:isDefinedBy>
        <rdfs:label xml:lang="en">IfcCondenserType</rdfs:label>
    </owl:Class>
    


    <!-- http://www.buildingsmart-tech.org/ifcOWL/IFC2X3_Final#IfcCoolingTowerType -->

    <owl:Class rdf:about="http://www.buildingsmart-tech.org/ifcOWL/IFC2X3_Final#IfcCoolingTowerType">
        <rdfs:subClassOf rdf:resource="http://www.buildingsmart-tech.org/ifcOWL/IFC2X3_Final#IfcEnergyConversionDevice"/>
        <rdfs:comment xml:lang="en">IfcCoolingTowerType is defined in IFC2X3. We made it equivalent to IfcCoolingTower defined in IFC4.</rdfs:comment>
        <rdfs:isDefinedBy xml:lang="en">http://www.buildingsmart-tech.org/ifcOWL/IFC2X3_Final#IfcCoolingTowerType</rdfs:isDefinedBy>
        <rdfs:label xml:lang="en">IfcCoolingTowerType</rdfs:label>
    </owl:Class>
    


    <!-- http://www.buildingsmart-tech.org/ifcOWL/IFC2X3_Final#IfcCovering -->

    <owl:Class rdf:about="http://www.buildingsmart-tech.org/ifcOWL/IFC2X3_Final#IfcCovering">
        <rdfs:subClassOf rdf:resource="http://www.buildingsmart-tech.org/ifcOWL/IFC2X3_Final#IfcBuildingElement"/>
        <rdfs:comment xml:lang="en">A covering is an element which covers some part of another element and is fully dependent on that other element. The IfcCovering defines the occurrence of a covering type, that (if given) is expressed by the IfcCoveringType.

EXAMPLEs include wall claddings, floorings and suspended ceilings as well as finish trim and base molding.</rdfs:comment>
        <rdfs:isDefinedBy rdf:resource="http://www.buildingsmart-tech.org/ifcOWL/IFC2X3_Final#IfcCovering"/>
        <rdfs:label xml:lang="en">IfcCovering</rdfs:label>
    </owl:Class>
    


    <!-- http://www.buildingsmart-tech.org/ifcOWL/IFC2X3_Final#IfcCurtainWall -->

    <owl:Class rdf:about="http://www.buildingsmart-tech.org/ifcOWL/IFC2X3_Final#IfcCurtainWall">
        <rdfs:subClassOf rdf:resource="http://www.buildingsmart-tech.org/ifcOWL/IFC2X3_Final#IfcBuildingElement"/>
        <rdfs:comment xml:lang="en">Exterior wall of a building which is an assembly of components, hung from the edge of the floor/roof structure rather than bearing on a floor</rdfs:comment>
        <rdfs:isDefinedBy rdf:resource="http://www.buildingsmart-tech.org/ifcOWL/IFC2X3_Final#IfcCurtainWall"/>
        <rdfs:label xml:lang="en">IfcCurtainWall</rdfs:label>
    </owl:Class>
    


    <!-- http://www.buildingsmart-tech.org/ifcOWL/IFC2X3_Final#IfcDamperType -->

    <owl:Class rdf:about="http://www.buildingsmart-tech.org/ifcOWL/IFC2X3_Final#IfcDamperType">
        <rdfs:subClassOf rdf:resource="http://www.buildingsmart-tech.org/ifcOWL/IFC2X3_Final#IfcFlowController"/>
        <rdfs:comment xml:lang="en">IfcDamperType is defined in IFC2X3. We made it equivalent to IfcDamper defined in IFC4.</rdfs:comment>
        <rdfs:isDefinedBy xml:lang="en">http://www.buildingsmart-tech.org/ifcOWL/IFC2X3_Final#IfcDamperType</rdfs:isDefinedBy>
        <rdfs:label xml:lang="en">IfcDamperType</rdfs:label>
    </owl:Class>
    


    <!-- http://www.buildingsmart-tech.org/ifcOWL/IFC2X3_Final#IfcDistributionCircuit -->

    <owl:Class rdf:about="http://www.buildingsmart-tech.org/ifcOWL/IFC2X3_Final#IfcDistributionCircuit">
        <rdfs:subClassOf rdf:resource="http://hit2gap.eu/ontomg#InfraBranch"/>
        <rdfs:subClassOf rdf:resource="http://www.buildingsmart-tech.org/ifcOWL/IFC2X3_Final#IfcDistributionSystem"/>
        <rdfs:comment xml:lang="en">A distribution circuit is a partition of a distribution system that is conditionally switched such as an electrical circuit.</rdfs:comment>
        <rdfs:isDefinedBy xml:lang="en">http://www.buildingsmart-tech.org/ifcOWL/IFC2X3_Final#IfcDistributionCircuit</rdfs:isDefinedBy>
        <rdfs:label xml:lang="en">IfcDistributionCircuit</rdfs:label>
    </owl:Class>
    


    <!-- http://www.buildingsmart-tech.org/ifcOWL/IFC2X3_Final#IfcDistributionControlElement -->

    <owl:Class rdf:about="http://www.buildingsmart-tech.org/ifcOWL/IFC2X3_Final#IfcDistributionControlElement">
        <rdfs:subClassOf rdf:resource="http://www.buildingsmart-tech.org/ifcOWL/IFC2X3_Final#IfcDistributionElement"/>
        <rdfs:comment rdf:resource="http://www.buildingsmart-tech.org/ifcOWL/IFC2X3_Final#IfcDistributionControlElement"/>
        <rdfs:comment xml:lang="en">IfcDistributionControlElement defines occurrence elements of a building automation control system that are used to impart control over elements of a distribution system.</rdfs:comment>
        <rdfs:label xml:lang="en">IfcDistributionControlElement</rdfs:label>
    </owl:Class>
    


    <!-- http://www.buildingsmart-tech.org/ifcOWL/IFC2X3_Final#IfcDistributionElement -->

    <owl:Class rdf:about="http://www.buildingsmart-tech.org/ifcOWL/IFC2X3_Final#IfcDistributionElement">
        <rdfs:subClassOf rdf:resource="http://hit2gap.eu/ontomg#ELBranch"/>
        <rdfs:subClassOf rdf:resource="http://hit2gap.eu/ontomg#ESBranch"/>
        <rdfs:subClassOf rdf:resource="http://www.buildingsmart-tech.org/ifcOWL/IFC2X3_Final#IfcElement"/>
        <rdfs:subClassOf>
            <owl:Restriction>
                <owl:onProperty rdf:resource="http://hit2gap.eu/h2g/h2gBI#contains"/>
                <owl:someValuesFrom rdf:resource="http://www.buildingsmart-tech.org/ifcOWL/IFC2X3_Final#IfcBuildingElement"/>
            </owl:Restriction>
        </rdfs:subClassOf>
        <rdfs:comment xml:lang="en">The IfcDistributionElement defines the occurrence of any HVAC, electrical, sanitary or other element within a distribution system. Common information about distribution element types (or styles) is handled by subtypes of IfcDistributionElementType. The IfcDistributionElementType (if present) may establish the common type name, usage (or predefined) type, common material, common set of properties and common shape representations (using IfcRepresentationMap).</rdfs:comment>
        <rdfs:isDefinedBy rdf:resource="http://www.buildingsmart-tech.org/ifcOWL/IFC2X3_Final#IfcDistributionElement"/>
        <rdfs:label xml:lang="en">IfcDistributionElement</rdfs:label>
    </owl:Class>
    


    <!-- http://www.buildingsmart-tech.org/ifcOWL/IFC2X3_Final#IfcDistributionFlowElement -->

    <owl:Class rdf:about="http://www.buildingsmart-tech.org/ifcOWL/IFC2X3_Final#IfcDistributionFlowElement">
        <rdfs:subClassOf rdf:resource="http://www.buildingsmart-tech.org/ifcOWL/IFC2X3_Final#IfcDistributionElement"/>
        <rdfs:comment rdf:resource="http://www.buildingsmart-tech.org/ifcOWL/IFC2X3_Final#IfcDistributionFlowElement"/>
        <rdfs:comment xml:lang="en">The distribution element IfcDistributionFlowElement defines occurrence elements of a distribution system that facilitate the distribution of energy or matter, such as air, water or power.

EXAMPLEs of distribution flow elements are ducts, pipes, wires, fittings, equipment, etc.

The IfcDistributionFlowElement defines the occurrence of a distribution element within the spatial context of a project.</rdfs:comment>
        <rdfs:label xml:lang="en">IfcDistributionFlowElement</rdfs:label>
    </owl:Class>
    


    <!-- http://www.buildingsmart-tech.org/ifcOWL/IFC2X3_Final#IfcDistributionSystem -->

    <owl:Class rdf:about="http://www.buildingsmart-tech.org/ifcOWL/IFC2X3_Final#IfcDistributionSystem">
        <rdfs:comment xml:lang="en">A distribution system is a network designed to receive, store, maintain, distribute, or control the flow of a distribution media. A common example is a heating hot water system that consists of a pump, a tank, and an interconnected piping system for distributing hot water to terminals.
The group IfcDistributionSystem defines the occurrence of a specialized system for use within the context of building services.
Important functionalities for the description of a distribution system are derived from existing IFC entities:

From IfcSystem it inherits the ability to couple the distribution system via IfcRelServicesBuildings to one or more IfcSpatialElement subtypes as necessary.

From IfcGroup it inherits the inverse attribute IsGroupedBy, pointing to the relationship entity IfcRelAssignsToGroup. This allows to group distribution elements (instances of IfcDistributionElement subtypes), and in special cases ports directly (instances of IfcDistributionPort).

From IfcObject it inherits the inverse attribute IsDecomposedBy pointing to the relationship entity IfcRelAggregates. It provides the hierarchy between the separate (partial) distribution systems. For example, an electrical main circuit may be aggregated into branch circuits.</rdfs:comment>
        <rdfs:isDefinedBy xml:lang="en">http://www.buildingsmart-tech.org/ifcOWL/IFC2X3_Final#IfcDistributionSystem</rdfs:isDefinedBy>
        <rdfs:label xml:lang="en">IfcDistributionSystem</rdfs:label>
    </owl:Class>
    


    <!-- http://www.buildingsmart-tech.org/ifcOWL/IFC2X3_Final#IfcDoor -->

    <owl:Class rdf:about="http://www.buildingsmart-tech.org/ifcOWL/IFC2X3_Final#IfcDoor">
        <rdfs:subClassOf rdf:resource="http://www.buildingsmart-tech.org/ifcOWL/IFC2X3_Final#IfcBuildingElement"/>
        <rdfs:comment xml:lang="en">The door is a building element that is predominately used to provide controlled access for people and goods. It includes constructions with hinged, pivoted, sliding, and additionally revolving and folding operations. A door consists of a lining and one or several panels, properties concerning the lining and panel are defined by the IfcDoorLiningProperties and the IfcDoorPanelProperties.

The door entity, IfcDoor, defines a particular occurrence of a door inserted in the spatial context of a project</rdfs:comment>
        <rdfs:isDefinedBy rdf:resource="http://www.buildingsmart-tech.org/ifcOWL/IFC2X3_Final#IfcDoor"/>
        <rdfs:label xml:lang="en">IfcDoor</rdfs:label>
    </owl:Class>
    


    <!-- http://www.buildingsmart-tech.org/ifcOWL/IFC2X3_Final#IfcElectricApplianceType -->

    <owl:Class rdf:about="http://www.buildingsmart-tech.org/ifcOWL/IFC2X3_Final#IfcElectricApplianceType">
        <rdfs:subClassOf rdf:resource="http://www.buildingsmart-tech.org/ifcOWL/IFC2X3_Final#IfcFlowTerminal"/>
        <rdfs:comment xml:lang="en">IfcElectricApplianceType is defined in IFC2X3. We made it equivalent to IfcElectricAppliance defined in IFC4.</rdfs:comment>
        <rdfs:isDefinedBy xml:lang="en">http://www.buildingsmart-tech.org/ifcOWL/IFC2X3_Final#IfcElectricApplianceType</rdfs:isDefinedBy>
        <rdfs:label xml:lang="en">IfcElectricApplianceType</rdfs:label>
    </owl:Class>
    


    <!-- http://www.buildingsmart-tech.org/ifcOWL/IFC2X3_Final#IfcElectricFlowStorageDeviceType -->

    <owl:Class rdf:about="http://www.buildingsmart-tech.org/ifcOWL/IFC2X3_Final#IfcElectricFlowStorageDeviceType">
        <rdfs:subClassOf rdf:resource="http://www.buildingsmart-tech.org/ifcOWL/IFC2X3_Final#IfcFlowStorageDevice"/>
        <rdfs:comment xml:lang="en">IfcElectricFlowStorageDeviceType is defined in IFC2X3. We made it equivalent to IfcElectricFlowStorageDevice defined in IFC4.</rdfs:comment>
        <rdfs:isDefinedBy xml:lang="en">http://www.buildingsmart-tech.org/ifcOWL/IFC2X3_Final#IfcElectricFlowStorageDeviceType</rdfs:isDefinedBy>
        <rdfs:label xml:lang="en">IfcElectricFlowStorageDeviceType</rdfs:label>
    </owl:Class>
    


    <!-- http://www.buildingsmart-tech.org/ifcOWL/IFC2X3_Final#IfcElectricGeneratorType -->

    <owl:Class rdf:about="http://www.buildingsmart-tech.org/ifcOWL/IFC2X3_Final#IfcElectricGeneratorType">
        <rdfs:subClassOf rdf:resource="http://www.buildingsmart-tech.org/ifcOWL/IFC2X3_Final#IfcEnergyConversionDevice"/>
        <rdfs:comment xml:lang="en">IfcElectricGeneratorType is defined in IFC2X3. We made it equivalent to IfcElectricGenerator defined in IFC4.</rdfs:comment>
        <rdfs:isDefinedBy xml:lang="en">http://www.buildingsmart-tech.org/ifcOWL/IFC2X3_Final#IfcElectricGeneratorType</rdfs:isDefinedBy>
        <rdfs:label xml:lang="en">IfcElectricGeneratorType</rdfs:label>
    </owl:Class>
    


    <!-- http://www.buildingsmart-tech.org/ifcOWL/IFC2X3_Final#IfcElectricMotorType -->

    <owl:Class rdf:about="http://www.buildingsmart-tech.org/ifcOWL/IFC2X3_Final#IfcElectricMotorType">
        <rdfs:subClassOf rdf:resource="http://www.buildingsmart-tech.org/ifcOWL/IFC2X3_Final#IfcEnergyConversionDevice"/>
        <rdfs:comment xml:lang="en">IfcElectricMotorType is defined in IFC2X3. We made it equivalent to IfcElectricMotor defined in IFC4.</rdfs:comment>
        <rdfs:isDefinedBy xml:lang="en">http://www.buildingsmart-tech.org/ifcOWL/IFC2X3_Final#IfcElectricMotorType</rdfs:isDefinedBy>
        <rdfs:label xml:lang="en">IfcElectricMotorType</rdfs:label>
    </owl:Class>
    


    <!-- http://www.buildingsmart-tech.org/ifcOWL/IFC2X3_Final#IfcElement -->

    <owl:Class rdf:about="http://www.buildingsmart-tech.org/ifcOWL/IFC2X3_Final#IfcElement">
        <rdfs:subClassOf rdf:resource="http://hit2gap.eu/h2g/h2gSensor#FeatureOfInterest"/>
        <rdfs:subClassOf rdf:resource="http://www.buildingsmart-tech.org/ifcOWL/IFC2X3_TC1#IfcRoot"/>
        <rdfs:comment xml:lang="en">An element is a generalization of all components that make up an AEC product.
Elements are physically existent objects, although they might be void elements, such as holes. Elements either remain permanently in the AEC product, or only temporarily, as formwork does. Elements can be either assembled on site or pre-manufactured and built in on site.</rdfs:comment>
        <rdfs:isDefinedBy rdf:resource="http://www.buildingsmart-tech.org/ifcOWL/IFC2X3_Final#IfcElement"/>
        <rdfs:label xml:lang="en">IfcElement</rdfs:label>
    </owl:Class>
    


    <!-- http://www.buildingsmart-tech.org/ifcOWL/IFC2X3_Final#IfcElementComponent -->

    <owl:Class rdf:about="http://www.buildingsmart-tech.org/ifcOWL/IFC2X3_Final#IfcElementComponent">
        <rdfs:subClassOf rdf:resource="http://www.buildingsmart-tech.org/ifcOWL/IFC2X3_Final#IfcElement"/>
        <rdfs:comment xml:lang="en">An element component is a representation for minor items included in, added to or connecting to or between elements, which usually are not of interest from the overall building structure viewpoint. However, these small parts may have vital and load carrying functions within the construction. These items do not provide any actual space boundaries. Typical examples of IfcElementComponents include different kinds of fasteners and various accessories.</rdfs:comment>
        <rdfs:isDefinedBy rdf:resource="http://www.buildingsmart-tech.org/ifcOWL/IFC2X3_Final#IfcElementComponent"/>
        <rdfs:label xml:lang="en">IfcElementComponent</rdfs:label>
    </owl:Class>
    


    <!-- http://www.buildingsmart-tech.org/ifcOWL/IFC2X3_Final#IfcEnergyConversionDevice -->

    <owl:Class rdf:about="http://www.buildingsmart-tech.org/ifcOWL/IFC2X3_Final#IfcEnergyConversionDevice">
        <rdfs:subClassOf rdf:resource="http://hit2gap.eu/h2g/h2gBA#StaticBuildingAppliance"/>
        <rdfs:subClassOf rdf:resource="http://hit2gap.eu/ontomg#ELBranch"/>
        <rdfs:subClassOf rdf:resource="http://www.buildingsmart-tech.org/ifcOWL/IFC2X3_Final#IfcDistributionFlowElement"/>
        <rdfs:subClassOf>
            <owl:Restriction>
                <owl:onProperty rdf:resource="http://hit2gap.eu/h2g/h2gBI#consumes"/>
                <owl:someValuesFrom rdf:resource="http://hit2gap.eu/h2g/h2gBI#PhysicalMedium"/>
            </owl:Restriction>
        </rdfs:subClassOf>
        <rdfs:subClassOf>
            <owl:Restriction>
                <owl:onProperty rdf:resource="http://hit2gap.eu/h2g/h2gBI#produces"/>
                <owl:someValuesFrom rdf:resource="http://hit2gap.eu/h2g/h2gBI#PhysicalMedium"/>
            </owl:Restriction>
        </rdfs:subClassOf>
        <rdfs:subClassOf>
            <owl:Restriction>
                <owl:onProperty rdf:resource="http://hit2gap.eu/h2g/h2gBI#InputOutput"/>
                <owl:allValuesFrom rdf:resource="http://www.buildingsmart-tech.org/ifcOWL/IFC2X3_Final#IfcZone"/>
            </owl:Restriction>
        </rdfs:subClassOf>
        <rdfs:comment xml:lang="en">IfcEnergyConversionDevice defines the occurrence of a device used to perform energy conversion or heat transfer and typically participates in a flow distribution system. Its type is defined by IfcEnergyConversionDeviceType or its subtypes.</rdfs:comment>
        <rdfs:isDefinedBy xml:lang="en">http://www.buildingsmart-tech.org/ifcOWL/IFC2X3_Final#IfcEnergyConversionDevice</rdfs:isDefinedBy>
        <rdfs:label xml:lang="en">IfcEnergyConversionDevice</rdfs:label>
    </owl:Class>
    


    <!-- http://www.buildingsmart-tech.org/ifcOWL/IFC2X3_Final#IfcEvaporativeCoolerType -->

    <owl:Class rdf:about="http://www.buildingsmart-tech.org/ifcOWL/IFC2X3_Final#IfcEvaporativeCoolerType">
        <rdfs:subClassOf rdf:resource="http://www.buildingsmart-tech.org/ifcOWL/IFC2X3_Final#IfcEnergyConversionDevice"/>
        <rdfs:comment xml:lang="en">IfcEvaporativeCoolerType is defined in IFC2X3. We made it equivalent to IfcEvaporativeCooler defined in IFC4.</rdfs:comment>
        <rdfs:isDefinedBy xml:lang="en">http://www.buildingsmart-tech.org/ifcOWL/IFC2X3_Final#IfcEvaporativeCoolerType</rdfs:isDefinedBy>
        <rdfs:label xml:lang="en">IfcEvaporativeCoolerType</rdfs:label>
    </owl:Class>
    


    <!-- http://www.buildingsmart-tech.org/ifcOWL/IFC2X3_Final#IfcEvaporatorType -->

    <owl:Class rdf:about="http://www.buildingsmart-tech.org/ifcOWL/IFC2X3_Final#IfcEvaporatorType">
        <rdfs:subClassOf rdf:resource="http://www.buildingsmart-tech.org/ifcOWL/IFC2X3_Final#IfcEnergyConversionDevice"/>
        <rdfs:comment xml:lang="en">IfcEvaporatorType is defined in IFC2X3. We made it equivalent to IfcEvaporator defined in IFC4.</rdfs:comment>
        <rdfs:isDefinedBy xml:lang="en">http://www.buildingsmart-tech.org/ifcOWL/IFC2X3_Final#IfcEvaporatorType</rdfs:isDefinedBy>
        <rdfs:label xml:lang="en">IfcEvaporatorType</rdfs:label>
    </owl:Class>
    


    <!-- http://www.buildingsmart-tech.org/ifcOWL/IFC2X3_Final#IfcFanType -->

    <owl:Class rdf:about="http://www.buildingsmart-tech.org/ifcOWL/IFC2X3_Final#IfcFanType">
        <rdfs:subClassOf rdf:resource="http://www.buildingsmart-tech.org/ifcOWL/IFC2X3_Final#IfcFlowMovingDevice"/>
        <rdfs:comment xml:lang="en">IfcFanType is defined in IFC2X3. We made it equivalent to IfcFan defined in IFC4.</rdfs:comment>
        <rdfs:isDefinedBy xml:lang="en">http://www.buildingsmart-tech.org/ifcOWL/IFC2X3_Final#IfcFanType</rdfs:isDefinedBy>
        <rdfs:label xml:lang="en">IfcFanType</rdfs:label>
    </owl:Class>
    


    <!-- http://www.buildingsmart-tech.org/ifcOWL/IFC2X3_Final#IfcFireSuppressionTerminalType -->

    <owl:Class rdf:about="http://www.buildingsmart-tech.org/ifcOWL/IFC2X3_Final#IfcFireSuppressionTerminalType">
        <rdfs:subClassOf rdf:resource="http://www.buildingsmart-tech.org/ifcOWL/IFC2X3_Final#IfcFlowTerminal"/>
        <rdfs:comment xml:lang="en">IfcFireSuppressionTerminalType is defined in IFC2X3. We made it equivalent to IfcFireSuppressionTerminal defined in IFC4.</rdfs:comment>
        <rdfs:isDefinedBy xml:lang="en">http://www.buildingsmart-tech.org/ifcOWL/IFC2X3_Final#IfcFireSuppressionTerminalType</rdfs:isDefinedBy>
        <rdfs:label xml:lang="en">IfcFireSuppressionTerminalType</rdfs:label>
    </owl:Class>
    


    <!-- http://www.buildingsmart-tech.org/ifcOWL/IFC2X3_Final#IfcFlowController -->

    <owl:Class rdf:about="http://www.buildingsmart-tech.org/ifcOWL/IFC2X3_Final#IfcFlowController">
        <rdfs:subClassOf rdf:resource="http://hit2gap.eu/h2g/h2gBA#StaticBuildingAppliance"/>
        <rdfs:subClassOf rdf:resource="http://hit2gap.eu/ontomg#BranchController"/>
        <rdfs:subClassOf rdf:resource="http://www.buildingsmart-tech.org/ifcOWL/IFC2X3_Final#IfcDistributionControlElement"/>
        <rdfs:subClassOf rdf:resource="http://www.buildingsmart-tech.org/ifcOWL/IFC2X3_Final#IfcDistributionFlowElement"/>
        <rdfs:subClassOf>
            <owl:Restriction>
                <owl:onProperty rdf:resource="http://hit2gap.eu/h2g/h2gBI#controls"/>
                <owl:someValuesFrom rdf:resource="http://hit2gap.eu/h2g/h2gBI#PhysicalMedium"/>
            </owl:Restriction>
        </rdfs:subClassOf>
        <rdfs:comment xml:lang="en">IfcFlowController defines the occurrence of elements of a distribution system that are used to regulate flow through a distribution system. Examples include dampers, valves, switches, and relays. Its type is defined by IfcFlowControllerType or subtypes.</rdfs:comment>
        <rdfs:isDefinedBy xml:lang="en">http://www.buildingsmart-tech.org/ifcOWL/IFC2X3_Final#IfcFlowController</rdfs:isDefinedBy>
        <rdfs:label xml:lang="en">IfcFlowController</rdfs:label>
    </owl:Class>
    


    <!-- http://www.buildingsmart-tech.org/ifcOWL/IFC2X3_Final#IfcFlowMovingDevice -->

    <owl:Class rdf:about="http://www.buildingsmart-tech.org/ifcOWL/IFC2X3_Final#IfcFlowMovingDevice">
        <rdfs:subClassOf rdf:resource="http://hit2gap.eu/h2g/h2gBA#StaticBuildingAppliance"/>
        <rdfs:subClassOf rdf:resource="http://hit2gap.eu/ontomg#ELBranch"/>
        <rdfs:subClassOf rdf:resource="http://www.buildingsmart-tech.org/ifcOWL/IFC2X3_Final#IfcDistributionFlowElement"/>
        <rdfs:subClassOf>
            <owl:Restriction>
                <owl:onProperty rdf:resource="http://hit2gap.eu/h2g/h2gBI#transports"/>
                <owl:someValuesFrom rdf:resource="http://hit2gap.eu/h2g/h2gBI#PhysicalMedium"/>
            </owl:Restriction>
        </rdfs:subClassOf>
        <rdfs:comment xml:lang="en">IfcFlowMovingDevice</rdfs:comment>
        <rdfs:comment xml:lang="en">IfcFlowMovingDevice defines the occurrence of an apparatus used to distribute, circulate, or perform conveyance of fluids, including liquids and gases (such as a pump or fan), and typically participates in a flow distribution system. Its type is defined by IfcFlowMovingDeviceType or its subtypes.</rdfs:comment>
        <rdfs:isDefinedBy xml:lang="en">http://www.buildingsmart-tech.org/ifcOWL/IFC2X3_Final#IfcFlowMovingDevice</rdfs:isDefinedBy>
    </owl:Class>
    


    <!-- http://www.buildingsmart-tech.org/ifcOWL/IFC2X3_Final#IfcFlowStorageDevice -->

    <owl:Class rdf:about="http://www.buildingsmart-tech.org/ifcOWL/IFC2X3_Final#IfcFlowStorageDevice">
        <rdfs:subClassOf rdf:resource="http://hit2gap.eu/h2g/h2gBA#StaticBuildingAppliance"/>
        <rdfs:subClassOf rdf:resource="http://www.buildingsmart-tech.org/ifcOWL/IFC2X3_Final#IfcDistributionFlowElement"/>
        <rdfs:subClassOf>
            <owl:Restriction>
                <owl:onProperty rdf:resource="http://hit2gap.eu/h2g/h2gBI#stores"/>
                <owl:someValuesFrom rdf:resource="http://hit2gap.eu/h2g/h2gBI#PhysicalMedium"/>
            </owl:Restriction>
        </rdfs:subClassOf>
        <rdfs:comment xml:lang="en">The distribution flow element IfcFlowStorageDevice defines the occurrence of a device that participates in a distribution system and is used for temporary storage (such as a tank). Its type is defined by IfcFlowStorageDeviceType or its subtypes.</rdfs:comment>
        <rdfs:isDefinedBy xml:lang="en">http://www.buildingsmart-tech.org/ifcOWL/IFC2X3_Final#IfcFlowStorageDevice</rdfs:isDefinedBy>
        <rdfs:label xml:lang="en">IfcFlowStorageDevice</rdfs:label>
    </owl:Class>
    


    <!-- http://www.buildingsmart-tech.org/ifcOWL/IFC2X3_Final#IfcFlowTerminal -->

    <owl:Class rdf:about="http://www.buildingsmart-tech.org/ifcOWL/IFC2X3_Final#IfcFlowTerminal">
        <rdfs:subClassOf rdf:resource="http://hit2gap.eu/h2g/h2gBA#StaticBuildingAppliance"/>
        <rdfs:subClassOf rdf:resource="http://www.buildingsmart-tech.org/ifcOWL/IFC2X3_Final#IfcDistributionFlowElement"/>
        <rdfs:subClassOf>
            <owl:Restriction>
                <owl:onProperty rdf:resource="http://hit2gap.eu/h2g/h2gBI#consumes"/>
                <owl:someValuesFrom rdf:resource="http://hit2gap.eu/h2g/h2gBI#PhysicalMedium"/>
            </owl:Restriction>
        </rdfs:subClassOf>
        <rdfs:comment xml:lang="en">The distribution flow element IfcFlowTerminal defines the occurrence of a permanently attached element that acts as a terminus or beginning of a distribution system (e.g., air outlet, drain, water closet, sink, etc.). A terminal is typically a point at which a system interfaces with an external environment. Its type is defined by IfcFlowTerminalType or its subtypes.</rdfs:comment>
        <rdfs:isDefinedBy xml:lang="en">http://www.buildingsmart-tech.org/ifcOWL/IFC2X3_Final#IfcFlowTerminal</rdfs:isDefinedBy>
        <rdfs:label xml:lang="en">IfcFlowTerminal</rdfs:label>
    </owl:Class>
    


    <!-- http://www.buildingsmart-tech.org/ifcOWL/IFC2X3_Final#IfcFlowTreatmentDevice -->

    <owl:Class rdf:about="http://www.buildingsmart-tech.org/ifcOWL/IFC2X3_Final#IfcFlowTreatmentDevice">
        <rdfs:subClassOf rdf:resource="http://hit2gap.eu/h2g/h2gBA#StaticBuildingAppliance"/>
        <rdfs:subClassOf rdf:resource="http://www.buildingsmart-tech.org/ifcOWL/IFC2X3_Final#IfcDistributionFlowElement"/>
        <rdfs:comment xml:lang="en">The distribution flow element IfcFlowTreatmentDevice defines the occurrence of a device typically used to remove unwanted matter from a fluid, either liquid or gas, and typically participates in a flow distribution system. Its type is defined by IfcFlowTreatmentDeviceType or its subtypes.</rdfs:comment>
        <rdfs:isDefinedBy xml:lang="en">http://www.buildingsmart-tech.org/ifcOWL/IFC2X3_Final#IfcFlowTreatmentDevice</rdfs:isDefinedBy>
        <rdfs:label xml:lang="en">IfcFlowTreatmentDevice</rdfs:label>
    </owl:Class>
    


    <!-- http://www.buildingsmart-tech.org/ifcOWL/IFC2X3_Final#IfcFooting -->

    <owl:Class rdf:about="http://www.buildingsmart-tech.org/ifcOWL/IFC2X3_Final#IfcFooting">
        <rdfs:subClassOf rdf:resource="http://www.buildingsmart-tech.org/ifcOWL/IFC2X3_Final#IfcBuildingElement"/>
        <rdfs:comment xml:lang="en">IfcFooting is a part of the foundation of a structure that spreads and transmits the load directly to the soil.</rdfs:comment>
        <rdfs:isDefinedBy rdf:resource="http://www.buildingsmart-tech.org/ifcOWL/IFC2X3_Final#IfcFooting"/>
        <rdfs:label xml:lang="en">IfcFooting</rdfs:label>
    </owl:Class>
    


    <!-- http://www.buildingsmart-tech.org/ifcOWL/IFC2X3_Final#IfcHeatExchangerType -->

    <owl:Class rdf:about="http://www.buildingsmart-tech.org/ifcOWL/IFC2X3_Final#IfcHeatExchangerType">
        <rdfs:subClassOf rdf:resource="http://www.buildingsmart-tech.org/ifcOWL/IFC2X3_Final#IfcEnergyConversionDevice"/>
        <rdfs:comment xml:lang="en">IfcHeatExchangerType is defined in IFC2X3. We made it equivalent to IfcHeatExchanger defined in IFC4.</rdfs:comment>
        <rdfs:isDefinedBy xml:lang="en">http://www.buildingsmart-tech.org/ifcOWL/IFC2X3_Final#IfcHeatExchangerType</rdfs:isDefinedBy>
        <rdfs:label xml:lang="en">IfcHeatExchangerType</rdfs:label>
    </owl:Class>
    


    <!-- http://www.buildingsmart-tech.org/ifcOWL/IFC2X3_Final#IfcHumidifierType -->

    <owl:Class rdf:about="http://www.buildingsmart-tech.org/ifcOWL/IFC2X3_Final#IfcHumidifierType">
        <rdfs:subClassOf rdf:resource="http://www.buildingsmart-tech.org/ifcOWL/IFC2X3_Final#IfcEnergyConversionDevice"/>
        <rdfs:comment xml:lang="en">IfcHumidifierType is defined in IFC2X3. We made it equivalent to IfcHumiidifier defined in IFC4.</rdfs:comment>
        <rdfs:isDefinedBy xml:lang="en">http://www.buildingsmart-tech.org/ifcOWL/IFC2X3_Final#IfcHumidifierType</rdfs:isDefinedBy>
        <rdfs:label xml:lang="en">IfcHumidifierType</rdfs:label>
    </owl:Class>
    


    <!-- http://www.buildingsmart-tech.org/ifcOWL/IFC2X3_Final#IfcLampType -->

    <owl:Class rdf:about="http://www.buildingsmart-tech.org/ifcOWL/IFC2X3_Final#IfcLampType">
        <rdfs:subClassOf rdf:resource="http://www.buildingsmart-tech.org/ifcOWL/IFC2X3_Final#IfcFlowTerminal"/>
        <rdfs:subClassOf>
            <owl:Restriction>
                <owl:onProperty rdf:resource="http://hit2gap.eu/h2g/h2gBI#hasLampType"/>
                <owl:allValuesFrom rdf:resource="http://hit2gap.eu/h2g/h2gBI#LampType"/>
            </owl:Restriction>
        </rdfs:subClassOf>
        <rdfs:comment xml:lang="en">IfcLampType is defined in IFC2X3. We made it equivalent to IfcLamp defined in IFC4.</rdfs:comment>
        <rdfs:isDefinedBy xml:lang="en">http://www.buildingsmart-tech.org/ifcOWL/IFC2X3_Final#IfcLampType</rdfs:isDefinedBy>
        <rdfs:label xml:lang="en">IfcLampType</rdfs:label>
    </owl:Class>
    


    <!-- http://www.buildingsmart-tech.org/ifcOWL/IFC2X3_Final#IfcMember -->

    <owl:Class rdf:about="http://www.buildingsmart-tech.org/ifcOWL/IFC2X3_Final#IfcMember">
        <rdfs:subClassOf rdf:resource="http://www.buildingsmart-tech.org/ifcOWL/IFC2X3_Final#IfcBuildingElement"/>
        <rdfs:comment xml:lang="en">An IfcMember is a structural member designed to carry loads between or beyond points of support. It is not required to be load bearing. The location of the member (being horizontal, vertical or sloped) is not relevant to its definition (in contrary to IfcBeam and IfcColumn).</rdfs:comment>
        <rdfs:isDefinedBy rdf:resource="http://www.buildingsmart-tech.org/ifcOWL/IFC2X3_Final#IfcMember"/>
        <rdfs:label xml:lang="en">IfcMember</rdfs:label>
    </owl:Class>
    


    <!-- http://www.buildingsmart-tech.org/ifcOWL/IFC2X3_Final#IfcOutletType -->

    <owl:Class rdf:about="http://www.buildingsmart-tech.org/ifcOWL/IFC2X3_Final#IfcOutletType">
        <rdfs:subClassOf rdf:resource="http://www.buildingsmart-tech.org/ifcOWL/IFC2X3_Final#IfcFlowTerminal"/>
        <rdfs:comment xml:lang="en">IfcOutletType is defined in IFC2X3. We made it equivalent to IfcOutlet defined in IFC4.</rdfs:comment>
        <rdfs:isDefinedBy xml:lang="en">http://www.buildingsmart-tech.org/ifcOWL/IFC2X3_Final#IfcOutletType</rdfs:isDefinedBy>
        <rdfs:label xml:lang="en">IfcOutletType</rdfs:label>
    </owl:Class>
    


    <!-- http://www.buildingsmart-tech.org/ifcOWL/IFC2X3_Final#IfcPile -->

    <owl:Class rdf:about="http://www.buildingsmart-tech.org/ifcOWL/IFC2X3_Final#IfcPile">
        <rdfs:subClassOf rdf:resource="http://www.buildingsmart-tech.org/ifcOWL/IFC2X3_Final#IfcBuildingElement"/>
        <rdfs:comment xml:lang="en">A pile is a slender timber, concrete, or steel structural element, driven, jetted, or otherwise embedded on end in the ground for the purpose of supporting a load. A pile is also characterized as deep foundation, where the loads are transfered to deeper subsurface layers.</rdfs:comment>
        <rdfs:isDefinedBy rdf:resource="http://www.buildingsmart-tech.org/ifcOWL/IFC2X3_Final#IfcPile"/>
        <rdfs:label xml:lang="en">IfcPile</rdfs:label>
    </owl:Class>
    


    <!-- http://www.buildingsmart-tech.org/ifcOWL/IFC2X3_Final#IfcPlate -->

    <owl:Class rdf:about="http://www.buildingsmart-tech.org/ifcOWL/IFC2X3_Final#IfcPlate">
        <rdfs:subClassOf rdf:resource="http://www.buildingsmart-tech.org/ifcOWL/IFC2X3_Final#IfcBuildingElement"/>
        <rdfs:comment xml:lang="en">An IfcPlate is a planar and often flat part with constant thickness. A plate can be a structural part carrying loads between or beyond points of support, however it is not required to be load bearing. The location of the plate (being horizontal, vertical or sloped) is not relevant to its definition (in contrary to IfcWall and IfcSlab (as floor slab)).</rdfs:comment>
        <rdfs:isDefinedBy rdf:resource="http://www.buildingsmart-tech.org/ifcOWL/IFC2X3_Final#IfcPlate"/>
        <rdfs:label xml:lang="en">IfcPlate</rdfs:label>
    </owl:Class>
    


    <!-- http://www.buildingsmart-tech.org/ifcOWL/IFC2X3_Final#IfcPumpType -->

    <owl:Class rdf:about="http://www.buildingsmart-tech.org/ifcOWL/IFC2X3_Final#IfcPumpType">
        <rdfs:subClassOf rdf:resource="http://www.buildingsmart-tech.org/ifcOWL/IFC2X3_Final#IfcFlowMovingDevice"/>
        <rdfs:comment xml:lang="en">IfcPumpType is defined in IFC2X3. We made it equivalent to IfcPump defined in IFC4.</rdfs:comment>
        <rdfs:isDefinedBy xml:lang="en">http://www.buildingsmart-tech.org/ifcOWL/IFC2X3_Final#IfcPumpType</rdfs:isDefinedBy>
        <rdfs:label xml:lang="en">IfcPumpType</rdfs:label>
    </owl:Class>
    


    <!-- http://www.buildingsmart-tech.org/ifcOWL/IFC2X3_Final#IfcRailing -->

    <owl:Class rdf:about="http://www.buildingsmart-tech.org/ifcOWL/IFC2X3_Final#IfcRailing">
        <rdfs:subClassOf rdf:resource="http://www.buildingsmart-tech.org/ifcOWL/IFC2X3_Final#IfcBuildingElement"/>
        <rdfs:comment xml:lang="en">The railing is a frame assembly adjacent to human circulation spaces and at some space boundaries where it is used in lieu of walls or to compliment walls. Designed to aid humans, either as an optional physical support, or to prevent injury by falling.</rdfs:comment>
        <rdfs:isDefinedBy rdf:resource="http://www.buildingsmart-tech.org/ifcOWL/IFC2X3_Final#IfcRailing"/>
        <rdfs:label xml:lang="en">IfcRailing</rdfs:label>
    </owl:Class>
    


    <!-- http://www.buildingsmart-tech.org/ifcOWL/IFC2X3_Final#IfcRamp -->

    <owl:Class rdf:about="http://www.buildingsmart-tech.org/ifcOWL/IFC2X3_Final#IfcRamp">
        <rdfs:subClassOf rdf:resource="http://www.buildingsmart-tech.org/ifcOWL/IFC2X3_Final#IfcBuildingElement"/>
        <rdfs:comment xml:lang="en">An vertical passageway which provides a human circulation link between one floor level and another floor level at a different elevation. It may include a landing as an intermediate floor slab. A ramp normally does not include steps (stepped ramps are out of scope for this IFC Release).

The ramp is a container entity that aggregates all components of the ramp, it represents. The aggregation is handled via the IfcRelAggregates relationship, relating an IfcRamp with the related flights (IfcRampFlight) and landings (IfcSlab with type &apos;Landing&apos;). Railings belonging to the ramp may be included into the aggregation as IfcRailing.</rdfs:comment>
        <rdfs:isDefinedBy rdf:resource="http://www.buildingsmart-tech.org/ifcOWL/IFC2X3_Final#IfcRamp"/>
        <rdfs:label xml:lang="en">IfcRamp</rdfs:label>
    </owl:Class>
    


    <!-- http://www.buildingsmart-tech.org/ifcOWL/IFC2X3_Final#IfcRampFlight -->

    <owl:Class rdf:about="http://www.buildingsmart-tech.org/ifcOWL/IFC2X3_Final#IfcRampFlight">
        <rdfs:subClassOf rdf:resource="http://www.buildingsmart-tech.org/ifcOWL/IFC2X3_Final#IfcBuildingElement"/>
        <rdfs:comment xml:lang="en">An IfcRampFlight is an aggregated part of an IfcRamp realized through the IfcRelAggregates relationship, the ramp flight is therefore included in the set of IfcRelAggregates.RelatedObjects.
An IfcRampFlight connects the floor slab of zero to two different storeys (or partial storeys or landings) within a building.</rdfs:comment>
        <rdfs:isDefinedBy rdf:resource="http://www.buildingsmart-tech.org/ifcOWL/IFC2X3_Final#IfcRampFlight"/>
        <rdfs:label xml:lang="en">IfcRampFlight</rdfs:label>
    </owl:Class>
    


    <!-- http://www.buildingsmart-tech.org/ifcOWL/IFC2X3_Final#IfcRoof -->

    <owl:Class rdf:about="http://www.buildingsmart-tech.org/ifcOWL/IFC2X3_Final#IfcRoof">
        <rdfs:subClassOf rdf:resource="http://www.buildingsmart-tech.org/ifcOWL/IFC2X3_Final#IfcBuildingElement"/>
        <rdfs:comment xml:lang="en">The IfcRoof is a description of the total roof. It acts as a container entity, that aggregates all components of the roof, it represents. The aggregation is handled via the IfcRelAggregates relationship, relating a roof (IfcRoof) with the related roof entities, like slabs (IfcSlab), rafters and purlins (IfcBeam), or other (included) roofs, such as dormers (IfcRoof).</rdfs:comment>
        <rdfs:isDefinedBy rdf:resource="http://www.buildingsmart-tech.org/ifcOWL/IFC2X3_Final#IfcRoof"/>
        <rdfs:label xml:lang="en">IfcRoof</rdfs:label>
    </owl:Class>
    


    <!-- http://www.buildingsmart-tech.org/ifcOWL/IFC2X3_Final#IfcSanitaryTerminalType -->

    <owl:Class rdf:about="http://www.buildingsmart-tech.org/ifcOWL/IFC2X3_Final#IfcSanitaryTerminalType">
        <rdfs:subClassOf rdf:resource="http://www.buildingsmart-tech.org/ifcOWL/IFC2X3_Final#IfcFlowTerminal"/>
        <rdfs:comment xml:lang="en">IfcSanitaryTerminalType is defined in IFC2X3. We made it equivalent to IfcSanitaryTerminal defined in IFC4.</rdfs:comment>
        <rdfs:isDefinedBy xml:lang="en">http://www.buildingsmart-tech.org/ifcOWL/IFC2X3_Final#IfcSanitaryTerminalType</rdfs:isDefinedBy>
        <rdfs:label xml:lang="en">IfcSanitaryTerminalType</rdfs:label>
    </owl:Class>
    


    <!-- http://www.buildingsmart-tech.org/ifcOWL/IFC2X3_Final#IfcSensorType -->

    <owl:Class rdf:about="http://www.buildingsmart-tech.org/ifcOWL/IFC2X3_Final#IfcSensorType">
        <rdfs:subClassOf rdf:resource="http://hit2gap.eu/h2g/h2gBA#Monitoring"/>
        <rdfs:subClassOf rdf:resource="http://www.buildingsmart-tech.org/ifcOWL/IFC2X3_Final#IfcDistributionControlElement"/>
        <rdfs:subClassOf rdf:resource="http://www.w3.org/ns/ssn/System"/>
        <rdfs:comment xml:lang="en">IfcSensorType is defined in IFC2X3. We made it equivalent to IfcSensor defined in IFC4.</rdfs:comment>
        <rdfs:isDefinedBy xml:lang="en">http://www.buildingsmart-tech.org/ifcOWL/IFC2X3_Final#IfcSensorType</rdfs:isDefinedBy>
        <rdfs:label xml:lang="en">IfcSensorType</rdfs:label>
    </owl:Class>
    


    <!-- http://www.buildingsmart-tech.org/ifcOWL/IFC2X3_Final#IfcShadingDevice -->

    <owl:Class rdf:about="http://www.buildingsmart-tech.org/ifcOWL/IFC2X3_Final#IfcShadingDevice">
        <rdfs:subClassOf rdf:resource="http://www.buildingsmart-tech.org/ifcOWL/IFC2X3_Final#IfcBuildingElement"/>
        <rdfs:comment xml:lang="en">Shading devices are purpose built devices to protect from the sunlight, from natural light, or screening them from view. Shading devices can form part of the facade or can be mounted inside the building, they can be fixed or operable.</rdfs:comment>
        <rdfs:isDefinedBy rdf:resource="http://www.buildingsmart-tech.org/ifcOWL/IFC2X3_Final#IfcShadingDevice"/>
        <rdfs:label xml:lang="en">IfcShadingDevice</rdfs:label>
    </owl:Class>
    


    <!-- http://www.buildingsmart-tech.org/ifcOWL/IFC2X3_Final#IfcSite -->

    <owl:Class rdf:about="http://www.buildingsmart-tech.org/ifcOWL/IFC2X3_Final#IfcSite">
        <rdfs:subClassOf rdf:resource="http://www.buildingsmart-tech.org/ifcOWL/IFC2X3_Final#IfcSpatialStructureElement"/>
        <rdfs:subClassOf>
            <owl:Restriction>
                <owl:onProperty rdf:resource="http://hit2gap.eu/h2g/h2gBI#contains"/>
                <owl:someValuesFrom rdf:resource="http://www.buildingsmart-tech.org/ifcOWL/IFC2X3_Final#IfcBuilding"/>
            </owl:Restriction>
        </rdfs:subClassOf>
        <rdfs:subClassOf>
            <owl:Restriction>
                <owl:onProperty rdf:resource="http://hit2gap.eu/h2g/h2gBI#contains"/>
                <owl:someValuesFrom rdf:resource="http://www.buildingsmart-tech.org/ifcOWL/IFC2X3_Final#IfcSite"/>
            </owl:Restriction>
        </rdfs:subClassOf>
        <rdfs:subClassOf>
            <owl:Restriction>
                <owl:onProperty rdf:resource="http://www.buildingsmart-tech.org/ifcOWL/IFC2X3_TC1#refElevation_IfcSite"/>
                <owl:someValuesFrom rdf:resource="http://www.buildingsmart-tech.org/ifcOWL/IFC2X3_TC1#IfcLengthMeasure"/>
            </owl:Restriction>
        </rdfs:subClassOf>
        <rdfs:subClassOf>
            <owl:Restriction>
                <owl:onProperty rdf:resource="http://hit2gap.eu/h2g/h2gBI#hasOrientation"/>
                <owl:allValuesFrom rdf:resource="http://hit2gap.eu/h2g/h2gBI#Orientation"/>
            </owl:Restriction>
        </rdfs:subClassOf>
        <rdfs:subClassOf>
            <owl:Restriction>
                <owl:onProperty rdf:resource="http://www.buildingsmart-tech.org/ifcOWL/IFC2X3_TC1#refLatitude_IfcSite"/>
                <owl:allValuesFrom rdf:resource="http://www.buildingsmart-tech.org/ifcOWL/IFC2X3_TC1#IfcCompoundPlaneAngleMeasure"/>
            </owl:Restriction>
        </rdfs:subClassOf>
        <rdfs:subClassOf>
            <owl:Restriction>
                <owl:onProperty rdf:resource="http://www.buildingsmart-tech.org/ifcOWL/IFC2X3_TC1#refLongitude_IfcSite"/>
                <owl:allValuesFrom rdf:resource="http://www.buildingsmart-tech.org/ifcOWL/IFC2X3_TC1#IfcCompoundPlaneAngleMeasure"/>
            </owl:Restriction>
        </rdfs:subClassOf>
        <rdfs:subClassOf>
            <owl:Restriction>
                <owl:onProperty rdf:resource="http://www.buildingsmart-tech.org/ifcOWL/IFC2X3_TC1#refElevation_IfcSite"/>
                <owl:maxQualifiedCardinality rdf:datatype="http://www.w3.org/2001/XMLSchema#nonNegativeInteger">1</owl:maxQualifiedCardinality>
                <owl:onClass rdf:resource="http://www.buildingsmart-tech.org/ifcOWL/IFC2X3_TC1#IfcLengthMeasure"/>
            </owl:Restriction>
        </rdfs:subClassOf>
        <rdfs:subClassOf>
            <owl:Restriction>
                <owl:onProperty rdf:resource="http://www.buildingsmart-tech.org/ifcOWL/IFC2X3_TC1#refLatitude_IfcSite"/>
                <owl:maxQualifiedCardinality rdf:datatype="http://www.w3.org/2001/XMLSchema#nonNegativeInteger">1</owl:maxQualifiedCardinality>
                <owl:onClass rdf:resource="http://www.buildingsmart-tech.org/ifcOWL/IFC2X3_TC1#IfcCompoundPlaneAngleMeasure"/>
            </owl:Restriction>
        </rdfs:subClassOf>
        <rdfs:subClassOf>
            <owl:Restriction>
                <owl:onProperty rdf:resource="http://www.buildingsmart-tech.org/ifcOWL/IFC2X3_TC1#refLongitude_IfcSite"/>
                <owl:maxQualifiedCardinality rdf:datatype="http://www.w3.org/2001/XMLSchema#nonNegativeInteger">1</owl:maxQualifiedCardinality>
                <owl:onClass rdf:resource="http://www.buildingsmart-tech.org/ifcOWL/IFC2X3_TC1#IfcCompoundPlaneAngleMeasure"/>
            </owl:Restriction>
        </rdfs:subClassOf>
        <rdfs:comment xml:lang="en">A defined area of land, possibly covered with water, on which the project construction is to be completed. A site may be used to erect building(s) or other AEC products.

A site (IfcSite) may include a definition of the single geographic reference point for this site (global position using Longitude, Latitude and Elevation) for the project. This definition may specify an exact global position of the origin of the local placement of the IfcSite in geospatial terms or it may specify an approximate position intended for informational purposes only.

The geometrical placement of the site, defined by the IfcLocalPlacement, shall be always relative to the spatial structure element, in which this site is included, or absolute, i.e. to the world coordinate system, as established by the geometric representation context of the project. The world coordinate system, established at the IfcProject.RepresentationContexts, may include a definition of the true north within the XY plane of the world coordinate system, if provided, it can be obtained at IfcGeometricRepresentationContext.TrueNorth.

A project may span over several connected or disconnected sites. Therefore site complex provides for a collection of sites included in a project. A site can also be decomposed in parts, where each part defines a site section. This is defined by the composition type attribute of the supertype IfcSpatialStructureElements which is interpreted as follow:

COMPLEX = site complex
ELEMENT = site
PARTIAL = site section</rdfs:comment>
        <rdfs:isDefinedBy rdf:resource="http://www.buildingsmart-tech.org/ifcOWL/IFC2X3_Final#IfcSite"/>
        <rdfs:label xml:lang="en">IfcSite</rdfs:label>
    </owl:Class>
    


    <!-- http://www.buildingsmart-tech.org/ifcOWL/IFC2X3_Final#IfcSlab -->

    <owl:Class rdf:about="http://www.buildingsmart-tech.org/ifcOWL/IFC2X3_Final#IfcSlab">
        <rdfs:subClassOf rdf:resource="http://www.buildingsmart-tech.org/ifcOWL/IFC2X3_Final#IfcBuildingElement"/>
        <rdfs:comment xml:lang="en">The IfcSlab defines the occuurence of any slab, common information about slab types (or styles) is handled by IfcSlabType. The IfcSlabType (if present) may establish the common type name, usage (or predefined) type, common set of properties, common material layer set, and common shape representations (using IfcRepresentationMap). The IfcSlabType is attached using the IfcRelDefinedByType.RelatingType objectified relationship and is accessible by the inverse IsDefinedBy attribute.

As an additional use agreement for standard slabs (i.e. slabs with constant thickness along the extrusion direction), the IfcSlabType should have a unique IfcMaterialLayerSet, that is referenced by the IfcMaterialLayerSetUsage assigned to all occurrences of this slab type.</rdfs:comment>
        <rdfs:isDefinedBy rdf:resource="http://www.buildingsmart-tech.org/ifcOWL/IFC2X3_Final#IfcSlab"/>
        <rdfs:label xml:lang="en">IfcSlab</rdfs:label>
    </owl:Class>
    


    <!-- http://www.buildingsmart-tech.org/ifcOWL/IFC2X3_Final#IfcSpace -->

    <owl:Class rdf:about="http://www.buildingsmart-tech.org/ifcOWL/IFC2X3_Final#IfcSpace">
        <rdfs:subClassOf rdf:resource="http://www.buildingsmart-tech.org/ifcOWL/IFC2X3_Final#IfcSpatialStructureElement"/>
        <rdfs:subClassOf>
            <owl:Restriction>
                <owl:onProperty rdf:resource="http://hit2gap.eu/h2g/h2gBI#contains"/>
                <owl:someValuesFrom rdf:resource="http://www.buildingsmart-tech.org/ifcOWL/IFC2X3_Final#IfcBuildingElement"/>
            </owl:Restriction>
        </rdfs:subClassOf>
        <rdfs:subClassOf>
            <owl:Restriction>
                <owl:onProperty rdf:resource="http://hit2gap.eu/h2g/h2gBI#isContainedIn"/>
                <owl:allValuesFrom rdf:resource="http://www.buildingsmart-tech.org/ifcOWL/IFC2X3_Final#IfcBuildingStorey"/>
            </owl:Restriction>
        </rdfs:subClassOf>
        <rdfs:comment xml:lang="en">A space represents an area or volume bounded actually or theoretically. Spaces are areas or volumes that provide for certain functions within a building.

A space is (if specified) associated to a building storey (or in case of exterior spaces to a site). A space may span over several connected spaces. Therefore a space group provides for a collection of spaces included in a storey. A space can also be decomposed in parts, where each part defines a partial space. This is defined by the composition type attribute of the supertype IfcSpatialStructureElement which is interpreted as follow:

COMPLEX = space group
ELEMENT = space
PARTIAL = partial space
The following guidelines should apply for using the Name, Description, LongName and ObjectType attributes.

Name holds the unique name (or space number) from the plan.
Description holds any additional information field the user may have specified, there are no further recommendations.
LongName holds the full name of the space, it is often used in addition to the Name, if a number is assigned to the room, then the descriptive name is exchanged as LongName.
ObjectType holds the space type, i.e. usually the functional category of the space.</rdfs:comment>
        <rdfs:isDefinedBy rdf:resource="http://www.buildingsmart-tech.org/ifcOWL/IFC2X3_Final#IfcSpace"/>
        <rdfs:label xml:lang="en">IfcSpace</rdfs:label>
    </owl:Class>
    


    <!-- http://www.buildingsmart-tech.org/ifcOWL/IFC2X3_Final#IfcSpaceHeaterType -->

    <owl:Class rdf:about="http://www.buildingsmart-tech.org/ifcOWL/IFC2X3_Final#IfcSpaceHeaterType">
        <rdfs:subClassOf rdf:resource="http://www.buildingsmart-tech.org/ifcOWL/IFC2X3_Final#IfcFlowTerminal"/>
        <rdfs:comment xml:lang="en">IfcSpaceHeaterType is defined in IFC2X3. We made it equivalent to IfcSpaceHeater defined in IFC4.</rdfs:comment>
        <rdfs:isDefinedBy xml:lang="en">http://www.buildingsmart-tech.org/ifcOWL/IFC2X3_Final#IfcSpaceHeaterType</rdfs:isDefinedBy>
        <rdfs:label xml:lang="en">IfcSpaceHeaterType</rdfs:label>
    </owl:Class>
    


    <!-- http://www.buildingsmart-tech.org/ifcOWL/IFC2X3_Final#IfcSpatialElement -->

    <owl:Class rdf:about="http://www.buildingsmart-tech.org/ifcOWL/IFC2X3_Final#IfcSpatialElement">
        <rdfs:subClassOf rdf:resource="http://hit2gap.eu/h2g/h2gSensor#FeatureOfInterest"/>
        <rdfs:subClassOf rdf:resource="http://www.buildingsmart-tech.org/ifcOWL/IFC2X3_TC1#IfcRoot"/>
        <rdfs:subClassOf>
            <owl:Restriction>
                <owl:onProperty rdf:resource="http://hit2gap.eu/h2g/h2gBI#contains"/>
                <owl:someValuesFrom rdf:resource="http://www.buildingsmart-tech.org/ifcOWL/IFC2X3_Final#IfcBuildingElement"/>
            </owl:Restriction>
        </rdfs:subClassOf>
        <rdfs:comment xml:lang="en">A spatial element is the generalization of all spatial elements that might be used to define a spatial structure or to define spatial zones.

a hierarchical spatial structure element as IfcSpatialStructureElement
a spatial structure is a hiearchical decomposition of the project. That spatial structure is often used to provide a project structure to organize a building project.

A spatial project structure might define as many levels of decomposition as necessary for the building project. Elements within the spatial project structure are site, building, storey, and space
a spatial zone as IfcSpatialZone
a spatial zone is a non-hierarchical and potentially overlapping decomposition of the project under some functional consideration.
a spatial zone might be used to represent a thermal zone, a lighting zone, a usable area zone.
a spatial zone might have its independent placement and shape representation.</rdfs:comment>
        <rdfs:isDefinedBy rdf:resource="http://www.buildingsmart-tech.org/ifcOWL/IFC2X3_Final#IfcSpatialElement"/>
        <rdfs:label xml:lang="en">IfcSpatialElement</rdfs:label>
    </owl:Class>
    


    <!-- http://www.buildingsmart-tech.org/ifcOWL/IFC2X3_Final#IfcSpatialStructureElement -->

    <owl:Class rdf:about="http://www.buildingsmart-tech.org/ifcOWL/IFC2X3_Final#IfcSpatialStructureElement">
        <rdfs:subClassOf rdf:resource="http://www.buildingsmart-tech.org/ifcOWL/IFC2X3_Final#IfcSpatialElement"/>
        <rdfs:subClassOf>
            <owl:Restriction>
                <owl:onProperty rdf:resource="http://www.w3.org/ns/ssn/hasProperty"/>
                <owl:someValuesFrom rdf:resource="http://hit2gap.eu/h2g/h2gProperty#PhenomenonProperty"/>
            </owl:Restriction>
        </rdfs:subClassOf>
        <rdfs:comment xml:lang="en">A spatial structure element (IfcSpatialStructureElement) is the generalization of all spatial elements that might be used to define a spatial structure. That spatial structure is often used to provide a project structure to organize a building project.

A spatial project structure might define as many levels of decomposition as necessary for the building project. Elements within the spatial project structure are:

site as IfcSite
building as IfcBuilding
storey as IfcBuildingStorey
space as IfcSpace

or aggregations or parts thereof. The composition type declares an element 
to be either an element itself, or an aggregation (complex) or a decomposition (part). The interpretation of these types is given at each subtype of IfcSpatialStructureElement.</rdfs:comment>
        <rdfs:isDefinedBy rdf:resource="http://www.buildingsmart-tech.org/ifcOWL/IFC2X3_Final#IfcSpatialStructureElement"/>
        <rdfs:label xml:lang="en">IfcSpatialStructureElement</rdfs:label>
    </owl:Class>
    


    <!-- http://www.buildingsmart-tech.org/ifcOWL/IFC2X3_Final#IfcSpatialZone -->

    <owl:Class rdf:about="http://www.buildingsmart-tech.org/ifcOWL/IFC2X3_Final#IfcSpatialZone">
        <rdfs:subClassOf rdf:resource="http://www.buildingsmart-tech.org/ifcOWL/IFC2X3_Final#IfcSpatialElement"/>
        <rdfs:subClassOf>
            <owl:Restriction>
                <owl:onProperty rdf:resource="http://hit2gap.eu/h2g/h2gBI#contains"/>
                <owl:someValuesFrom rdf:resource="http://www.buildingsmart-tech.org/ifcOWL/IFC2X3_Final#IfcElement"/>
            </owl:Restriction>
        </rdfs:subClassOf>
        <rdfs:comment xml:lang="en">A spatial zone is a non-hierarchical and potentially overlapping decomposition of the project under some functional consideration. A spatial zone might be used to represent a thermal zone, a construction zone, a lighting zone, a usable area zone. A spatial zone might have its independent placement and shape representation.

NOTE  The IfcSpatialZone is different to the IfcZone entity by allowing an own placement and shape representation, whereas IfcZone is only a grouping of IfcSpace&apos;s.</rdfs:comment>
        <rdfs:isDefinedBy rdf:resource="http://www.buildingsmart-tech.org/ifcOWL/IFC2X3_Final#IfcSpatialZone"/>
        <rdfs:label xml:lang="en">IfcSpatialZone</rdfs:label>
    </owl:Class>
    


    <!-- http://www.buildingsmart-tech.org/ifcOWL/IFC2X3_Final#IfcStackTerminalType -->

    <owl:Class rdf:about="http://www.buildingsmart-tech.org/ifcOWL/IFC2X3_Final#IfcStackTerminalType">
        <rdfs:subClassOf rdf:resource="http://www.buildingsmart-tech.org/ifcOWL/IFC2X3_Final#IfcFlowTerminal"/>
        <rdfs:comment xml:lang="en">IfcStackTerminalType is defined in IFC2X3. We made it equivalent to IfcStackTerminal defined in IFC4.</rdfs:comment>
        <rdfs:isDefinedBy xml:lang="en">http://www.buildingsmart-tech.org/ifcOWL/IFC2X3_Final#IfcStackTerminalType</rdfs:isDefinedBy>
        <rdfs:label xml:lang="en">IfcStackTerminalType</rdfs:label>
    </owl:Class>
    


    <!-- http://www.buildingsmart-tech.org/ifcOWL/IFC2X3_Final#IfcStair -->

    <owl:Class rdf:about="http://www.buildingsmart-tech.org/ifcOWL/IFC2X3_Final#IfcStair">
        <rdfs:subClassOf rdf:resource="http://www.buildingsmart-tech.org/ifcOWL/IFC2X3_Final#IfcBuildingElement"/>
        <rdfs:comment xml:lang="en">A stair is a vertical passageway allowing occupants to walk (step) from one floor level to another floor level at a different elevation. It may include a landing as an intermediate floor slab.</rdfs:comment>
        <rdfs:isDefinedBy rdf:resource="http://www.buildingsmart-tech.org/ifcOWL/IFC2X3_Final#IfcStair"/>
        <rdfs:label xml:lang="en">IfcStair</rdfs:label>
    </owl:Class>
    


    <!-- http://www.buildingsmart-tech.org/ifcOWL/IFC2X3_Final#IfcStairFlight -->

    <owl:Class rdf:about="http://www.buildingsmart-tech.org/ifcOWL/IFC2X3_Final#IfcStairFlight">
        <rdfs:subClassOf rdf:resource="http://www.buildingsmart-tech.org/ifcOWL/IFC2X3_Final#IfcBuildingElement"/>
        <rdfs:comment xml:lang="en">Assembly of building components in a single &quot;run&quot; of stair steps (not interrupted by a landing). The stair steps and any stringers are included in this object. A winder is regarded as part of a stair flight.

An IfcStairFlight is normally aggregated by a stair (IfcStair) through the IfcRelAggregates relationship, the stair flight is then included in the set of IfcRelAggregates.RelatedObjects.

An IfcStairFlight normally connects the floor slab of zero to two different storeys (or partial storeys) within a building.</rdfs:comment>
        <rdfs:isDefinedBy rdf:resource="http://www.buildingsmart-tech.org/ifcOWL/IFC2X3_Final#IfcStairFlight"/>
        <rdfs:label xml:lang="en">IfcStairFlight</rdfs:label>
    </owl:Class>
    


    <!-- http://www.buildingsmart-tech.org/ifcOWL/IFC2X3_Final#IfcTankType -->

    <owl:Class rdf:about="http://www.buildingsmart-tech.org/ifcOWL/IFC2X3_Final#IfcTankType">
        <rdfs:subClassOf rdf:resource="http://www.buildingsmart-tech.org/ifcOWL/IFC2X3_Final#IfcFlowStorageDevice"/>
        <rdfs:comment xml:lang="en">IfcTankType is defined in IFC2X3. We made it equivalent to IfcTank defined in IFC4.</rdfs:comment>
        <rdfs:isDefinedBy xml:lang="en">http://www.buildingsmart-tech.org/ifcOWL/IFC2X3_Final#IfcTankType</rdfs:isDefinedBy>
        <rdfs:label xml:lang="en">IfcTankType</rdfs:label>
    </owl:Class>
    


    <!-- http://www.buildingsmart-tech.org/ifcOWL/IFC2X3_Final#IfcTransformerType -->

    <owl:Class rdf:about="http://www.buildingsmart-tech.org/ifcOWL/IFC2X3_Final#IfcTransformerType">
        <rdfs:subClassOf rdf:resource="http://www.buildingsmart-tech.org/ifcOWL/IFC2X3_Final#IfcEnergyConversionDevice"/>
        <rdfs:comment xml:lang="en">IfcTransformerType is defined in IFC2X3. We made it equivalent to IfcTransformer defined in IFC4.</rdfs:comment>
        <rdfs:isDefinedBy xml:lang="en">http://www.buildingsmart-tech.org/ifcOWL/IFC2X3_Final#IfcTransformerType</rdfs:isDefinedBy>
        <rdfs:label xml:lang="en">IfcTransformerType</rdfs:label>
    </owl:Class>
    


    <!-- http://www.buildingsmart-tech.org/ifcOWL/IFC2X3_Final#IfcUnitaryControlElementType -->

    <owl:Class rdf:about="http://www.buildingsmart-tech.org/ifcOWL/IFC2X3_Final#IfcUnitaryControlElementType">
        <rdfs:subClassOf rdf:resource="http://www.buildingsmart-tech.org/ifcOWL/IFC2X3_Final#IfcDistributionControlElement"/>
        <rdfs:comment xml:lang="en">IfcUnitaryControlElementType is defined in IFC2X3. We made it equivalent to IfcUnitaryControlElement defined in IFC4.</rdfs:comment>
        <rdfs:isDefinedBy xml:lang="en">http://www.buildingsmart-tech.org/ifcOWL/IFC2X3_Final#IfcUnitaryControlElementType</rdfs:isDefinedBy>
        <rdfs:label xml:lang="en">IfcUnitaryControlElementType</rdfs:label>
    </owl:Class>
    


    <!-- http://www.buildingsmart-tech.org/ifcOWL/IFC2X3_Final#IfcValveType -->

    <owl:Class rdf:about="http://www.buildingsmart-tech.org/ifcOWL/IFC2X3_Final#IfcValveType">
        <rdfs:subClassOf rdf:resource="http://www.buildingsmart-tech.org/ifcOWL/IFC2X3_Final#IfcFlowController"/>
        <rdfs:comment xml:lang="en">IfcValveType is defined in IFC2X3. We made it equivalent to IfcValve defined in IFC4.</rdfs:comment>
        <rdfs:isDefinedBy xml:lang="en">http://www.buildingsmart-tech.org/ifcOWL/IFC2X3_Final#IfcValveType</rdfs:isDefinedBy>
        <rdfs:label xml:lang="en">IfcValveType</rdfs:label>
    </owl:Class>
    


    <!-- http://www.buildingsmart-tech.org/ifcOWL/IFC2X3_Final#IfcVibrationIsolatorType -->

    <owl:Class rdf:about="http://www.buildingsmart-tech.org/ifcOWL/IFC2X3_Final#IfcVibrationIsolatorType">
        <rdfs:subClassOf rdf:resource="http://www.buildingsmart-tech.org/ifcOWL/IFC2X3_Final#IfcElementComponent"/>
        <rdfs:comment xml:lang="en">IfcVibrationisolatorType is defined in IFC2X3. We made it equivalent to IfcVibrationisolator defined in IFC4.</rdfs:comment>
        <rdfs:isDefinedBy xml:lang="en">http://www.buildingsmart-tech.org/ifcOWL/IFC2X3_Final#IfcVibrationIsolatorType</rdfs:isDefinedBy>
        <rdfs:label xml:lang="en">IfcVibrationIsolatorType</rdfs:label>
    </owl:Class>
    


    <!-- http://www.buildingsmart-tech.org/ifcOWL/IFC2X3_Final#IfcWall -->

    <owl:Class rdf:about="http://www.buildingsmart-tech.org/ifcOWL/IFC2X3_Final#IfcWall">
        <rdfs:subClassOf rdf:resource="http://www.buildingsmart-tech.org/ifcOWL/IFC2X3_Final#IfcBuildingElement"/>
        <rdfs:subClassOf>
            <owl:Restriction>
                <owl:onProperty rdf:resource="http://hit2gap.eu/h2g/h2gBI#isInside"/>
                <owl:allValuesFrom rdf:resource="http://www.w3.org/2001/XMLSchema#boolean"/>
            </owl:Restriction>
        </rdfs:subClassOf>
        <rdfs:subClassOf>
            <owl:Restriction>
                <owl:onProperty rdf:resource="http://hit2gap.eu/h2g/h2gBI#windowWallRatio"/>
                <owl:allValuesFrom rdf:resource="http://www.w3.org/2001/XMLSchema#float"/>
            </owl:Restriction>
        </rdfs:subClassOf>
        <rdfs:comment xml:lang="en">The wall represents a vertical construction that bounds or subdivides spaces. Wall are usually vertical, or nearly vertical, planar elements, often designed to bear structural loads. A wall is however not required to be load bearing.</rdfs:comment>
        <rdfs:isDefinedBy rdf:resource="http://www.buildingsmart-tech.org/ifcOWL/IFC2X3_Final#IfcWall"/>
        <rdfs:label xml:lang="en">IfcWall</rdfs:label>
    </owl:Class>
    


    <!-- http://www.buildingsmart-tech.org/ifcOWL/IFC2X3_Final#IfcWasteTerminalType -->

    <owl:Class rdf:about="http://www.buildingsmart-tech.org/ifcOWL/IFC2X3_Final#IfcWasteTerminalType">
        <rdfs:subClassOf rdf:resource="http://www.buildingsmart-tech.org/ifcOWL/IFC2X3_Final#IfcFlowTerminal"/>
        <rdfs:comment xml:lang="en">IfcWasteTerminalType is defined in IFC2X3. We made it equivalent to IfcWasteTerminal defined in IFC4.</rdfs:comment>
        <rdfs:isDefinedBy xml:lang="en">http://www.buildingsmart-tech.org/ifcOWL/IFC2X3_Final#IfcWasteTerminalType</rdfs:isDefinedBy>
        <rdfs:label xml:lang="en">IfcWasteTerminalType</rdfs:label>
    </owl:Class>
    


    <!-- http://www.buildingsmart-tech.org/ifcOWL/IFC2X3_Final#IfcWindow -->

    <owl:Class rdf:about="http://www.buildingsmart-tech.org/ifcOWL/IFC2X3_Final#IfcWindow">
        <rdfs:subClassOf rdf:resource="http://www.buildingsmart-tech.org/ifcOWL/IFC2X3_Final#IfcBuildingElement"/>
        <rdfs:subClassOf>
            <owl:Restriction>
                <owl:onProperty rdf:resource="http://hit2gap.eu/h2g/h2gBI#hasWindowCovering"/>
                <owl:someValuesFrom rdf:resource="http://hit2gap.eu/h2g/h2gBI#WindowCovering"/>
            </owl:Restriction>
        </rdfs:subClassOf>
        <rdfs:subClassOf>
            <owl:Restriction>
                <owl:onProperty rdf:resource="http://hit2gap.eu/h2g/h2gBI#hasWindowGlazing"/>
                <owl:someValuesFrom rdf:resource="http://hit2gap.eu/h2g/h2gBI#WindowGlazing"/>
            </owl:Restriction>
        </rdfs:subClassOf>
        <rdfs:subClassOf>
            <owl:Restriction>
                <owl:onProperty rdf:resource="http://hit2gap.eu/h2g/h2gBI#hasPartitioningType"/>
                <owl:allValuesFrom rdf:resource="http://www.buildingsmart-tech.org/ifcOWL/IFC2X3_Final#IfcWindowTypePartitioningEnum"/>
            </owl:Restriction>
        </rdfs:subClassOf>
        <rdfs:subClassOf>
            <owl:Restriction>
                <owl:onProperty rdf:resource="http://hit2gap.eu/h2g/h2gBI#hasWindowType"/>
                <owl:allValuesFrom rdf:resource="http://www.buildingsmart-tech.org/ifcOWL/IFC2X3_Final#IfcWindowTypeEnum"/>
            </owl:Restriction>
        </rdfs:subClassOf>
        <rdfs:comment xml:lang="en">The window is a building element that is predominately used to provide natural light and fresh air. It includes vertical and horizontal opening (e.g. skylights or light domes). It includes constructions with swinging, pivoting, sliding, or revolving panels and fixed panels. A window consists of a lining and one or several panels.

The IfcWindow defines a particular occurrence of a window inserted in the spatial context of a project.</rdfs:comment>
        <rdfs:isDefinedBy rdf:resource="http://www.buildingsmart-tech.org/ifcOWL/IFC2X3_Final#IfcWindow"/>
        <rdfs:label xml:lang="en">IfcWindow</rdfs:label>
    </owl:Class>
    


    <!-- http://www.buildingsmart-tech.org/ifcOWL/IFC2X3_Final#IfcZone -->

    <owl:Class rdf:about="http://www.buildingsmart-tech.org/ifcOWL/IFC2X3_Final#IfcZone">
        <rdfs:subClassOf>
            <owl:Restriction>
                <owl:onProperty rdf:resource="http://hit2gap.eu/h2g/h2gBI#contains"/>
                <owl:someValuesFrom rdf:resource="http://www.buildingsmart-tech.org/ifcOWL/IFC2X3_Final#IfcSpace"/>
            </owl:Restriction>
        </rdfs:subClassOf>
        <rdfs:subClassOf>
            <owl:Restriction>
                <owl:onProperty rdf:resource="http://hit2gap.eu/h2g/h2gBI#contains"/>
                <owl:someValuesFrom rdf:resource="http://www.buildingsmart-tech.org/ifcOWL/IFC2X3_Final#IfcZone"/>
            </owl:Restriction>
        </rdfs:subClassOf>
        <rdfs:comment xml:lang="en">A zone (IfcZone) is an aggregation of spaces, partial spaces or other zones. Zone structures may not be hierarchical (in contrary to the spatial structure of a project - see IfcSpatialStructureElement), i.e. one individual IfcSpace may be associated with zero, one, or several IfcZone&apos;s. IfcSpace&apos;s are aggregated into an IfcZone by using the objectified relationship IfcRelAssignsToGroup as specified at the supertype IfcGroup.

NOTE  Certain use cases may restrict the freedom of non hierarchical relationships. In some building service use cases the zone denotes a view based delimited volume for the purpose of analysis and calculation. This type of zone cannot overlap with respect to that analysis, but may overlap otherwise.

NOTE  One of the purposes of a zone is to define a fire compartmentation. In this case it defines the geometric information about the fire compartment (through the contained spaces) and information, whether this compartment is ventilated or sprinkler protected. In addition the fire risk code and the hazard type can be added, the coding is normally defined within a national fire regulation. All that information is available within the relevant property sets.
RECOMMENDATION  In case of a zone denoting a (fire) compartment, the following types should be used, if applicable, as values of the ObjectType attribute:

FireCompartment - a zone of spaces, collected to represent a single fire compartment.

ElevatorShaft - a collection of spaces within an elevator, potentially going through many storeys.

RisingDuct

RunningDuct

Additional classifications of the IfcZone, as provided by a national classification system, can be assigned by using the IfcRelAssociatesClassification relationship.</rdfs:comment>
        <rdfs:isDefinedBy xml:lang="en">http://www.buildingsmart-tech.org/ifcOWL/IFC2X3_Final#IfcZone</rdfs:isDefinedBy>
        <rdfs:label xml:lang="en">IfcZone</rdfs:label>
    </owl:Class>
    


    <!-- http://www.buildingsmart-tech.org/ifcOWL/IFC2X3_TC1#IfcCompoundPlaneAngleMeasure -->

    <owl:Class rdf:about="http://www.buildingsmart-tech.org/ifcOWL/IFC2X3_TC1#IfcCompoundPlaneAngleMeasure">
        <rdfs:comment xml:lang="en">IfcCompoundPlaneAngleMeasure is a compound measure of plane angle in degrees, minutes, seconds, and optionally millionth-seconds of arc.</rdfs:comment>
        <rdfs:isDefinedBy rdf:resource="http://www.buildingsmart-tech.org/ifcOWL/IFC2X3_TC1#IfcCompoundPlaneAngleMeasure"/>
        <rdfs:label xml:lang="en">IfcCompoundPlaneAngleMeasure</rdfs:label>
    </owl:Class>
    


    <!-- http://www.buildingsmart-tech.org/ifcOWL/IFC2X3_TC1#IfcGloballyUniqueId -->

    <owl:Class rdf:about="http://www.buildingsmart-tech.org/ifcOWL/IFC2X3_TC1#IfcGloballyUniqueId">
        <rdfs:comment xml:lang="en">Holds an identifier that is unique throughout the software world. This is also known as a Globally Unique Identifier (GUID) or Universal Unique Identifier (UUID) by the Open Group. The identifier is generated using an algorithm published by the Object Management Group. The algorithm is explained at the open group website. The Microsoft Foundation Class (MFC) function &quot;CoCreateGuid&quot;, which is an implementation of the above algorithm, has been used by many IFC implementers to create an identifier.

An identifier is a unique 128-bit number. Since this identifier is required for all IFC object instances, it is desirable to compress the identifier size to reduce overhead. Beginning in IFC R1.5.1, IFC implementers agreed to compress the identifier down to 20 characters using an algorithm developed by IAI Implementers. This algorithm maps the identifier bits onto a base 85 digit encoded from the following character set:

0123456789ABCDEFGHIJKLMNOPQRSTUVWXYZabcdefghijklmnopqrstuvwxyz!#$%&amp;^|*+,-./:;&lt;=&gt;?~`@_

An index (0-84) into this character set string determines the &quot;value&quot; for each character (e.g. &quot;A&quot; has a value of 10, &quot;@&quot; has a value of 83, etc.). Note that all characters are case-sensitive. In order to prevent possible problems with some parsers, implementers have agreed not to use the &quot;/*&quot; and &quot;*/&quot; character combinations in the identifier string and instead to use &quot;\*&quot; and &quot;*\&quot;.

The implementation of the compression algorithm has changed in IFC R2x in order to prevent conflicts with special characters in the ISO 10303-21 exchange file and the W3C XML file (such as &apos;&lt;*&apos;, &apos;*&gt;&apos;, &apos;&lt;&apos; and &apos;&gt;&apos;). Using 64 characters for the base rather than 85, the resulting compressed string now needs 22 characters. The encoding of the base 64 character set is shown below:

           1         2         3         4         5         6 
 0123456789012345678901234567890123456789012345678901234567890123
&quot;0123456789ABCDEFGHIJKLMNOPQRSTUVWXYZabcdefghijklmnopqrstuvwxyz_$&quot;;

The following code example in C is given as a guideline for creating the base 64 compressed strings and for mapping the previous base 85 strings to the base 64 strings. This code is provided &quot;as-is&quot; with no support or guarantee of suitability provided by the IAI. Use of the code example is at the sole risk of the user.

CreateGuid_64.h
CreateGuid_64.c
The resulting string is a fixed 22 character length string to be exchanged within the IFC exchange file structure.

HISTORY: New type in IFC R1.5.1.</rdfs:comment>
        <rdfs:isDefinedBy rdf:resource="http://www.buildingsmart-tech.org/ifcOWL/IFC2X3_TC1#IfcGloballyUniqueId"/>
        <rdfs:label xml:lang="en">IfcGloballyUniqueId</rdfs:label>
    </owl:Class>
    


    <!-- http://www.buildingsmart-tech.org/ifcOWL/IFC2X3_TC1#IfcLabel -->

    <owl:Class rdf:about="http://www.buildingsmart-tech.org/ifcOWL/IFC2X3_TC1#IfcLabel">
        <rdfs:comment xml:lang="en">A label is the term by which something may be referred to. It is a string which represents the human-interpretable name of something and shall have a natural-language meaning.</rdfs:comment>
        <rdfs:label rdf:resource="http://www.buildingsmart-tech.org/ifcOWL/IFC2X3_TC1#IfcLabel"/>
        <rdfs:label xml:lang="en">IfcLabel</rdfs:label>
    </owl:Class>
    


    <!-- http://www.buildingsmart-tech.org/ifcOWL/IFC2X3_TC1#IfcLengthMeasure -->

    <owl:Class rdf:about="http://www.buildingsmart-tech.org/ifcOWL/IFC2X3_TC1#IfcLengthMeasure">
        <rdfs:comment xml:lang="en">A length measure is the value of a distance.

Usually measured in millimeters (mm).</rdfs:comment>
        <rdfs:isDefinedBy rdf:resource="http://www.buildingsmart-tech.org/ifcOWL/IFC2X3_TC1#IfcLengthMeasure"/>
        <rdfs:label xml:lang="en">IfcLengthMeasure</rdfs:label>
    </owl:Class>
    


    <!-- http://www.buildingsmart-tech.org/ifcOWL/IFC2X3_TC1#IfcRoot -->

    <owl:Class rdf:about="http://www.buildingsmart-tech.org/ifcOWL/IFC2X3_TC1#IfcRoot">
        <rdfs:subClassOf>
            <owl:Restriction>
                <owl:onProperty rdf:resource="http://www.buildingsmart-tech.org/ifcOWL/IFC2X3_TC1#description_IfcRoot"/>
                <owl:allValuesFrom rdf:resource="http://www.buildingsmart-tech.org/ifcOWL/IFC2X3_TC1#IfcText"/>
            </owl:Restriction>
        </rdfs:subClassOf>
        <rdfs:subClassOf>
            <owl:Restriction>
                <owl:onProperty rdf:resource="http://www.buildingsmart-tech.org/ifcOWL/IFC2X3_TC1#globalId_IfcRoot"/>
                <owl:allValuesFrom rdf:resource="http://www.buildingsmart-tech.org/ifcOWL/IFC2X3_TC1#IfcGloballyUniqueId"/>
            </owl:Restriction>
        </rdfs:subClassOf>
        <rdfs:subClassOf>
            <owl:Restriction>
                <owl:onProperty rdf:resource="http://www.buildingsmart-tech.org/ifcOWL/IFC2X3_TC1#name_IfcRoot"/>
                <owl:allValuesFrom rdf:resource="http://www.buildingsmart-tech.org/ifcOWL/IFC2X3_TC1#IfcLabel"/>
            </owl:Restriction>
        </rdfs:subClassOf>
        <rdfs:subClassOf>
            <owl:Restriction>
                <owl:onProperty rdf:resource="http://www.buildingsmart-tech.org/ifcOWL/IFC2X3_TC1#globalId_IfcRoot"/>
                <owl:qualifiedCardinality rdf:datatype="http://www.w3.org/2001/XMLSchema#nonNegativeInteger">1</owl:qualifiedCardinality>
                <owl:onClass rdf:resource="http://www.buildingsmart-tech.org/ifcOWL/IFC2X3_TC1#IfcGloballyUniqueId"/>
            </owl:Restriction>
        </rdfs:subClassOf>
        <rdfs:subClassOf>
            <owl:Restriction>
                <owl:onProperty rdf:resource="http://www.buildingsmart-tech.org/ifcOWL/IFC2X3_TC1#description_IfcRoot"/>
                <owl:maxQualifiedCardinality rdf:datatype="http://www.w3.org/2001/XMLSchema#nonNegativeInteger">1</owl:maxQualifiedCardinality>
                <owl:onClass rdf:resource="http://www.buildingsmart-tech.org/ifcOWL/IFC2X3_TC1#IfcText"/>
            </owl:Restriction>
        </rdfs:subClassOf>
        <rdfs:subClassOf>
            <owl:Restriction>
                <owl:onProperty rdf:resource="http://www.buildingsmart-tech.org/ifcOWL/IFC2X3_TC1#name_IfcRoot"/>
                <owl:maxQualifiedCardinality rdf:datatype="http://www.w3.org/2001/XMLSchema#nonNegativeInteger">1</owl:maxQualifiedCardinality>
                <owl:onClass rdf:resource="http://www.buildingsmart-tech.org/ifcOWL/IFC2X3_TC1#IfcLabel"/>
            </owl:Restriction>
        </rdfs:subClassOf>
        <rdfs:comment xml:lang="en">The IfcRoot is the most abstract and root class for all IFC entity definitions that roots in the kernel or in subsequent layers of the IFC object model. It is therefore the common supertype all all IFC entities, beside those defined in an IFC resource schema. All entities that are subtypes of IfcRoot can be used independently, whereas resource schema entities, that are not subtypes of IfcRoot, are not supposed to be independent entities.

The IfcRoot assigns the globally unique ID, and the ownership and history information to the entity. In addition it may provide for a name and a description about the concepts.</rdfs:comment>
        <rdfs:isDefinedBy rdf:resource="http://www.buildingsmart-tech.org/ifcOWL/IFC2X3_TC1#IfcRoot"/>
        <rdfs:label xml:lang="en">IfcRoot</rdfs:label>
    </owl:Class>
    


    <!-- http://www.buildingsmart-tech.org/ifcOWL/IFC2X3_TC1#IfcText -->

    <owl:Class rdf:about="http://www.buildingsmart-tech.org/ifcOWL/IFC2X3_TC1#IfcText">
        <rdfs:comment xml:lang="en">A text is an alphanumeric string of characters which is intended to be read and understood by a human being. It is for information purposes only.

Type: STRING
NOTE Corresponding STEP name: text, please refer to ISO/IS 10303-41:1994 for the final definition of the formal standard.</rdfs:comment>
        <rdfs:isDefinedBy rdf:resource="http://www.buildingsmart-tech.org/ifcOWL/IFC2X3_TC1#IfcText"/>
        <rdfs:label xml:lang="en">fcText</rdfs:label>
    </owl:Class>
    


    <!-- http://www.opengis/net/gml/Envelope -->

    <owl:Class rdf:about="http://www.opengis/net/gml/Envelope">
        <rdfs:subClassOf rdf:resource="http://www.opengis/net/gml/_Geometry"/>
        <rdfs:isDefinedBy rdf:resource="http://www.opengis/net/gml/Envelope"/>
        <rdfs:label xml:lang="en">Envelope</rdfs:label>
    </owl:Class>
    


    <!-- http://www.opengis/net/gml/LineString -->

    <owl:Class rdf:about="http://www.opengis/net/gml/LineString">
        <rdfs:subClassOf rdf:resource="http://www.opengis/net/gml/_Geometry"/>
        <rdfs:comment rdf:resource="http://www.opengis/net/gml/LineString"/>
        <rdfs:comment xml:lang="en">The gml:posList property is defined for all elements of LineString.</rdfs:comment>
        <rdfs:label xml:lang="en">LineString</rdfs:label>
    </owl:Class>
    


    <!-- http://www.opengis/net/gml/LinearRing -->

    <owl:Class rdf:about="http://www.opengis/net/gml/LinearRing">
        <rdfs:subClassOf rdf:resource="http://www.opengis/net/gml/_Geometry"/>
        <rdfs:comment xml:lang="en">The gml:posList property is defined for all elements of LinearRing</rdfs:comment>
        <rdfs:isDefinedBy rdf:resource="http://www.opengis/net/gml/LinearRing"/>
        <rdfs:label xml:lang="en">LinearRing</rdfs:label>
    </owl:Class>
    


    <!-- http://www.opengis/net/gml/Point -->

    <owl:Class rdf:about="http://www.opengis/net/gml/Point">
        <rdfs:subClassOf rdf:resource="http://www.opengis/net/gml/_Geometry"/>
        <rdfs:comment xml:lang="en">A point contains a single coordinate pair. The coordinate pair contains a latitude value and a longitude value in that order. The preferred serialization of this uses a space to separate the two values.</rdfs:comment>
        <rdfs:comment xml:lang="en">The gml:pos property is defined for all elements of Point</rdfs:comment>
        <rdfs:isDefinedBy rdf:resource="http://www.opengis/net/gml/Point"/>
        <rdfs:label xml:lang="en">Point</rdfs:label>
    </owl:Class>
    


    <!-- http://www.opengis/net/gml/Polygon -->

    <owl:Class rdf:about="http://www.opengis/net/gml/Polygon">
        <rdfs:subClassOf rdf:resource="http://www.opengis/net/gml/_Geometry"/>
        <rdfs:comment xml:lang="en">A polygon contains at least four coordinate pairs. Each pair contains a latitude value and a longitude value in that order. The preferred serialization of this uses a space to separate the two values. Pairs are separated from each other by a space. The last coordinate pair must be identical to the first.</rdfs:comment>
        <rdfs:isDefinedBy xml:lang="en">http://www.opengis/net/gml/Polygon</rdfs:isDefinedBy>
        <rdfs:label xml:lang="en">Polygon</rdfs:label>
    </owl:Class>
    


    <!-- http://www.opengis/net/gml/_Feature -->

    <owl:Class rdf:about="http://www.opengis/net/gml/_Feature">
        <rdfs:subClassOf>
            <owl:Restriction>
                <owl:onProperty rdf:resource="http://hit2gap.eu/h2g/h2gBI#locatedInClimate"/>
                <owl:allValuesFrom rdf:resource="http://hit2gap.eu/h2g/h2gBI#Climate"/>
            </owl:Restriction>
        </rdfs:subClassOf>
        <rdfs:subClassOf>
            <owl:Restriction>
                <owl:onProperty rdf:resource="http://hit2gap.eu/h2g/h2gSensor#locatedInHemisphere"/>
                <owl:allValuesFrom rdf:resource="http://hit2gap.eu/h2g/h2gSensor#Hemisphere"/>
            </owl:Restriction>
        </rdfs:subClassOf>
        <rdfs:subClassOf>
            <owl:Restriction>
                <owl:onProperty rdf:resource="http://www.georss.org/georss/where"/>
                <owl:allValuesFrom rdf:resource="http://www.opengis/net/gml/_Geometry"/>
            </owl:Restriction>
        </rdfs:subClassOf>
        <rdfs:comment xml:lang="en">_Feature is taken from  the GeoRSS Feature Model. The model provides a general feature property which can be used to characterize any appropriate content as a geographic feature. Specific subproperties such as &lt;where&gt; associate the discerned feature with one of a limited number of  geometry types which provide a numerical representation for analysis and visualization. Other subproperties describe additional commonly used feature attributes such as feature name and feature type.</rdfs:comment>
        <rdfs:isDefinedBy rdf:resource="http://www.opengis/net/gml/_Feature"/>
        <rdfs:label xml:lang="en">_Feature</rdfs:label>
    </owl:Class>
    


    <!-- http://www.opengis/net/gml/_Geometry -->

    <owl:Class rdf:about="http://www.opengis/net/gml/_Geometry">
        <rdfs:comment xml:lang="en">GeoRSS feature model allows the description of rectangles, points, lines, and polygons as geometric representation properties of discerned geographic features. Simple Features&apos; geometric representations consist of point and multipoint, curve (a.k.a. line) and multicurve, surface (polygon) and multisurface.</rdfs:comment>
        <rdfs:isDefinedBy rdf:resource="http://www.opengis/net/gml/_Geometry"/>
        <rdfs:label xml:lang="en">_Geometry</rdfs:label>
    </owl:Class>
    


    <!-- http://www.w3.org/2006/time#DateTimeInterval -->

    <owl:Class rdf:about="http://www.w3.org/2006/time#DateTimeInterval">
        <rdfs:subClassOf>
            <owl:Restriction>
                <owl:onProperty rdf:resource="http://www.w3.org/2006/time#inXSDDateTime"/>
                <owl:allValuesFrom rdf:resource="http://www.w3.org/2001/XMLSchema#dateTime"/>
            </owl:Restriction>
        </rdfs:subClassOf>
        <rdfs:comment xml:lang="en">It enables compact representation of an interval corresponding to a single element in a date-time description (i.e. a specified year, month, week, day, hour, minute, second).</rdfs:comment>
        <rdfs:isDefinedBy xml:lang="en">http://www.w3.org/2006/time#DateTimeInterval</rdfs:isDefinedBy>
        <rdfs:label xml:lang="en">DateTimeInterval</rdfs:label>
    </owl:Class>
    


    <!-- http://www.w3.org/2006/time#Instant -->

    <owl:Class rdf:about="http://www.w3.org/2006/time#Instant">
        <rdfs:subClassOf>
            <owl:Restriction>
                <owl:onProperty rdf:resource="http://www.w3.org/2006/time#inXSDDateTime"/>
                <owl:allValuesFrom rdf:resource="http://www.w3.org/2001/XMLSchema#dateTime"/>
            </owl:Restriction>
        </rdfs:subClassOf>
        <rdfs:comment xml:lang="en">A temporal entity with zero extent or duration.</rdfs:comment>
        <rdfs:isDefinedBy xml:lang="en">http://www.w3.org/2006/time#Instant</rdfs:isDefinedBy>
        <rdfs:label xml:lang="en">Instant</rdfs:label>
    </owl:Class>
    


    <!-- http://www.w3.org/ns/sosa/FeatureOfInterest -->

    <rdf:Description rdf:about="http://www.w3.org/ns/sosa/FeatureOfInterest"/>
    


    <!-- http://www.w3.org/ns/sosa/Result -->

    <owl:Class rdf:about="http://www.w3.org/ns/sosa/Result">
        <rdfs:subClassOf>
            <owl:Restriction>
                <owl:onProperty rdf:resource="http://data.qudt.org/qudt/owl/1.0.0/qudt.owl#hasUnit"/>
                <owl:allValuesFrom rdf:resource="http://qudt.org/schema/qudt#Unit"/>
            </owl:Restriction>
        </rdfs:subClassOf>
        <rdfs:comment xml:lang="en">The Result of an Observation, Actuation, or act of Sampling. To store an observation&apos;s simple result value one can use the hasSimpleResult property.</rdfs:comment>
        <rdfs:isDefinedBy xml:lang="en">http://www.w3.org/ns/sosa/Result</rdfs:isDefinedBy>
        <rdfs:label xml:lang="en">Result</rdfs:label>
    </owl:Class>
    


    <!-- http://www.w3.org/ns/sosa/Sensor -->

    <owl:Class rdf:about="http://www.w3.org/ns/sosa/Sensor">
        <rdfs:subClassOf rdf:resource="http://hit2gap.eu/h2g/h2gBA#Monitoring"/>
        <rdfs:subClassOf rdf:resource="http://www.w3.org/ns/ssn/System"/>
        <rdfs:subClassOf>
            <owl:Restriction>
                <owl:onProperty rdf:resource="http://www.w3.org/ns/sosa/madeObservation"/>
                <owl:allValuesFrom rdf:resource="http://hit2gap.eu/h2g/h2gSensor#Observation"/>
            </owl:Restriction>
        </rdfs:subClassOf>
        <rdfs:comment xml:lang="en">Device, agent (including humans), or software (simulation) involved in, or implementing, a (Sensing) Procedure. Sensors respond to a stimulus, e.g., a change in the environment, or input data composed from the results of prior Observations, and generate a Result. Sensors can be hosted by Platforms.</rdfs:comment>
        <rdfs:isDefinedBy xml:lang="en">http://www.w3.org/ns/sosa/Sensor</rdfs:isDefinedBy>
        <rdfs:label xml:lang="en">Sensor</rdfs:label>
    </owl:Class>
    


    <!-- http://www.w3.org/ns/ssn/System -->

    <owl:Class rdf:about="http://www.w3.org/ns/ssn/System">
        <rdfs:subClassOf rdf:resource="http://www.opengis/net/gml/_Feature"/>
        <rdfs:subClassOf>
            <owl:Restriction>
                <owl:onProperty rdf:resource="http://www.w3.org/ns/ssn/hasSubSystem"/>
                <owl:allValuesFrom rdf:resource="http://www.w3.org/ns/ssn/System"/>
            </owl:Restriction>
        </rdfs:subClassOf>
        <rdfs:comment xml:lang="en">System is a unit of abstraction for pieces of infrastructure that implements Procedures. A System may have components, its subsystems, which are other systems.</rdfs:comment>
        <rdfs:isDefinedBy xml:lang="en">http://www.w3.org/ns/ssn/System</rdfs:isDefinedBy>
        <rdfs:label xml:lang="en">System</rdfs:label>
    </owl:Class>
    


    <!-- 
    ///////////////////////////////////////////////////////////////////////////////////////
    //
    // Individuals
    //
    ///////////////////////////////////////////////////////////////////////////////////////
     -->

    


    <!-- http://hit2gap.eu/h2g/h2gBA#Smartphone -->

    <owl:NamedIndividual rdf:about="http://hit2gap.eu/h2g/h2gBA#Smartphone">
        <rdf:type rdf:resource="http://hit2gap.eu/h2g/h2gBA#Wearable"/>
    </owl:NamedIndividual>
    


    <!-- http://hit2gap.eu/h2g/h2gBA#Smartwatch -->

    <owl:NamedIndividual rdf:about="http://hit2gap.eu/h2g/h2gBA#Smartwatch">
        <rdf:type rdf:resource="http://hit2gap.eu/h2g/h2gBA#Wearable"/>
    </owl:NamedIndividual>
    


    <!-- http://hit2gap.eu/h2g/h2gBI#CentralLight -->

    <owl:NamedIndividual rdf:about="http://hit2gap.eu/h2g/h2gBI#CentralLight">
        <rdf:type rdf:resource="http://hit2gap.eu/h2g/h2gBI#LampType"/>
    </owl:NamedIndividual>
    


    <!-- http://hit2gap.eu/h2g/h2gBI#ColdDesert -->

    <owl:NamedIndividual rdf:about="http://hit2gap.eu/h2g/h2gBI#ColdDesert">
        <rdf:type rdf:resource="http://hit2gap.eu/h2g/h2gBI#Arid"/>
    </owl:NamedIndividual>
    


    <!-- http://hit2gap.eu/h2g/h2gBI#ColdSemiArid -->

    <owl:NamedIndividual rdf:about="http://hit2gap.eu/h2g/h2gBI#ColdSemiArid">
        <rdf:type rdf:resource="http://hit2gap.eu/h2g/h2gBI#Arid"/>
    </owl:NamedIndividual>
    


    <!-- http://hit2gap.eu/h2g/h2gBI#CoolSummerMediterranean -->

    <owl:NamedIndividual rdf:about="http://hit2gap.eu/h2g/h2gBI#CoolSummerMediterranean">
        <rdf:type rdf:resource="http://hit2gap.eu/h2g/h2gBI#Temperate"/>
    </owl:NamedIndividual>
    


    <!-- http://hit2gap.eu/h2g/h2gBI#DeskLight -->

    <owl:NamedIndividual rdf:about="http://hit2gap.eu/h2g/h2gBI#DeskLight">
        <rdf:type rdf:resource="http://hit2gap.eu/h2g/h2gBI#LampType"/>
    </owl:NamedIndividual>
    


    <!-- http://hit2gap.eu/h2g/h2gBI#DrySummerSubartic -->

    <owl:NamedIndividual rdf:about="http://hit2gap.eu/h2g/h2gBI#DrySummerSubartic">
        <rdf:type rdf:resource="http://hit2gap.eu/h2g/h2gBI#Continental"/>
    </owl:NamedIndividual>
    


    <!-- http://hit2gap.eu/h2g/h2gBI#East -->

    <owl:NamedIndividual rdf:about="http://hit2gap.eu/h2g/h2gBI#East">
        <rdf:type rdf:resource="http://hit2gap.eu/h2g/h2gBI#Orientation"/>
    </owl:NamedIndividual>
    


    <!-- http://hit2gap.eu/h2g/h2gBI#ExtremelyColdDrySummerSubartic -->

    <owl:NamedIndividual rdf:about="http://hit2gap.eu/h2g/h2gBI#ExtremelyColdDrySummerSubartic">
        <rdf:type rdf:resource="http://hit2gap.eu/h2g/h2gBI#Continental"/>
    </owl:NamedIndividual>
    


    <!-- http://hit2gap.eu/h2g/h2gBI#ExtremelyColdSubartic -->

    <owl:NamedIndividual rdf:about="http://hit2gap.eu/h2g/h2gBI#ExtremelyColdSubartic">
        <rdf:type rdf:resource="http://hit2gap.eu/h2g/h2gBI#Continental"/>
    </owl:NamedIndividual>
    


    <!-- http://hit2gap.eu/h2g/h2gBI#FrostColdTundra -->

    <owl:NamedIndividual rdf:about="http://hit2gap.eu/h2g/h2gBI#FrostColdTundra">
        <rdf:type rdf:resource="http://hit2gap.eu/h2g/h2gBI#Polar"/>
    </owl:NamedIndividual>
    


    <!-- http://hit2gap.eu/h2g/h2gBI#HotDesert -->

    <owl:NamedIndividual rdf:about="http://hit2gap.eu/h2g/h2gBI#HotDesert">
        <rdf:type rdf:resource="http://hit2gap.eu/h2g/h2gBI#Arid"/>
    </owl:NamedIndividual>
    


    <!-- http://hit2gap.eu/h2g/h2gBI#HotDrySummerContinental -->

    <owl:NamedIndividual rdf:about="http://hit2gap.eu/h2g/h2gBI#HotDrySummerContinental">
        <rdf:type rdf:resource="http://hit2gap.eu/h2g/h2gBI#Continental"/>
    </owl:NamedIndividual>
    


    <!-- http://hit2gap.eu/h2g/h2gBI#HotSemiArid -->

    <owl:NamedIndividual rdf:about="http://hit2gap.eu/h2g/h2gBI#HotSemiArid">
        <rdf:type rdf:resource="http://hit2gap.eu/h2g/h2gBI#Arid"/>
    </owl:NamedIndividual>
    


    <!-- http://hit2gap.eu/h2g/h2gBI#HotSummerHumidContinental -->

    <owl:NamedIndividual rdf:about="http://hit2gap.eu/h2g/h2gBI#HotSummerHumidContinental">
        <rdf:type rdf:resource="http://hit2gap.eu/h2g/h2gBI#Continental"/>
    </owl:NamedIndividual>
    


    <!-- http://hit2gap.eu/h2g/h2gBI#HotSummerMediterranean -->

    <owl:NamedIndividual rdf:about="http://hit2gap.eu/h2g/h2gBI#HotSummerMediterranean">
        <rdf:type rdf:resource="http://hit2gap.eu/h2g/h2gBI#Temperate"/>
    </owl:NamedIndividual>
    


    <!-- http://hit2gap.eu/h2g/h2gBI#HumidSubtropical -->

    <owl:NamedIndividual rdf:about="http://hit2gap.eu/h2g/h2gBI#HumidSubtropical">
        <rdf:type rdf:resource="http://hit2gap.eu/h2g/h2gBI#Temperate"/>
    </owl:NamedIndividual>
    


    <!-- http://hit2gap.eu/h2g/h2gBI#IceCap -->

    <owl:NamedIndividual rdf:about="http://hit2gap.eu/h2g/h2gBI#IceCap">
        <rdf:type rdf:resource="http://hit2gap.eu/h2g/h2gBI#Polar"/>
    </owl:NamedIndividual>
    


    <!-- http://hit2gap.eu/h2g/h2gBI#MildDesert -->

    <owl:NamedIndividual rdf:about="http://hit2gap.eu/h2g/h2gBI#MildDesert">
        <rdf:type rdf:resource="http://hit2gap.eu/h2g/h2gBI#Arid"/>
    </owl:NamedIndividual>
    


    <!-- http://hit2gap.eu/h2g/h2gBI#MildSemiArid -->

    <owl:NamedIndividual rdf:about="http://hit2gap.eu/h2g/h2gBI#MildSemiArid">
        <rdf:type rdf:resource="http://hit2gap.eu/h2g/h2gBI#Arid"/>
    </owl:NamedIndividual>
    


    <!-- http://hit2gap.eu/h2g/h2gBI#MildTundra -->

    <owl:NamedIndividual rdf:about="http://hit2gap.eu/h2g/h2gBI#MildTundra">
        <rdf:type rdf:resource="http://hit2gap.eu/h2g/h2gBI#Polar"/>
    </owl:NamedIndividual>
    


    <!-- http://hit2gap.eu/h2g/h2gBI#MonsoonInfluencedExtremelyColdSubartic -->

    <owl:NamedIndividual rdf:about="http://hit2gap.eu/h2g/h2gBI#MonsoonInfluencedExtremelyColdSubartic">
        <rdf:type rdf:resource="http://hit2gap.eu/h2g/h2gBI#Continental"/>
    </owl:NamedIndividual>
    


    <!-- http://hit2gap.eu/h2g/h2gBI#MonsoonInfluencedHotSummerHumidContinental -->

    <owl:NamedIndividual rdf:about="http://hit2gap.eu/h2g/h2gBI#MonsoonInfluencedHotSummerHumidContinental">
        <rdf:type rdf:resource="http://hit2gap.eu/h2g/h2gBI#Continental"/>
    </owl:NamedIndividual>
    


    <!-- http://hit2gap.eu/h2g/h2gBI#MonsoonInfluencedHumidsubtropical -->

    <owl:NamedIndividual rdf:about="http://hit2gap.eu/h2g/h2gBI#MonsoonInfluencedHumidsubtropical">
        <rdf:type rdf:resource="http://hit2gap.eu/h2g/h2gBI#Temperate"/>
    </owl:NamedIndividual>
    


    <!-- http://hit2gap.eu/h2g/h2gBI#MonsoonInfluencedSubartic -->

    <owl:NamedIndividual rdf:about="http://hit2gap.eu/h2g/h2gBI#MonsoonInfluencedSubartic">
        <rdf:type rdf:resource="http://hit2gap.eu/h2g/h2gBI#Continental"/>
    </owl:NamedIndividual>
    


    <!-- http://hit2gap.eu/h2g/h2gBI#MonsoonInfluencedWarmSummerHumidContinental -->

    <owl:NamedIndividual rdf:about="http://hit2gap.eu/h2g/h2gBI#MonsoonInfluencedWarmSummerHumidContinental">
        <rdf:type rdf:resource="http://hit2gap.eu/h2g/h2gBI#Continental"/>
    </owl:NamedIndividual>
    


    <!-- http://hit2gap.eu/h2g/h2gBI#North -->

    <owl:NamedIndividual rdf:about="http://hit2gap.eu/h2g/h2gBI#North">
        <rdf:type rdf:resource="http://hit2gap.eu/h2g/h2gBI#Orientation"/>
    </owl:NamedIndividual>
    


    <!-- http://hit2gap.eu/h2g/h2gBI#North_East -->

    <owl:NamedIndividual rdf:about="http://hit2gap.eu/h2g/h2gBI#North_East">
        <rdf:type rdf:resource="http://hit2gap.eu/h2g/h2gBI#Orientation"/>
    </owl:NamedIndividual>
    


    <!-- http://hit2gap.eu/h2g/h2gBI#North_West -->

    <owl:NamedIndividual rdf:about="http://hit2gap.eu/h2g/h2gBI#North_West">
        <rdf:type rdf:resource="http://hit2gap.eu/h2g/h2gBI#Orientation"/>
    </owl:NamedIndividual>
    


    <!-- http://hit2gap.eu/h2g/h2gBI#OutdoorLight -->

    <owl:NamedIndividual rdf:about="http://hit2gap.eu/h2g/h2gBI#OutdoorLight">
        <rdf:type rdf:resource="http://hit2gap.eu/h2g/h2gBI#LampType"/>
    </owl:NamedIndividual>
    


    <!-- http://hit2gap.eu/h2g/h2gBI#South -->

    <owl:NamedIndividual rdf:about="http://hit2gap.eu/h2g/h2gBI#South">
        <rdf:type rdf:resource="http://hit2gap.eu/h2g/h2gBI#Orientation"/>
    </owl:NamedIndividual>
    


    <!-- http://hit2gap.eu/h2g/h2gBI#South_East -->

    <owl:NamedIndividual rdf:about="http://hit2gap.eu/h2g/h2gBI#South_East">
        <rdf:type rdf:resource="http://hit2gap.eu/h2g/h2gBI#Orientation"/>
    </owl:NamedIndividual>
    


    <!-- http://hit2gap.eu/h2g/h2gBI#South_West -->

    <owl:NamedIndividual rdf:about="http://hit2gap.eu/h2g/h2gBI#South_West">
        <rdf:type rdf:resource="http://hit2gap.eu/h2g/h2gBI#Orientation"/>
    </owl:NamedIndividual>
    


    <!-- http://hit2gap.eu/h2g/h2gBI#Subartic -->

    <owl:NamedIndividual rdf:about="http://hit2gap.eu/h2g/h2gBI#Subartic">
        <rdf:type rdf:resource="http://hit2gap.eu/h2g/h2gBI#Continental"/>
    </owl:NamedIndividual>
    


    <!-- http://hit2gap.eu/h2g/h2gBI#SubpolarOceanic -->

    <owl:NamedIndividual rdf:about="http://hit2gap.eu/h2g/h2gBI#SubpolarOceanic">
        <rdf:type rdf:resource="http://hit2gap.eu/h2g/h2gBI#Temperate"/>
    </owl:NamedIndividual>
    


    <!-- http://hit2gap.eu/h2g/h2gBI#SubpolarOceanicWithDryWinters -->

    <owl:NamedIndividual rdf:about="http://hit2gap.eu/h2g/h2gBI#SubpolarOceanicWithDryWinters">
        <rdf:type rdf:resource="http://hit2gap.eu/h2g/h2gBI#Temperate"/>
    </owl:NamedIndividual>
    


    <!-- http://hit2gap.eu/h2g/h2gBI#TemperateOceanic -->

    <owl:NamedIndividual rdf:about="http://hit2gap.eu/h2g/h2gBI#TemperateOceanic">
        <rdf:type rdf:resource="http://hit2gap.eu/h2g/h2gBI#Temperate"/>
    </owl:NamedIndividual>
    


    <!-- http://hit2gap.eu/h2g/h2gBI#TemperateOceanicWithDryWinters -->

    <owl:NamedIndividual rdf:about="http://hit2gap.eu/h2g/h2gBI#TemperateOceanicWithDryWinters">
        <rdf:type rdf:resource="http://hit2gap.eu/h2g/h2gBI#Temperate"/>
    </owl:NamedIndividual>
    


    <!-- http://hit2gap.eu/h2g/h2gBI#TropicalMonsoon -->

    <owl:NamedIndividual rdf:about="http://hit2gap.eu/h2g/h2gBI#TropicalMonsoon">
        <rdf:type rdf:resource="http://hit2gap.eu/h2g/h2gBI#Tropical"/>
    </owl:NamedIndividual>
    


    <!-- http://hit2gap.eu/h2g/h2gBI#TropicalRainforest -->

    <owl:NamedIndividual rdf:about="http://hit2gap.eu/h2g/h2gBI#TropicalRainforest">
        <rdf:type rdf:resource="http://hit2gap.eu/h2g/h2gBI#Tropical"/>
    </owl:NamedIndividual>
    


    <!-- http://hit2gap.eu/h2g/h2gBI#TropicalSavanna -->

    <owl:NamedIndividual rdf:about="http://hit2gap.eu/h2g/h2gBI#TropicalSavanna">
        <rdf:type rdf:resource="http://hit2gap.eu/h2g/h2gBI#Tropical"/>
    </owl:NamedIndividual>
    


    <!-- http://hit2gap.eu/h2g/h2gBI#WarmDrySummerContinental -->

    <owl:NamedIndividual rdf:about="http://hit2gap.eu/h2g/h2gBI#WarmDrySummerContinental">
        <rdf:type rdf:resource="http://hit2gap.eu/h2g/h2gBI#Continental"/>
    </owl:NamedIndividual>
    


    <!-- http://hit2gap.eu/h2g/h2gBI#WarmDrySummerMediterranean -->

    <owl:NamedIndividual rdf:about="http://hit2gap.eu/h2g/h2gBI#WarmDrySummerMediterranean"/>
    


    <!-- http://hit2gap.eu/h2g/h2gBI#WarmSummerHumidContinental -->

    <owl:NamedIndividual rdf:about="http://hit2gap.eu/h2g/h2gBI#WarmSummerHumidContinental">
        <rdf:type rdf:resource="http://hit2gap.eu/h2g/h2gBI#Continental"/>
    </owl:NamedIndividual>
    


    <!-- http://hit2gap.eu/h2g/h2gBI#WarmSummerMediterranean -->

    <owl:NamedIndividual rdf:about="http://hit2gap.eu/h2g/h2gBI#WarmSummerMediterranean">
        <rdf:type rdf:resource="http://hit2gap.eu/h2g/h2gBI#Temperate"/>
    </owl:NamedIndividual>
    


    <!-- http://hit2gap.eu/h2g/h2gBI#West -->

    <owl:NamedIndividual rdf:about="http://hit2gap.eu/h2g/h2gBI#West">
        <rdf:type rdf:resource="http://hit2gap.eu/h2g/h2gBI#Orientation"/>
    </owl:NamedIndividual>
    


    <!-- http://hit2gap.eu/h2g/h2gSensor#Northern -->

    <owl:NamedIndividual rdf:about="http://hit2gap.eu/h2g/h2gSensor#Northern">
        <rdf:type rdf:resource="http://hit2gap.eu/h2g/h2gSensor#Hemisphere"/>
        <rdfs:isDefinedBy xml:lang="en">http://hit2gap.eu/h2g/h2gSensor#Northern</rdfs:isDefinedBy>
    </owl:NamedIndividual>
    


    <!-- http://hit2gap.eu/h2g/h2gSensor#Southern -->

    <owl:NamedIndividual rdf:about="http://hit2gap.eu/h2g/h2gSensor#Southern">
        <rdf:type rdf:resource="http://hit2gap.eu/h2g/h2gSensor#Hemisphere"/>
        <rdfs:isDefinedBy xml:lang="en">http://hit2gap.eu/h2g/h2gSensor#Southern</rdfs:isDefinedBy>
    </owl:NamedIndividual>
    


    <!-- http://ifcowl.openbimstandards.org/IFC4_ADD2/index.html#SOLARCOLLECTOR -->

    <owl:NamedIndividual rdf:about="http://ifcowl.openbimstandards.org/IFC4_ADD2/index.html#SOLARCOLLECTOR">
        <rdf:type rdf:resource="http://ifcowl.openbimstandards.org/IFC4_ADD2/index.html#IfcSolarDevice"/>
        <rdfs:isDefinedBy xml:lang="en">http://ifcowl.openbimstandards.org/IFC4_ADD2/index.html#SOLARCOLLECTOR</rdfs:isDefinedBy>
    </owl:NamedIndividual>
    


    <!-- http://ifcowl.openbimstandards.org/IFC4_ADD2/index.html#SOLARELECTRIC -->

    <owl:NamedIndividual rdf:about="http://ifcowl.openbimstandards.org/IFC4_ADD2/index.html#SOLARELECTRIC">
        <rdf:type rdf:resource="http://ifcowl.openbimstandards.org/IFC4_ADD2/index.html#IfcSolarDevice"/>
        <rdfs:isDefinedBy xml:lang="en">http://ifcowl.openbimstandards.org/IFC4_ADD2/index.html#SOLARELECTRIC</rdfs:isDefinedBy>
    </owl:NamedIndividual>
    


    <!-- http://ifcowl.openbimstandards.org/IFC4_ADD2/index.html#SOLARPANEL -->

    <owl:NamedIndividual rdf:about="http://ifcowl.openbimstandards.org/IFC4_ADD2/index.html#SOLARPANEL">
        <rdf:type rdf:resource="http://ifcowl.openbimstandards.org/IFC4_ADD2/index.html#IfcSolarDevice"/>
        <rdfs:isDefinedBy xml:lang="en">http://ifcowl.openbimstandards.org/IFC4_ADD2/index.html#SOLARPANEL</rdfs:isDefinedBy>
    </owl:NamedIndividual>
    


    <!-- http://ifcowl.openbimstandards.org/IFC4_ADD2/index.html#SOLARTHERMAL -->

    <owl:NamedIndividual rdf:about="http://ifcowl.openbimstandards.org/IFC4_ADD2/index.html#SOLARTHERMAL">
        <rdf:type rdf:resource="http://ifcowl.openbimstandards.org/IFC4_ADD2/index.html#IfcSolarDevice"/>
        <rdfs:isDefinedBy xml:lang="en">http://ifcowl.openbimstandards.org/IFC4_ADD2/index.html#SOLARTHERMAL</rdfs:isDefinedBy>
    </owl:NamedIndividual>
</rdf:RDF>



<!-- Generated by the OWL API (version 4.2.8.20170104-2310) https://github.com/owlcs/owlapi -->

