<?xml version="1.0"?>
<rdf:RDF xmlns="http://hit2gap.eu/h2g/h2gProperty#"
     xml:base="http://hit2gap.eu/h2g/h2gProperty"
     xmlns:rdf="http://www.w3.org/1999/02/22-rdf-syntax-ns#"
     xmlns:terms="http://purl.org/dc/terms/"
     xmlns:owl="http://www.w3.org/2002/07/owl#"
     xmlns:xml="http://www.w3.org/XML/1998/namespace"
     xmlns:xsd="http://www.w3.org/2001/XMLSchema#"
     xmlns:rdfs="http://www.w3.org/2000/01/rdf-schema#"
     xmlns:dc="http://purl.org/dc/elements/1.1/">
    <owl:Ontology rdf:about="http://hit2gap.eu/h2g/h2gProperty#">
        <dc:creator xml:lang="en">Aitor Corchero (aitor.corchero@eurecat.org)</dc:creator>
        <dc:creator xml:lang="en">Pierre Bourreau (pbourreau@nobatek.com)</dc:creator>
        <dc:creator xml:lang="en">Richard Chbeir (richard.chbeir@univ-pau.fr)</dc:creator>
        <dc:creator xml:lang="en">Yudith Cardinale (ycardinale@usb.ve)</dc:creator>
        <dc:description xml:lang="en">This semantic model is focused on representing the phenomenon (or property), which provides a common vision about the general characteristics to be considered in the building. This model is an extension of the “ssn:Property” representation. Two main families of characteristics were considered: economic and physical properties.</dc:description>
        <dc:title xml:lang="en">Hit2Gap Ontology-Property</dc:title>
        <terms:license xml:lang="en">https://opensource.org/licenses/MIT</terms:license>
        <owl:versionInfo xml:lang="en">This current version includes the initial version of the semantic model based on the diagrams generated.</owl:versionInfo>
    </owl:Ontology>
    


    <!-- 
    ///////////////////////////////////////////////////////////////////////////////////////
    //
    // Annotation properties
    //
    ///////////////////////////////////////////////////////////////////////////////////////
     -->

    


    <!-- http://purl.org/dc/elements/1.1/contributor -->

    <owl:AnnotationProperty rdf:about="http://purl.org/dc/elements/1.1/contributor"/>
    


    <!-- http://purl.org/dc/elements/1.1/creator -->

    <owl:AnnotationProperty rdf:about="http://purl.org/dc/elements/1.1/creator"/>
    


    <!-- http://purl.org/dc/elements/1.1/description -->

    <owl:AnnotationProperty rdf:about="http://purl.org/dc/elements/1.1/description"/>
    


    <!-- http://purl.org/dc/elements/1.1/title -->

    <owl:AnnotationProperty rdf:about="http://purl.org/dc/elements/1.1/title"/>
    


    <!-- http://purl.org/dc/terms/license -->

    <owl:AnnotationProperty rdf:about="http://purl.org/dc/terms/license"/>
    


    <!-- 
    ///////////////////////////////////////////////////////////////////////////////////////
    //
    // Object Properties
    //
    ///////////////////////////////////////////////////////////////////////////////////////
     -->

    


    <!-- http://hit2gap.eu/h2g/h2gProperty#hasSpaceCapacity -->

    <owl:ObjectProperty rdf:about="http://hit2gap.eu/h2g/h2gProperty#hasSpaceCapacity"/>
    


    <!-- 
    ///////////////////////////////////////////////////////////////////////////////////////
    //
    // Classes
    //
    ///////////////////////////////////////////////////////////////////////////////////////
     -->

    


    <!-- http://hit2gap.eu/h2g/h2gProperty#AbsorbedIncidentRadiation -->

    <owl:Class rdf:about="http://hit2gap.eu/h2g/h2gProperty#AbsorbedIncidentRadiation">
        <rdfs:subClassOf rdf:resource="http://hit2gap.eu/h2g/h2gProperty#IncidentRadiation"/>
        <rdfs:comment xml:lang="en">AbsorbedIncidentRadiation represents an observation of the  measure of the absorbed incident radiation  in a specific time.</rdfs:comment>
        <rdfs:label xml:lang="en">AbsorbedIncidentRadiation</rdfs:label>
    </owl:Class>
    


    <!-- http://hit2gap.eu/h2g/h2gProperty#AbsorbedScatteredIncidentRadiation -->

    <owl:Class rdf:about="http://hit2gap.eu/h2g/h2gProperty#AbsorbedScatteredIncidentRadiation">
        <rdfs:subClassOf rdf:resource="http://hit2gap.eu/h2g/h2gProperty#IncidentRadiation"/>
        <rdfs:comment xml:lang="en">AbsorbedScatteredIncidentRadiation represents an observation of the  measure of the absorbed scattered incident radiation  in a specific time.</rdfs:comment>
        <rdfs:label xml:lang="en">AbsorbedScatteredIncidentRadiation</rdfs:label>
    </owl:Class>
    


    <!-- http://hit2gap.eu/h2g/h2gProperty#AirQuality -->

    <owl:Class rdf:about="http://hit2gap.eu/h2g/h2gProperty#AirQuality">
        <rdfs:subClassOf rdf:resource="http://hit2gap.eu/h2g/h2gProperty#PhysicalProperties"/>
        <rdfs:comment xml:lang="en">AirQuality represents an observation of the  measure of the air quality in a specific time.</rdfs:comment>
        <rdfs:label xml:lang="en">AirQuality</rdfs:label>
    </owl:Class>
    


    <!-- http://hit2gap.eu/h2g/h2gProperty#Altitude -->

    <owl:Class rdf:about="http://hit2gap.eu/h2g/h2gProperty#Altitude">
        <rdfs:subClassOf rdf:resource="http://hit2gap.eu/h2g/h2gProperty#Position"/>
        <rdfs:comment xml:lang="en">Altitude represents an observation of the  measure of the position altitude  of an element in the building  in a specific time.</rdfs:comment>
        <rdfs:label xml:lang="en">Altitude</rdfs:label>
    </owl:Class>
    


    <!-- http://hit2gap.eu/h2g/h2gProperty#Area -->

    <owl:Class rdf:about="http://hit2gap.eu/h2g/h2gProperty#Area">
        <rdfs:subClassOf rdf:resource="http://hit2gap.eu/h2g/h2gProperty#PhysicalProperties"/>
        <rdfs:comment xml:lang="en">Area represents an observation of the  measure of the area.</rdfs:comment>
        <rdfs:label xml:lang="en">Area</rdfs:label>
    </owl:Class>
    


    <!-- http://hit2gap.eu/h2g/h2gProperty#Arid -->

    <owl:Class rdf:about="http://hit2gap.eu/h2g/h2gProperty#Arid">
        <rdfs:subClassOf rdf:resource="http://hit2gap.eu/h2g/h2gProperty#Climate"/>
        <rdfs:comment xml:lang="en">Arid represents an observation of the arid climate in a specific time.</rdfs:comment>
        <rdfs:label xml:lang="en">Arid</rdfs:label>
    </owl:Class>
    


    <!-- http://hit2gap.eu/h2g/h2gProperty#Capacity -->

    <owl:Class rdf:about="http://hit2gap.eu/h2g/h2gProperty#Capacity">
        <rdfs:subClassOf rdf:resource="http://hit2gap.eu/h2g/h2gProperty#PhysicalProperties"/>
        <rdfs:comment xml:lang="en">Capacity represents an observation of the  measure of the capacity of an elment in the building.</rdfs:comment>
        <rdfs:label xml:lang="en">Capacity</rdfs:label>
    </owl:Class>
    


    <!-- http://hit2gap.eu/h2g/h2gProperty#Climate -->

    <owl:Class rdf:about="http://hit2gap.eu/h2g/h2gProperty#Climate">
        <rdfs:subClassOf rdf:resource="http://hit2gap.eu/h2g/h2gProperty#PhysicalProperties"/>
        <rdfs:comment xml:lang="en">Climate represents an observation of the climate  in a specific time.</rdfs:comment>
        <rdfs:label xml:lang="en">Climate</rdfs:label>
    </owl:Class>
    


    <!-- http://hit2gap.eu/h2g/h2gProperty#Co2Rate -->

    <owl:Class rdf:about="http://hit2gap.eu/h2g/h2gProperty#Co2Rate">
        <rdfs:subClassOf rdf:resource="http://hit2gap.eu/h2g/h2gProperty#PhysicalProperties"/>
        <rdfs:comment xml:lang="en">Co2Rate represents an observation of the  measure of the Co2 in the building in a specific time.</rdfs:comment>
        <rdfs:label xml:lang="en">Co2Rate</rdfs:label>
    </owl:Class>
    


    <!-- http://hit2gap.eu/h2g/h2gProperty#Color -->

    <owl:Class rdf:about="http://hit2gap.eu/h2g/h2gProperty#Color">
        <rdfs:subClassOf rdf:resource="http://hit2gap.eu/h2g/h2gProperty#PhysicalProperties"/>
        <rdfs:comment xml:lang="en">Color represents an observation of the  value of the color of an elment in the building in a specific time.</rdfs:comment>
        <rdfs:label xml:lang="en">Color</rdfs:label>
    </owl:Class>
    


    <!-- http://hit2gap.eu/h2g/h2gProperty#Condensation -->

    <owl:Class rdf:about="http://hit2gap.eu/h2g/h2gProperty#Condensation">
        <rdfs:subClassOf rdf:resource="http://hit2gap.eu/h2g/h2gProperty#PhysicalProperties"/>
        <rdfs:comment xml:lang="en">Condensation represents an observation of the  measure of the condensation  in a specific time.</rdfs:comment>
        <rdfs:label xml:lang="en">Condensation</rdfs:label>
    </owl:Class>
    


    <!-- http://hit2gap.eu/h2g/h2gProperty#Conductivity -->

    <owl:Class rdf:about="http://hit2gap.eu/h2g/h2gProperty#Conductivity">
        <rdfs:subClassOf rdf:resource="http://hit2gap.eu/h2g/h2gProperty#PhysicalProperties"/>
        <rdfs:comment xml:lang="en">Conductivity represents an observation of the  measure of the conductivity of an element  in the building in a specific time.</rdfs:comment>
        <rdfs:label xml:lang="en">Conductivity</rdfs:label>
    </owl:Class>
    


    <!-- http://hit2gap.eu/h2g/h2gProperty#Continental -->

    <owl:Class rdf:about="http://hit2gap.eu/h2g/h2gProperty#Continental">
        <rdfs:subClassOf rdf:resource="http://hit2gap.eu/h2g/h2gProperty#Climate"/>
        <rdfs:comment xml:lang="en">Continental represents an observation of the continental climate in a specific time.</rdfs:comment>
        <rdfs:label xml:lang="en">Continental</rdfs:label>
    </owl:Class>
    


    <!-- http://hit2gap.eu/h2g/h2gProperty#ContinousState -->

    <owl:Class rdf:about="http://hit2gap.eu/h2g/h2gProperty#ContinousState">
        <rdfs:subClassOf rdf:resource="http://hit2gap.eu/h2g/h2gProperty#DistributionElementState"/>
        <rdfs:comment xml:lang="en">Represents an observation of a continuous state.</rdfs:comment>
        <rdfs:label xml:lang="en">ContinousState</rdfs:label>
    </owl:Class>
    


    <!-- http://hit2gap.eu/h2g/h2gProperty#Cost -->

    <owl:Class rdf:about="http://hit2gap.eu/h2g/h2gProperty#Cost">
        <rdfs:subClassOf rdf:resource="http://hit2gap.eu/h2g/h2gProperty#EconomicProperties"/>
        <rdfs:comment xml:lang="en">Costs captures the investment costs of the building.</rdfs:comment>
        <rdfs:label xml:lang="en">Cost</rdfs:label>
    </owl:Class>
    


    <!-- http://hit2gap.eu/h2g/h2gProperty#CrossSection -->

    <owl:Class rdf:about="http://hit2gap.eu/h2g/h2gProperty#CrossSection">
        <rdfs:subClassOf rdf:resource="http://hit2gap.eu/h2g/h2gProperty#Shape"/>
        <rdfs:comment xml:lang="en">CrossSection represents an observation of the  cross section of an elment in the building.</rdfs:comment>
        <rdfs:label xml:lang="en">CrossSection</rdfs:label>
    </owl:Class>
    


    <!-- http://hit2gap.eu/h2g/h2gProperty#Density -->

    <owl:Class rdf:about="http://hit2gap.eu/h2g/h2gProperty#Density">
        <rdfs:subClassOf rdf:resource="http://hit2gap.eu/h2g/h2gProperty#PhysicalProperties"/>
        <rdfs:comment xml:lang="en">Density represents an observation of the  measure of the density of an element  in the building in a specific time.</rdfs:comment>
        <rdfs:label xml:lang="en">Density</rdfs:label>
    </owl:Class>
    


    <!-- http://hit2gap.eu/h2g/h2gProperty#Depth -->

    <owl:Class rdf:about="http://hit2gap.eu/h2g/h2gProperty#Depth">
        <rdfs:subClassOf rdf:resource="http://hit2gap.eu/h2g/h2gProperty#PhysicalProperties"/>
        <rdfs:comment xml:lang="en">Depth represents an observation of the  measure of the depth of an element  in the building in a specific time.</rdfs:comment>
        <rdfs:label xml:lang="en">Depth</rdfs:label>
    </owl:Class>
    


    <!-- http://hit2gap.eu/h2g/h2gProperty#Discharge -->

    <owl:Class rdf:about="http://hit2gap.eu/h2g/h2gProperty#Discharge">
        <rdfs:subClassOf rdf:resource="http://hit2gap.eu/h2g/h2gProperty#Volume"/>
        <rdfs:comment xml:lang="en">Discharge represents an observation of the  measure of the volume of a discharge in the building in a specific time.</rdfs:comment>
        <rdfs:label xml:lang="en">Discharge</rdfs:label>
    </owl:Class>
    


    <!-- http://hit2gap.eu/h2g/h2gProperty#DiscreteState -->

    <owl:Class rdf:about="http://hit2gap.eu/h2g/h2gProperty#DiscreteState">
        <rdfs:subClassOf rdf:resource="http://hit2gap.eu/h2g/h2gProperty#DistributionElementState"/>
        <rdfs:comment xml:lang="en">Represents an observation of a discrete state.</rdfs:comment>
        <rdfs:label xml:lang="en">DiscreteState</rdfs:label>
    </owl:Class>
    


    <!-- http://hit2gap.eu/h2g/h2gProperty#DistributionElementState -->

    <owl:Class rdf:about="http://hit2gap.eu/h2g/h2gProperty#DistributionElementState">
        <rdfs:subClassOf rdf:resource="http://hit2gap.eu/h2g/h2gProperty#State"/>
        <rdfs:comment xml:lang="en">DistributionElementState represents an observation of the  state of a distribution element in the building.</rdfs:comment>
        <rdfs:label>DistributionElementState</rdfs:label>
    </owl:Class>
    


    <!-- http://hit2gap.eu/h2g/h2gProperty#EconomicProperties -->

    <owl:Class rdf:about="http://hit2gap.eu/h2g/h2gProperty#EconomicProperties">
        <rdfs:subClassOf rdf:resource="http://purl.oclc.org/NET/ssnx/ssn#Property"/>
        <rdfs:comment xml:lang="en">The Economic phenomena makes reference to all monetary and investment aspects that could affect the building domains. For example, this part of the ontology allows one to represent water-related prices, energy bills, building investments, etc. These specific phenomena has been subdivided into: Cost and Investment.</rdfs:comment>
        <rdfs:label xml:lang="en">EconomicProperties</rdfs:label>
    </owl:Class>
    


    <!-- http://hit2gap.eu/h2g/h2gProperty#Evaporation -->

    <owl:Class rdf:about="http://hit2gap.eu/h2g/h2gProperty#Evaporation">
        <rdfs:subClassOf rdf:resource="http://hit2gap.eu/h2g/h2gProperty#PhysicalProperties"/>
        <rdfs:comment xml:lang="en">Evaporation represents an observation of the  measure of the evaporation in a specific time.</rdfs:comment>
        <rdfs:label xml:lang="en">Evaporation</rdfs:label>
    </owl:Class>
    


    <!-- http://hit2gap.eu/h2g/h2gProperty#Flow -->

    <owl:Class rdf:about="http://hit2gap.eu/h2g/h2gProperty#Flow">
        <rdfs:subClassOf rdf:resource="http://hit2gap.eu/h2g/h2gProperty#Volume"/>
        <rdfs:comment xml:lang="en">Flow represents an observation of the  measure of the volume of a flow in the building in a specific time.</rdfs:comment>
        <rdfs:label xml:lang="en">Flow</rdfs:label>
    </owl:Class>
    


    <!-- http://hit2gap.eu/h2g/h2gProperty#Height -->

    <owl:Class rdf:about="http://hit2gap.eu/h2g/h2gProperty#Height">
        <rdfs:subClassOf rdf:resource="http://hit2gap.eu/h2g/h2gProperty#Shape"/>
        <rdfs:comment xml:lang="en">Height represents an observation of the  height of an elment in the building.</rdfs:comment>
        <rdfs:label xml:lang="en">Height</rdfs:label>
    </owl:Class>
    


    <!-- http://hit2gap.eu/h2g/h2gProperty#Humidity -->

    <owl:Class rdf:about="http://hit2gap.eu/h2g/h2gProperty#Humidity">
        <rdfs:subClassOf rdf:resource="http://hit2gap.eu/h2g/h2gProperty#PhysicalProperties"/>
        <rdfs:comment xml:lang="en">Humidity represents an observation of the  measure of the humidity in a specific time.</rdfs:comment>
        <rdfs:label xml:lang="en">Humidity</rdfs:label>
    </owl:Class>
    


    <!-- http://hit2gap.eu/h2g/h2gProperty#IncidentRadiation -->

    <owl:Class rdf:about="http://hit2gap.eu/h2g/h2gProperty#IncidentRadiation">
        <rdfs:subClassOf rdf:resource="http://hit2gap.eu/h2g/h2gProperty#Radiation"/>
        <rdfs:comment xml:lang="en">IncidentRadiation represents an observation of the  measure of the incident radiation  in a specific time.</rdfs:comment>
        <rdfs:label xml:lang="en">IncidentRadiation</rdfs:label>
    </owl:Class>
    


    <!-- http://hit2gap.eu/h2g/h2gProperty#Inflow -->

    <owl:Class rdf:about="http://hit2gap.eu/h2g/h2gProperty#Inflow">
        <rdfs:subClassOf rdf:resource="http://hit2gap.eu/h2g/h2gProperty#Flow"/>
        <rdfs:comment xml:lang="en">Inflow represents an observation of the  measure of the volume of an input flow in the building in a specific time.</rdfs:comment>
        <rdfs:label xml:lang="en">Inflow</rdfs:label>
    </owl:Class>
    


    <!-- http://hit2gap.eu/h2g/h2gProperty#Intensity -->

    <owl:Class rdf:about="http://hit2gap.eu/h2g/h2gProperty#Intensity">
        <rdfs:subClassOf rdf:resource="http://hit2gap.eu/h2g/h2gProperty#PhysicalProperties"/>
        <rdfs:comment xml:lang="en">Intensity represents an observation of the  measure of the intensity in a specific time.</rdfs:comment>
        <rdfs:label xml:lang="en">Intensity</rdfs:label>
    </owl:Class>
    


    <!-- http://hit2gap.eu/h2g/h2gProperty#Investment -->

    <owl:Class rdf:about="http://hit2gap.eu/h2g/h2gProperty#Investment">
        <rdfs:subClassOf rdf:resource="http://hit2gap.eu/h2g/h2gProperty#EconomicProperties"/>
        <rdfs:comment xml:lang="en">Investment represents the building investment aspects and information.</rdfs:comment>
        <rdfs:label xml:lang="en">Investment</rdfs:label>
    </owl:Class>
    


    <!-- http://hit2gap.eu/h2g/h2gProperty#Latitude -->

    <owl:Class rdf:about="http://hit2gap.eu/h2g/h2gProperty#Latitude">
        <rdfs:subClassOf rdf:resource="http://hit2gap.eu/h2g/h2gProperty#Position"/>
        <rdfs:comment xml:lang="en">Latitude represents an observation of the  measure of the position latitude  of an element in the building  in a specific time.</rdfs:comment>
        <rdfs:label xml:lang="en">Latitude</rdfs:label>
    </owl:Class>
    


    <!-- http://hit2gap.eu/h2g/h2gProperty#Length -->

    <owl:Class rdf:about="http://hit2gap.eu/h2g/h2gProperty#Length">
        <rdfs:subClassOf rdf:resource="http://hit2gap.eu/h2g/h2gProperty#Shape"/>
        <rdfs:comment xml:lang="en">Length represents an observation of the  length of an elment in the building.</rdfs:comment>
        <rdfs:label xml:lang="en">Length</rdfs:label>
    </owl:Class>
    


    <!-- http://hit2gap.eu/h2g/h2gProperty#LightRadiation -->

    <owl:Class rdf:about="http://hit2gap.eu/h2g/h2gProperty#LightRadiation">
        <rdfs:subClassOf rdf:resource="http://hit2gap.eu/h2g/h2gProperty#Radiation"/>
        <rdfs:comment xml:lang="en">LightRadiation represents an observation of the  measure of the light radiation  in a specific time.</rdfs:comment>
        <rdfs:label xml:lang="en">LightRadiation</rdfs:label>
    </owl:Class>
    


    <!-- http://hit2gap.eu/h2g/h2gProperty#Longitude -->

    <owl:Class rdf:about="http://hit2gap.eu/h2g/h2gProperty#Longitude">
        <rdfs:subClassOf rdf:resource="http://hit2gap.eu/h2g/h2gProperty#Position"/>
        <rdfs:comment xml:lang="en">longitude represents an observation of the  measure of the position longitude  of an element in the building  in a specific time.</rdfs:comment>
        <rdfs:label xml:lang="en">Longitude</rdfs:label>
    </owl:Class>
    


    <!-- http://hit2gap.eu/h2g/h2gProperty#OccupantStateProperties -->

    <owl:Class rdf:about="http://hit2gap.eu/h2g/h2gProperty#OccupantStateProperties">
        <rdfs:subClassOf rdf:resource="http://purl.oclc.org/NET/ssnx/ssn#Property"/>
        <rdfs:comment xml:lang="en">The occupant Properties describes the state of an occupant of the building. For example, this part of the ontology allows to represent the pulse and stress of an occupant.</rdfs:comment>
        <rdfs:label xml:lang="en">OccupantStateProperties</rdfs:label>
    </owl:Class>
    


    <!-- http://hit2gap.eu/h2g/h2gProperty#Outflow -->

    <owl:Class rdf:about="http://hit2gap.eu/h2g/h2gProperty#Outflow">
        <rdfs:subClassOf rdf:resource="http://hit2gap.eu/h2g/h2gProperty#Flow"/>
        <rdfs:comment xml:lang="en">Outflow represents an observation of the  measure of the volume of an output flow in the building in a specific time.</rdfs:comment>
        <rdfs:label xml:lang="en">Outflow</rdfs:label>
    </owl:Class>
    


    <!-- http://hit2gap.eu/h2g/h2gProperty#PhysicalProperties -->

    <owl:Class rdf:about="http://hit2gap.eu/h2g/h2gProperty#PhysicalProperties">
        <rdfs:subClassOf rdf:resource="http://purl.oclc.org/NET/ssnx/ssn#Property"/>
        <rdfs:comment xml:lang="en">Physical properties represent all related physical aspects that can be observed: dimensional, volumetric, and radiation aspects that influence on the building and occupant behaviour. These phenomena support the alignment and fusion of specific observations based on general measurements (e.g. temperature, volume, etc.).</rdfs:comment>
        <rdfs:label xml:lang="en">PhysicProperties</rdfs:label>
    </owl:Class>
    


    <!-- http://hit2gap.eu/h2g/h2gProperty#Polar -->

    <owl:Class rdf:about="http://hit2gap.eu/h2g/h2gProperty#Polar">
        <rdfs:subClassOf rdf:resource="http://hit2gap.eu/h2g/h2gProperty#Climate"/>
        <rdfs:comment xml:lang="en">Polar represents an observation of the polar climate in a specific time.</rdfs:comment>
        <rdfs:label xml:lang="en">Polar</rdfs:label>
    </owl:Class>
    


    <!-- http://hit2gap.eu/h2g/h2gProperty#Position -->

    <owl:Class rdf:about="http://hit2gap.eu/h2g/h2gProperty#Position">
        <rdfs:subClassOf rdf:resource="http://hit2gap.eu/h2g/h2gProperty#PhysicalProperties"/>
        <rdfs:comment xml:lang="en">Position represents an observation of the  measure of the position of an element in the building  in a specific time.</rdfs:comment>
        <rdfs:label xml:lang="en">Position</rdfs:label>
    </owl:Class>
    


    <!-- http://hit2gap.eu/h2g/h2gProperty#Pressure -->

    <owl:Class rdf:about="http://hit2gap.eu/h2g/h2gProperty#Pressure">
        <rdfs:subClassOf rdf:resource="http://hit2gap.eu/h2g/h2gProperty#PhysicalProperties"/>
        <rdfs:comment xml:lang="en">Pressure represents an observation of the  measure of the pressure in a specific time.</rdfs:comment>
        <rdfs:label xml:lang="en">Pressure</rdfs:label>
    </owl:Class>
    


    <!-- http://hit2gap.eu/h2g/h2gProperty#ProductionCapacity -->

    <owl:Class rdf:about="http://hit2gap.eu/h2g/h2gProperty#ProductionCapacity">
        <rdfs:subClassOf rdf:resource="http://hit2gap.eu/h2g/h2gProperty#Capacity"/>
        <rdfs:comment xml:lang="en">ProductionCapacity represents an observation of the  measure of the capacity of production of an elment in the building.</rdfs:comment>
        <rdfs:label xml:lang="en">ProductionCapacity</rdfs:label>
    </owl:Class>
    


    <!-- http://hit2gap.eu/h2g/h2gProperty#Pulse -->

    <owl:Class rdf:about="http://hit2gap.eu/h2g/h2gProperty#Pulse">
        <rdfs:subClassOf rdf:resource="http://hit2gap.eu/h2g/h2gProperty#OccupantStateProperties"/>
        <rdfs:comment xml:lang="en">Pulse represents an observation of the  measure of the pulse of an occupant of the building in a specific time.</rdfs:comment>
        <rdfs:label xml:lang="en">Pulse</rdfs:label>
    </owl:Class>
    


    <!-- http://hit2gap.eu/h2g/h2gProperty#Radiation -->

    <owl:Class rdf:about="http://hit2gap.eu/h2g/h2gProperty#Radiation">
        <rdfs:subClassOf rdf:resource="http://hit2gap.eu/h2g/h2gProperty#PhysicalProperties"/>
        <rdfs:comment xml:lang="en">Radiation represents an observation of the  measure of the radiation  in a specific time.</rdfs:comment>
        <rdfs:label xml:lang="en">Radiation</rdfs:label>
    </owl:Class>
    


    <!-- http://hit2gap.eu/h2g/h2gProperty#Rainfall -->

    <owl:Class rdf:about="http://hit2gap.eu/h2g/h2gProperty#Rainfall">
        <rdfs:subClassOf rdf:resource="http://hit2gap.eu/h2g/h2gProperty#PhysicalProperties"/>
        <rdfs:comment xml:lang="en">Rainfall represents an observation of the  measure of the rainfall.</rdfs:comment>
        <rdfs:label xml:lang="en">Rainfall</rdfs:label>
    </owl:Class>
    


    <!-- http://hit2gap.eu/h2g/h2gProperty#ReflectedIncidentradiation -->

    <owl:Class rdf:about="http://hit2gap.eu/h2g/h2gProperty#ReflectedIncidentradiation">
        <rdfs:subClassOf rdf:resource="http://hit2gap.eu/h2g/h2gProperty#IncidentRadiation"/>
        <rdfs:comment xml:lang="en">ReflectedIncidentRadiation represents an observation of the  measure of the reflected incident radiation  in a specific time.</rdfs:comment>
        <rdfs:label xml:lang="en">ReflectedIncidentRadiation</rdfs:label>
    </owl:Class>
    


    <!-- http://hit2gap.eu/h2g/h2gProperty#Reflectivity -->

    <owl:Class rdf:about="http://hit2gap.eu/h2g/h2gProperty#Reflectivity">
        <rdfs:subClassOf rdf:resource="http://hit2gap.eu/h2g/h2gProperty#PhysicalProperties"/>
        <rdfs:comment xml:lang="en">Reflectivity represents an observation of the  reflectivity of an elment in the building.</rdfs:comment>
        <rdfs:label xml:lang="en">Reflectivity</rdfs:label>
    </owl:Class>
    


    <!-- http://hit2gap.eu/h2g/h2gProperty#Shape -->

    <owl:Class rdf:about="http://hit2gap.eu/h2g/h2gProperty#Shape">
        <rdfs:subClassOf rdf:resource="http://hit2gap.eu/h2g/h2gProperty#PhysicalProperties"/>
        <rdfs:comment xml:lang="en">Shape represents an observation of the  measure of the shape of an elment in the building.</rdfs:comment>
        <rdfs:label xml:lang="en">Shape</rdfs:label>
    </owl:Class>
    


    <!-- http://hit2gap.eu/h2g/h2gProperty#Slope -->

    <owl:Class rdf:about="http://hit2gap.eu/h2g/h2gProperty#Slope">
        <rdfs:subClassOf rdf:resource="http://hit2gap.eu/h2g/h2gProperty#Shape"/>
        <rdfs:comment xml:lang="en">Slope represents an observation of the  slope of an elment in the building.</rdfs:comment>
        <rdfs:label xml:lang="en">Slope</rdfs:label>
    </owl:Class>
    


    <!-- http://hit2gap.eu/h2g/h2gProperty#SpaceCapacity -->

    <owl:Class rdf:about="http://hit2gap.eu/h2g/h2gProperty#SpaceCapacity">
        <rdfs:subClassOf rdf:resource="http://hit2gap.eu/h2g/h2gProperty#Capacity"/>
        <rdfs:comment xml:lang="en">SpaceCapacity represents an observation of the  measure of the capacity of the space  in the building.</rdfs:comment>
        <rdfs:label xml:lang="en">SpaceCapacity</rdfs:label>
    </owl:Class>
    


    <!-- http://hit2gap.eu/h2g/h2gProperty#Speed -->

    <owl:Class rdf:about="http://hit2gap.eu/h2g/h2gProperty#Speed">
        <rdfs:subClassOf rdf:resource="http://hit2gap.eu/h2g/h2gProperty#PhysicalProperties"/>
        <rdfs:comment xml:lang="en">Speed represents an observation of the  measure of the speed of an elment in the building in a specific time.</rdfs:comment>
        <rdfs:label xml:lang="en">Speed</rdfs:label>
    </owl:Class>
    


    <!-- http://hit2gap.eu/h2g/h2gProperty#State -->

    <owl:Class rdf:about="http://hit2gap.eu/h2g/h2gProperty#State">
        <rdfs:subClassOf rdf:resource="http://hit2gap.eu/h2g/h2gProperty#PhysicalProperties"/>
        <rdfs:comment xml:lang="en">State represents an observation of the  state of an element in the building.</rdfs:comment>
        <rdfs:label xml:lang="en">State</rdfs:label>
    </owl:Class>
    


    <!-- http://hit2gap.eu/h2g/h2gProperty#Streess -->

    <owl:Class rdf:about="http://hit2gap.eu/h2g/h2gProperty#Streess">
        <rdfs:subClassOf rdf:resource="http://hit2gap.eu/h2g/h2gProperty#OccupantStateProperties"/>
        <rdfs:comment xml:lang="en">Stress represents an observation of the  measure of the stress of an occupant of the building in a specific time.</rdfs:comment>
        <rdfs:label xml:lang="en">Stress</rdfs:label>
    </owl:Class>
    


    <!-- http://hit2gap.eu/h2g/h2gProperty#Temperate -->

    <owl:Class rdf:about="http://hit2gap.eu/h2g/h2gProperty#Temperate">
        <rdfs:subClassOf rdf:resource="http://hit2gap.eu/h2g/h2gProperty#Climate"/>
        <rdfs:comment xml:lang="en">Temperate represents an observation of the temperate climate in a specific time.</rdfs:comment>
        <rdfs:label xml:lang="en">Temperate</rdfs:label>
    </owl:Class>
    


    <!-- http://hit2gap.eu/h2g/h2gProperty#Temperature -->

    <owl:Class rdf:about="http://hit2gap.eu/h2g/h2gProperty#Temperature">
        <rdfs:subClassOf rdf:resource="http://hit2gap.eu/h2g/h2gProperty#PhysicalProperties"/>
        <rdfs:comment xml:lang="en">Temperature represents an observation of the  measure of the temperature  in a specific time.</rdfs:comment>
        <rdfs:label xml:lang="en">Temperature</rdfs:label>
    </owl:Class>
    


    <!-- http://hit2gap.eu/h2g/h2gProperty#Tension -->

    <owl:Class rdf:about="http://hit2gap.eu/h2g/h2gProperty#Tension">
        <rdfs:subClassOf rdf:resource="http://hit2gap.eu/h2g/h2gProperty#PhysicalProperties"/>
        <rdfs:comment xml:lang="en">Tension represents an observation of the  measure of the tension of an element in the building.</rdfs:comment>
        <rdfs:label xml:lang="en">Tension</rdfs:label>
    </owl:Class>
    


    <!-- http://hit2gap.eu/h2g/h2gProperty#Time -->

    <owl:Class rdf:about="http://hit2gap.eu/h2g/h2gProperty#Time">
        <rdfs:subClassOf rdf:resource="http://hit2gap.eu/h2g/h2gProperty#PhysicalProperties"/>
        <rdfs:comment xml:lang="en">Time represents an observation of the  measure of the time.</rdfs:comment>
        <rdfs:label xml:lang="en">Time</rdfs:label>
    </owl:Class>
    


    <!-- http://hit2gap.eu/h2g/h2gProperty#TransmittedIncidentRadiation -->

    <owl:Class rdf:about="http://hit2gap.eu/h2g/h2gProperty#TransmittedIncidentRadiation">
        <rdfs:subClassOf rdf:resource="http://hit2gap.eu/h2g/h2gProperty#IncidentRadiation"/>
        <rdfs:comment xml:lang="en">TransmittedIncidentRadiation represents an observation of the  measure of the transmittedincident radiation  in a specific time.</rdfs:comment>
        <rdfs:label xml:lang="en">TransmittedIncidentRadiation</rdfs:label>
    </owl:Class>
    


    <!-- http://hit2gap.eu/h2g/h2gProperty#Transparency -->

    <owl:Class rdf:about="http://hit2gap.eu/h2g/h2gProperty#Transparency">
        <rdfs:subClassOf rdf:resource="http://hit2gap.eu/h2g/h2gProperty#PhysicalProperties"/>
        <rdfs:comment xml:lang="en">Transparency represents an observation of the  measure of the transparence of an elment in the building in a specific time.</rdfs:comment>
        <rdfs:label xml:lang="en">Transparency</rdfs:label>
    </owl:Class>
    


    <!-- http://hit2gap.eu/h2g/h2gProperty#Tropical -->

    <owl:Class rdf:about="http://hit2gap.eu/h2g/h2gProperty#Tropical">
        <rdfs:subClassOf rdf:resource="http://hit2gap.eu/h2g/h2gProperty#Climate"/>
        <rdfs:comment xml:lang="en">Tropical represents an observation of the tropical climate in a specific time.</rdfs:comment>
        <rdfs:label xml:lang="en">Tropical</rdfs:label>
    </owl:Class>
    


    <!-- http://hit2gap.eu/h2g/h2gProperty#Velocity -->

    <owl:Class rdf:about="http://hit2gap.eu/h2g/h2gProperty#Velocity">
        <rdfs:subClassOf rdf:resource="http://hit2gap.eu/h2g/h2gProperty#PhysicalProperties"/>
        <rdfs:comment xml:lang="en">Velocity represents an observation of the  measure of the velocity of an elment in the building in a specific time.</rdfs:comment>
        <rdfs:label xml:lang="en">Velocity</rdfs:label>
    </owl:Class>
    


    <!-- http://hit2gap.eu/h2g/h2gProperty#Visibility -->

    <owl:Class rdf:about="http://hit2gap.eu/h2g/h2gProperty#Visibility">
        <rdfs:subClassOf rdf:resource="http://hit2gap.eu/h2g/h2gProperty#PhysicalProperties"/>
        <rdfs:comment xml:lang="en">Visibility represents an observation of the  measure of the visibility of an elment in the building in a specific time.</rdfs:comment>
        <rdfs:label xml:lang="en">Visibility</rdfs:label>
    </owl:Class>
    


    <!-- http://hit2gap.eu/h2g/h2gProperty#Volume -->

    <owl:Class rdf:about="http://hit2gap.eu/h2g/h2gProperty#Volume">
        <rdfs:subClassOf rdf:resource="http://hit2gap.eu/h2g/h2gProperty#PhysicalProperties"/>
        <rdfs:comment xml:lang="en">Volume represents an observation of the  measure of the volume of an elment in the building in a specific time.</rdfs:comment>
        <rdfs:label xml:lang="en">Volume</rdfs:label>
    </owl:Class>
    


    <!-- http://hit2gap.eu/h2g/h2gProperty#Weight -->

    <owl:Class rdf:about="http://hit2gap.eu/h2g/h2gProperty#Weight">
        <rdfs:subClassOf rdf:resource="http://hit2gap.eu/h2g/h2gProperty#Shape"/>
        <rdfs:comment xml:lang="en">Weight represents an observation of the  weight of an elment in the building.</rdfs:comment>
        <rdfs:label xml:lang="en">Weight</rdfs:label>
    </owl:Class>
    


    <!-- http://hit2gap.eu/h2g/h2gProperty#Width -->

    <owl:Class rdf:about="http://hit2gap.eu/h2g/h2gProperty#Width">
        <rdfs:subClassOf rdf:resource="http://hit2gap.eu/h2g/h2gProperty#Shape"/>
        <rdfs:comment xml:lang="en">Width represents an observation of the  width of an elment in the building.</rdfs:comment>
        <rdfs:label xml:lang="en">Width</rdfs:label>
    </owl:Class>
    


    <!-- http://hit2gap.eu/h2g/h2gProperty#WindOrientation -->

    <owl:Class rdf:about="http://hit2gap.eu/h2g/h2gProperty#WindOrientation">
        <rdfs:subClassOf rdf:resource="http://hit2gap.eu/h2g/h2gProperty#PhysicalProperties"/>
        <rdfs:comment xml:lang="en">WindOrientation represents an observation of the  measure of the wind orientation in a specific time.</rdfs:comment>
        <rdfs:label xml:lang="en">WindOrientation</rdfs:label>
    </owl:Class>
    


    <!-- http://hit2gap.eu/h2g/h2gProperty#WindSpeed -->

    <owl:Class rdf:about="http://hit2gap.eu/h2g/h2gProperty#WindSpeed">
        <rdfs:subClassOf rdf:resource="http://hit2gap.eu/h2g/h2gProperty#PhysicalProperties"/>
        <rdfs:comment xml:lang="en">WindSpeed represents an observation of the  measure of the wind speed  in a specific time.</rdfs:comment>
        <rdfs:label xml:lang="en">WindSpeed</rdfs:label>
    </owl:Class>
    


    <!-- http://purl.oclc.org/NET/ssnx/ssn#Property -->

    <owl:Class rdf:about="http://purl.oclc.org/NET/ssnx/ssn#Property">
        <rdfs:comment xml:lang="en">A quality of an entity. An aspect of an entity that is intrinsic to and cannot exist without the entity.</rdfs:comment>
        <rdfs:isDefinedBy rdf:resource="http://www.w3.org/ns/ssn/"/>
        <rdfs:label xml:lang="en">Property</rdfs:label>
    </owl:Class>
    


    <!-- http://www.w3.org/2002/07/owl#Thing -->

    <owl:Class rdf:about="http://www.w3.org/2002/07/owl#Thing"/>
    


    <!-- 
    ///////////////////////////////////////////////////////////////////////////////////////
    //
    // Individuals
    //
    ///////////////////////////////////////////////////////////////////////////////////////
     -->

    


    <!-- http://hit2gap.eu/h2g/h2gProperty#ColdDesert -->

    <owl:NamedIndividual rdf:about="http://hit2gap.eu/h2g/h2gProperty#ColdDesert">
        <rdf:type rdf:resource="http://hit2gap.eu/h2g/h2gProperty#Arid"/>
    </owl:NamedIndividual>
    


    <!-- http://hit2gap.eu/h2g/h2gProperty#ColdSemiArid -->

    <owl:NamedIndividual rdf:about="http://hit2gap.eu/h2g/h2gProperty#ColdSemiArid">
        <rdf:type rdf:resource="http://hit2gap.eu/h2g/h2gProperty#Arid"/>
    </owl:NamedIndividual>
    


    <!-- http://hit2gap.eu/h2g/h2gProperty#CoolSummerMediterranean -->

    <owl:NamedIndividual rdf:about="http://hit2gap.eu/h2g/h2gProperty#CoolSummerMediterranean">
        <rdf:type rdf:resource="http://hit2gap.eu/h2g/h2gProperty#Temperate"/>
    </owl:NamedIndividual>
    


    <!-- http://hit2gap.eu/h2g/h2gProperty#DrySummerSubarctic -->

    <owl:NamedIndividual rdf:about="http://hit2gap.eu/h2g/h2gProperty#DrySummerSubarctic">
        <rdf:type rdf:resource="http://hit2gap.eu/h2g/h2gProperty#Continental"/>
    </owl:NamedIndividual>
    


    <!-- http://hit2gap.eu/h2g/h2gProperty#ExtremelyColdDrySummerSubarctic -->

    <owl:NamedIndividual rdf:about="http://hit2gap.eu/h2g/h2gProperty#ExtremelyColdDrySummerSubarctic">
        <rdf:type rdf:resource="http://hit2gap.eu/h2g/h2gProperty#Continental"/>
    </owl:NamedIndividual>
    


    <!-- http://hit2gap.eu/h2g/h2gProperty#ExtremelyColdSubartic -->

    <owl:NamedIndividual rdf:about="http://hit2gap.eu/h2g/h2gProperty#ExtremelyColdSubartic">
        <rdf:type rdf:resource="http://hit2gap.eu/h2g/h2gProperty#Continental"/>
    </owl:NamedIndividual>
    


    <!-- http://hit2gap.eu/h2g/h2gProperty#FrostColdTundra -->

    <owl:NamedIndividual rdf:about="http://hit2gap.eu/h2g/h2gProperty#FrostColdTundra">
        <rdf:type rdf:resource="http://hit2gap.eu/h2g/h2gProperty#Polar"/>
    </owl:NamedIndividual>
    


    <!-- http://hit2gap.eu/h2g/h2gProperty#HotDesert -->

    <owl:NamedIndividual rdf:about="http://hit2gap.eu/h2g/h2gProperty#HotDesert">
        <rdf:type rdf:resource="http://hit2gap.eu/h2g/h2gProperty#Arid"/>
    </owl:NamedIndividual>
    


    <!-- http://hit2gap.eu/h2g/h2gProperty#HotDrySummerContinental -->

    <owl:NamedIndividual rdf:about="http://hit2gap.eu/h2g/h2gProperty#HotDrySummerContinental">
        <rdf:type rdf:resource="http://hit2gap.eu/h2g/h2gProperty#Continental"/>
    </owl:NamedIndividual>
    


    <!-- http://hit2gap.eu/h2g/h2gProperty#HotSemiArid -->

    <owl:NamedIndividual rdf:about="http://hit2gap.eu/h2g/h2gProperty#HotSemiArid">
        <rdf:type rdf:resource="http://hit2gap.eu/h2g/h2gProperty#Arid"/>
    </owl:NamedIndividual>
    


    <!-- http://hit2gap.eu/h2g/h2gProperty#HotSummerHumidContinental -->

    <owl:NamedIndividual rdf:about="http://hit2gap.eu/h2g/h2gProperty#HotSummerHumidContinental">
        <rdf:type rdf:resource="http://hit2gap.eu/h2g/h2gProperty#Continental"/>
    </owl:NamedIndividual>
    


    <!-- http://hit2gap.eu/h2g/h2gProperty#HotSummerMediterranean -->

    <owl:NamedIndividual rdf:about="http://hit2gap.eu/h2g/h2gProperty#HotSummerMediterranean">
        <rdf:type rdf:resource="http://hit2gap.eu/h2g/h2gProperty#Temperate"/>
    </owl:NamedIndividual>
    


    <!-- http://hit2gap.eu/h2g/h2gProperty#HumidSubtropical -->

    <owl:NamedIndividual rdf:about="http://hit2gap.eu/h2g/h2gProperty#HumidSubtropical">
        <rdf:type rdf:resource="http://hit2gap.eu/h2g/h2gProperty#Temperate"/>
    </owl:NamedIndividual>
    


    <!-- http://hit2gap.eu/h2g/h2gProperty#IceCap -->

    <owl:NamedIndividual rdf:about="http://hit2gap.eu/h2g/h2gProperty#IceCap">
        <rdf:type rdf:resource="http://hit2gap.eu/h2g/h2gProperty#Polar"/>
    </owl:NamedIndividual>
    


    <!-- http://hit2gap.eu/h2g/h2gProperty#MildDesert -->

    <owl:NamedIndividual rdf:about="http://hit2gap.eu/h2g/h2gProperty#MildDesert">
        <rdf:type rdf:resource="http://hit2gap.eu/h2g/h2gProperty#Arid"/>
    </owl:NamedIndividual>
    


    <!-- http://hit2gap.eu/h2g/h2gProperty#MildSemiArid -->

    <owl:NamedIndividual rdf:about="http://hit2gap.eu/h2g/h2gProperty#MildSemiArid">
        <rdf:type rdf:resource="http://hit2gap.eu/h2g/h2gProperty#Arid"/>
    </owl:NamedIndividual>
    


    <!-- http://hit2gap.eu/h2g/h2gProperty#MildTundra -->

    <owl:NamedIndividual rdf:about="http://hit2gap.eu/h2g/h2gProperty#MildTundra">
        <rdf:type rdf:resource="http://hit2gap.eu/h2g/h2gProperty#Polar"/>
    </owl:NamedIndividual>
    


    <!-- http://hit2gap.eu/h2g/h2gProperty#MonsoonInfluencedExtremelyColdSubarctic -->

    <owl:NamedIndividual rdf:about="http://hit2gap.eu/h2g/h2gProperty#MonsoonInfluencedExtremelyColdSubarctic">
        <rdf:type rdf:resource="http://hit2gap.eu/h2g/h2gProperty#Continental"/>
    </owl:NamedIndividual>
    


    <!-- http://hit2gap.eu/h2g/h2gProperty#MonsoonInfluencedHotSummerHumidContinental -->

    <owl:NamedIndividual rdf:about="http://hit2gap.eu/h2g/h2gProperty#MonsoonInfluencedHotSummerHumidContinental">
        <rdf:type rdf:resource="http://hit2gap.eu/h2g/h2gProperty#Continental"/>
    </owl:NamedIndividual>
    


    <!-- http://hit2gap.eu/h2g/h2gProperty#MonsoonInfluencedHumidSubtropical -->

    <owl:NamedIndividual rdf:about="http://hit2gap.eu/h2g/h2gProperty#MonsoonInfluencedHumidSubtropical">
        <rdf:type rdf:resource="http://hit2gap.eu/h2g/h2gProperty#Temperate"/>
    </owl:NamedIndividual>
    


    <!-- http://hit2gap.eu/h2g/h2gProperty#MonsoonInfluencedSubartic -->

    <owl:NamedIndividual rdf:about="http://hit2gap.eu/h2g/h2gProperty#MonsoonInfluencedSubartic">
        <rdf:type rdf:resource="http://hit2gap.eu/h2g/h2gProperty#Continental"/>
    </owl:NamedIndividual>
    


    <!-- http://hit2gap.eu/h2g/h2gProperty#MonsoonInfluencedWarmSummerHumidContinental -->

    <owl:NamedIndividual rdf:about="http://hit2gap.eu/h2g/h2gProperty#MonsoonInfluencedWarmSummerHumidContinental">
        <rdf:type rdf:resource="http://hit2gap.eu/h2g/h2gProperty#Continental"/>
    </owl:NamedIndividual>
    


    <!-- http://hit2gap.eu/h2g/h2gProperty#SubPolarOceanicWithDryWinters -->

    <owl:NamedIndividual rdf:about="http://hit2gap.eu/h2g/h2gProperty#SubPolarOceanicWithDryWinters">
        <rdf:type rdf:resource="http://hit2gap.eu/h2g/h2gProperty#Temperate"/>
    </owl:NamedIndividual>
    


    <!-- http://hit2gap.eu/h2g/h2gProperty#Subartic -->

    <owl:NamedIndividual rdf:about="http://hit2gap.eu/h2g/h2gProperty#Subartic">
        <rdf:type rdf:resource="http://hit2gap.eu/h2g/h2gProperty#Continental"/>
    </owl:NamedIndividual>
    


    <!-- http://hit2gap.eu/h2g/h2gProperty#SubpolarOceanic -->

    <owl:NamedIndividual rdf:about="http://hit2gap.eu/h2g/h2gProperty#SubpolarOceanic">
        <rdf:type rdf:resource="http://hit2gap.eu/h2g/h2gProperty#Temperate"/>
    </owl:NamedIndividual>
    


    <!-- http://hit2gap.eu/h2g/h2gProperty#TemperateOceanic -->

    <owl:NamedIndividual rdf:about="http://hit2gap.eu/h2g/h2gProperty#TemperateOceanic">
        <rdf:type rdf:resource="http://hit2gap.eu/h2g/h2gProperty#Temperate"/>
    </owl:NamedIndividual>
    


    <!-- http://hit2gap.eu/h2g/h2gProperty#TemperateOceanicWithDryWinters -->

    <owl:NamedIndividual rdf:about="http://hit2gap.eu/h2g/h2gProperty#TemperateOceanicWithDryWinters">
        <rdf:type rdf:resource="http://hit2gap.eu/h2g/h2gProperty#Temperate"/>
    </owl:NamedIndividual>
    


    <!-- http://hit2gap.eu/h2g/h2gProperty#TropicalMonsoon -->

    <owl:NamedIndividual rdf:about="http://hit2gap.eu/h2g/h2gProperty#TropicalMonsoon">
        <rdf:type rdf:resource="http://hit2gap.eu/h2g/h2gProperty#Tropical"/>
    </owl:NamedIndividual>
    


    <!-- http://hit2gap.eu/h2g/h2gProperty#TropicalRainforest -->

    <owl:NamedIndividual rdf:about="http://hit2gap.eu/h2g/h2gProperty#TropicalRainforest">
        <rdf:type rdf:resource="http://hit2gap.eu/h2g/h2gProperty#Tropical"/>
    </owl:NamedIndividual>
    


    <!-- http://hit2gap.eu/h2g/h2gProperty#TropicalSavanna -->

    <owl:NamedIndividual rdf:about="http://hit2gap.eu/h2g/h2gProperty#TropicalSavanna">
        <rdf:type rdf:resource="http://hit2gap.eu/h2g/h2gProperty#Tropical"/>
    </owl:NamedIndividual>
    


    <!-- http://hit2gap.eu/h2g/h2gProperty#WarmDrySummerContinental -->

    <owl:NamedIndividual rdf:about="http://hit2gap.eu/h2g/h2gProperty#WarmDrySummerContinental">
        <rdf:type rdf:resource="http://hit2gap.eu/h2g/h2gProperty#Continental"/>
    </owl:NamedIndividual>
    


    <!-- http://hit2gap.eu/h2g/h2gProperty#WarmSummerHumidContinental -->

    <owl:NamedIndividual rdf:about="http://hit2gap.eu/h2g/h2gProperty#WarmSummerHumidContinental">
        <rdf:type rdf:resource="http://hit2gap.eu/h2g/h2gProperty#Continental"/>
    </owl:NamedIndividual>
    


    <!-- http://hit2gap.eu/h2g/h2gProperty#WarnSummerMediterranean -->

    <owl:NamedIndividual rdf:about="http://hit2gap.eu/h2g/h2gProperty#WarnSummerMediterranean">
        <rdf:type rdf:resource="http://hit2gap.eu/h2g/h2gProperty#Temperate"/>
    </owl:NamedIndividual>
</rdf:RDF>



<!-- Generated by the OWL API (version 4.3.1) https://github.com/owlcs/owlapi -->

